PREFIX owl: <http://www.w3.org/2002/07/owl#>
PREFIX rdfs: <http://www.w3.org/2000/01/rdf-schema#>
PREFIX xsd: <http://www.w3.org/2001/XMLSchema#>

<https://atproto.social/ontology/app.bsky.actor.defs#verificationState>
        a             owl:Class;
        rdfs:comment  "Represents the verification information about the user this object is attached to." .

<https://atproto.social/ontology/app.bsky.actor.defs#verificationState/verifications>
        a             owl:ObjectProperty;
        rdfs:domain   <https://atproto.social/ontology/app.bsky.actor.defs#verificationState>;
        rdfs:range    <https://atproto.social/ontology/app.bsky.actor.defs#verificationView>;
        rdfs:comment  "All verifications issued by trusted verifiers on behalf of this user. Verifications by untrusted verifiers are not included." .

<https://atproto.social/ontology/app.bsky.actor.defs#verificationState/verifiedStatus>
        a             owl:DatatypeProperty;
        rdfs:domain   <https://atproto.social/ontology/app.bsky.actor.defs#verificationState>;
        rdfs:range    <xsd:string>;
        rdfs:comment  "The user's status as a verified account." .

<https://atproto.social/ontology/app.bsky.actor.defs#verificationState/trustedVerifierStatus>
        a             owl:DatatypeProperty;
        rdfs:domain   <https://atproto.social/ontology/app.bsky.actor.defs#verificationState>;
        rdfs:range    <xsd:string>;
        rdfs:comment  "The user's status as a trusted verifier." .

<https://atproto.social/ontology/app.bsky.actor.defs#contentLabelPref>
        a       owl:Class .

<https://atproto.social/ontology/app.bsky.actor.defs#contentLabelPref/labelerDid>
        a             owl:DatatypeProperty;
        rdfs:domain   <https://atproto.social/ontology/app.bsky.actor.defs#contentLabelPref>;
        rdfs:range    <xsd:string>;
        rdfs:comment  "Which labeler does this preference apply to? If undefined, applies globally." .

<https://atproto.social/ontology/app.bsky.actor.defs#contentLabelPref/label>
        a            owl:DatatypeProperty;
        rdfs:domain  <https://atproto.social/ontology/app.bsky.actor.defs#contentLabelPref>;
        rdfs:range   <xsd:string> .

<https://atproto.social/ontology/app.bsky.actor.defs#contentLabelPref/visibility>
        a            owl:DatatypeProperty;
        rdfs:domain  <https://atproto.social/ontology/app.bsky.actor.defs#contentLabelPref>;
        rdfs:range   <xsd:string> .

<https://atproto.social/ontology/app.bsky.actor.defs#bskyAppProgressGuide>
        a             owl:Class;
        rdfs:comment  "If set, an active progress guide. Once completed, can be set to undefined. Should have unspecced fields tracking progress." .

<https://atproto.social/ontology/app.bsky.actor.defs#bskyAppProgressGuide/guide>
        a            owl:DatatypeProperty;
        rdfs:domain  <https://atproto.social/ontology/app.bsky.actor.defs#bskyAppProgressGuide>;
        rdfs:range   <xsd:string> .

<https://atproto.social/ontology/app.bsky.actor.defs#knownFollowers>
        a             owl:Class;
        rdfs:comment  "The subject's followers whom you also follow" .

<https://atproto.social/ontology/app.bsky.actor.defs#knownFollowers/count>
        a            owl:DatatypeProperty;
        rdfs:domain  <https://atproto.social/ontology/app.bsky.actor.defs#knownFollowers>;
        rdfs:range   <xsd:integer> .

<https://atproto.social/ontology/app.bsky.actor.defs#knownFollowers/followers>
        a            owl:ObjectProperty;
        rdfs:domain  <https://atproto.social/ontology/app.bsky.actor.defs#knownFollowers>;
        rdfs:range   <https://atproto.social/ontology/app.bsky.actor.defs#profileViewBasic> .

<https://atproto.social/ontology/app.bsky.actor.defs#mutedWord>
        a             owl:Class;
        rdfs:comment  "A word that the account owner has muted." .

<https://atproto.social/ontology/app.bsky.actor.defs#mutedWord/value>
        a             owl:DatatypeProperty;
        rdfs:domain   <https://atproto.social/ontology/app.bsky.actor.defs#mutedWord>;
        rdfs:range    <xsd:string>;
        rdfs:comment  "The muted word itself." .

<https://atproto.social/ontology/app.bsky.actor.defs#mutedWord/targets>
        a             owl:ObjectProperty;
        rdfs:domain   <https://atproto.social/ontology/app.bsky.actor.defs#mutedWord>;
        rdfs:range    <https://atproto.social/ontology/app.bsky.actor.defs#mutedWordTarget>;
        rdfs:comment  "The intended targets of the muted word." .

<https://atproto.social/ontology/app.bsky.actor.defs#mutedWord/actorTarget>
        a             owl:DatatypeProperty;
        rdfs:domain   <https://atproto.social/ontology/app.bsky.actor.defs#mutedWord>;
        rdfs:range    <xsd:string>;
        rdfs:comment  "Groups of users to apply the muted word to. If undefined, applies to all users." .

<https://atproto.social/ontology/app.bsky.actor.defs#mutedWord/expiresAt>
        a             owl:DatatypeProperty;
        rdfs:domain   <https://atproto.social/ontology/app.bsky.actor.defs#mutedWord>;
        rdfs:range    <xsd:string>;
        rdfs:comment  "The date and time at which the muted word will expire and no longer be applied." .

<https://atproto.social/ontology/app.bsky.actor.defs#mutedWord/id>
        a            owl:DatatypeProperty;
        rdfs:domain  <https://atproto.social/ontology/app.bsky.actor.defs#mutedWord>;
        rdfs:range   <xsd:string> .

<https://atproto.social/ontology/app.bsky.actor.defs#verificationPrefs>
        a             owl:Class;
        rdfs:comment  "Preferences for how verified accounts appear in the app." .

<https://atproto.social/ontology/app.bsky.actor.defs#verificationPrefs/hideBadges>
        a             owl:DatatypeProperty;
        rdfs:domain   <https://atproto.social/ontology/app.bsky.actor.defs#verificationPrefs>;
        rdfs:range    <xsd:boolean>;
        rdfs:comment  "Hide the blue check badges for verified accounts and trusted verifiers." .

<https://atproto.social/ontology/app.bsky.actor.defs#postInteractionSettingsPref>
        a             owl:Class;
        rdfs:comment  "Default post interaction settings for the account. These values should be applied as default values when creating new posts. These refs should mirror the threadgate and postgate records exactly." .

<https://atproto.social/ontology/app.bsky.actor.defs#postInteractionSettingsPref/threadgateAllowRules>
        a             owl:ObjectProperty;
        rdfs:domain   <https://atproto.social/ontology/app.bsky.actor.defs#postInteractionSettingsPref>;
        rdfs:comment  "Matches threadgate record. List of rules defining who can reply to this users posts. If value is an empty array, no one can reply. If value is undefined, anyone can reply." .

<https://atproto.social/ontology/app.bsky.actor.defs#postInteractionSettingsPref/postgateEmbeddingRules>
        a             owl:ObjectProperty;
        rdfs:domain   <https://atproto.social/ontology/app.bsky.actor.defs#postInteractionSettingsPref>;
        rdfs:comment  "Matches postgate record. List of rules defining who can embed this users posts. If value is an empty array or is undefined, no particular rules apply and anyone can embed." .

<https://atproto.social/ontology/app.bsky.actor.defs#statusView>
        a       owl:Class .

<https://atproto.social/ontology/app.bsky.actor.defs#statusView/expiresAt>
        a             owl:DatatypeProperty;
        rdfs:domain   <https://atproto.social/ontology/app.bsky.actor.defs#statusView>;
        rdfs:range    <xsd:string>;
        rdfs:comment  "The date when this status will expire. The application might choose to no longer return the status after expiration." .

<https://atproto.social/ontology/app.bsky.actor.defs#statusView/isActive>
        a             owl:DatatypeProperty;
        rdfs:domain   <https://atproto.social/ontology/app.bsky.actor.defs#statusView>;
        rdfs:range    <xsd:boolean>;
        rdfs:comment  "True if the status is not expired, false if it is expired. Only present if expiration was set." .

<https://atproto.social/ontology/app.bsky.actor.defs#statusView/status>
        a             owl:DatatypeProperty;
        rdfs:domain   <https://atproto.social/ontology/app.bsky.actor.defs#statusView>;
        rdfs:range    <xsd:string>;
        rdfs:comment  "The status for the account." .

<https://atproto.social/ontology/app.bsky.actor.defs#statusView/record>
        a            owl:ObjectProperty;
        rdfs:domain  <https://atproto.social/ontology/app.bsky.actor.defs#statusView> .

<https://atproto.social/ontology/app.bsky.actor.defs#statusView/embed>
        a             owl:ObjectProperty;
        rdfs:domain   <https://atproto.social/ontology/app.bsky.actor.defs#statusView>;
        rdfs:comment  "An optional embed associated with the status." .

<https://atproto.social/ontology/app.bsky.actor.defs#labelersPref>
        a       owl:Class .

<https://atproto.social/ontology/app.bsky.actor.defs#labelersPref/labelers>
        a            owl:ObjectProperty;
        rdfs:domain  <https://atproto.social/ontology/app.bsky.actor.defs#labelersPref>;
        rdfs:range   <https://atproto.social/ontology/app.bsky.actor.defs#labelerPrefItem> .

<https://atproto.social/ontology/app.bsky.actor.defs#verificationView>
        a             owl:Class;
        rdfs:comment  "An individual verification for an associated subject." .

<https://atproto.social/ontology/app.bsky.actor.defs#verificationView/isValid>
        a             owl:DatatypeProperty;
        rdfs:domain   <https://atproto.social/ontology/app.bsky.actor.defs#verificationView>;
        rdfs:range    <xsd:boolean>;
        rdfs:comment  "True if the verification passes validation, otherwise false." .

<https://atproto.social/ontology/app.bsky.actor.defs#verificationView/createdAt>
        a             owl:DatatypeProperty;
        rdfs:domain   <https://atproto.social/ontology/app.bsky.actor.defs#verificationView>;
        rdfs:range    <xsd:string>;
        rdfs:comment  "Timestamp when the verification was created." .

<https://atproto.social/ontology/app.bsky.actor.defs#verificationView/issuer>
        a             owl:DatatypeProperty;
        rdfs:domain   <https://atproto.social/ontology/app.bsky.actor.defs#verificationView>;
        rdfs:range    <xsd:string>;
        rdfs:comment  "The user who issued this verification." .

<https://atproto.social/ontology/app.bsky.actor.defs#verificationView/uri>
        a             owl:DatatypeProperty;
        rdfs:domain   <https://atproto.social/ontology/app.bsky.actor.defs#verificationView>;
        rdfs:range    <xsd:string>;
        rdfs:comment  "The AT-URI of the verification record." .

<https://atproto.social/ontology/app.bsky.actor.defs#savedFeed>
        a       owl:Class .

<https://atproto.social/ontology/app.bsky.actor.defs#savedFeed/pinned>
        a            owl:DatatypeProperty;
        rdfs:domain  <https://atproto.social/ontology/app.bsky.actor.defs#savedFeed>;
        rdfs:range   <xsd:boolean> .

<https://atproto.social/ontology/app.bsky.actor.defs#savedFeed/id>
        a            owl:DatatypeProperty;
        rdfs:domain  <https://atproto.social/ontology/app.bsky.actor.defs#savedFeed>;
        rdfs:range   <xsd:string> .

<https://atproto.social/ontology/app.bsky.actor.defs#savedFeed/type>
        a            owl:DatatypeProperty;
        rdfs:domain  <https://atproto.social/ontology/app.bsky.actor.defs#savedFeed>;
        rdfs:range   <xsd:string> .

<https://atproto.social/ontology/app.bsky.actor.defs#savedFeed/value>
        a            owl:DatatypeProperty;
        rdfs:domain  <https://atproto.social/ontology/app.bsky.actor.defs#savedFeed>;
        rdfs:range   <xsd:string> .

<https://atproto.social/ontology/app.bsky.actor.defs#personalDetailsPref>
        a       owl:Class .

<https://atproto.social/ontology/app.bsky.actor.defs#personalDetailsPref/birthDate>
        a             owl:DatatypeProperty;
        rdfs:domain   <https://atproto.social/ontology/app.bsky.actor.defs#personalDetailsPref>;
        rdfs:range    <xsd:string>;
        rdfs:comment  "The birth date of account owner." .

<https://atproto.social/ontology/app.bsky.actor.defs#mutedWordTarget>
        a       owl:Class .

<https://atproto.social/ontology/app.bsky.actor.defs#profileAssociated>
        a       owl:Class .

<https://atproto.social/ontology/app.bsky.actor.defs#profileAssociated/lists>
        a            owl:DatatypeProperty;
        rdfs:domain  <https://atproto.social/ontology/app.bsky.actor.defs#profileAssociated>;
        rdfs:range   <xsd:integer> .

<https://atproto.social/ontology/app.bsky.actor.defs#profileAssociated/feedgens>
        a            owl:DatatypeProperty;
        rdfs:domain  <https://atproto.social/ontology/app.bsky.actor.defs#profileAssociated>;
        rdfs:range   <xsd:integer> .

<https://atproto.social/ontology/app.bsky.actor.defs#profileAssociated/starterPacks>
        a            owl:DatatypeProperty;
        rdfs:domain  <https://atproto.social/ontology/app.bsky.actor.defs#profileAssociated>;
        rdfs:range   <xsd:integer> .

<https://atproto.social/ontology/app.bsky.actor.defs#profileAssociated/labeler>
        a            owl:DatatypeProperty;
        rdfs:domain  <https://atproto.social/ontology/app.bsky.actor.defs#profileAssociated>;
        rdfs:range   <xsd:boolean> .

<https://atproto.social/ontology/app.bsky.actor.defs#profileAssociated/chat>
        a            owl:ObjectProperty;
        rdfs:domain  <https://atproto.social/ontology/app.bsky.actor.defs#profileAssociated>;
        rdfs:range   <https://atproto.social/ontology/app.bsky.actor.defs#profileAssociatedChat> .

<https://atproto.social/ontology/app.bsky.actor.defs#profileAssociated/activitySubscription>
        a            owl:ObjectProperty;
        rdfs:domain  <https://atproto.social/ontology/app.bsky.actor.defs#profileAssociated>;
        rdfs:range   <https://atproto.social/ontology/app.bsky.actor.defs#profileAssociatedActivitySubscription> .

<https://atproto.social/ontology/app.bsky.actor.defs#threadViewPref>
        a       owl:Class .

<https://atproto.social/ontology/app.bsky.actor.defs#threadViewPref/sort>
        a             owl:DatatypeProperty;
        rdfs:domain   <https://atproto.social/ontology/app.bsky.actor.defs#threadViewPref>;
        rdfs:range    <xsd:string>;
        rdfs:comment  "Sorting mode for threads." .

<https://atproto.social/ontology/app.bsky.actor.defs#threadViewPref/prioritizeFollowedUsers>
        a             owl:DatatypeProperty;
        rdfs:domain   <https://atproto.social/ontology/app.bsky.actor.defs#threadViewPref>;
        rdfs:range    <xsd:boolean>;
        rdfs:comment  "Show followed users at the top of all replies." .

<https://atproto.social/ontology/app.bsky.actor.defs#interestsPref>
        a       owl:Class .

<https://atproto.social/ontology/app.bsky.actor.defs#interestsPref/tags>
        a             owl:DatatypeProperty;
        rdfs:domain   <https://atproto.social/ontology/app.bsky.actor.defs#interestsPref>;
        rdfs:range    <xsd:string>;
        rdfs:comment  "A list of tags which describe the account owner's interests gathered during onboarding." .

<https://atproto.social/ontology/app.bsky.actor.defs#labelerPrefItem>
        a       owl:Class .

<https://atproto.social/ontology/app.bsky.actor.defs#labelerPrefItem/did>
        a            owl:DatatypeProperty;
        rdfs:domain  <https://atproto.social/ontology/app.bsky.actor.defs#labelerPrefItem>;
        rdfs:range   <xsd:string> .

<https://atproto.social/ontology/app.bsky.actor.defs#bskyAppStatePref>
        a             owl:Class;
        rdfs:comment  "A grab bag of state that's specific to the bsky.app program. Third-party apps shouldn't use this." .

<https://atproto.social/ontology/app.bsky.actor.defs#bskyAppStatePref/queuedNudges>
        a             owl:DatatypeProperty;
        rdfs:domain   <https://atproto.social/ontology/app.bsky.actor.defs#bskyAppStatePref>;
        rdfs:range    <xsd:string>;
        rdfs:comment  "An array of tokens which identify nudges (modals, popups, tours, highlight dots) that should be shown to the user." .

<https://atproto.social/ontology/app.bsky.actor.defs#bskyAppStatePref/nuxs>
        a             owl:ObjectProperty;
        rdfs:domain   <https://atproto.social/ontology/app.bsky.actor.defs#bskyAppStatePref>;
        rdfs:range    <https://atproto.social/ontology/app.bsky.actor.defs#nux>;
        rdfs:comment  "Storage for NUXs the user has encountered." .

<https://atproto.social/ontology/app.bsky.actor.defs#bskyAppStatePref/activeProgressGuide>
        a            owl:ObjectProperty;
        rdfs:domain  <https://atproto.social/ontology/app.bsky.actor.defs#bskyAppStatePref>;
        rdfs:range   <https://atproto.social/ontology/app.bsky.actor.defs#bskyAppProgressGuide> .

<https://atproto.social/ontology/app.bsky.actor.defs#profileAssociatedActivitySubscription>
        a       owl:Class .

<https://atproto.social/ontology/app.bsky.actor.defs#profileAssociatedActivitySubscription/allowSubscriptions>
        a            owl:DatatypeProperty;
        rdfs:domain  <https://atproto.social/ontology/app.bsky.actor.defs#profileAssociatedActivitySubscription>;
        rdfs:range   <xsd:string> .

<https://atproto.social/ontology/app.bsky.actor.defs#preferences>
        a       owl:Class .

<https://atproto.social/ontology/app.bsky.actor.defs#feedViewPref>
        a       owl:Class .

<https://atproto.social/ontology/app.bsky.actor.defs#feedViewPref/feed>
        a             owl:DatatypeProperty;
        rdfs:domain   <https://atproto.social/ontology/app.bsky.actor.defs#feedViewPref>;
        rdfs:range    <xsd:string>;
        rdfs:comment  "The URI of the feed, or an identifier which describes the feed." .

<https://atproto.social/ontology/app.bsky.actor.defs#feedViewPref/hideReplies>
        a             owl:DatatypeProperty;
        rdfs:domain   <https://atproto.social/ontology/app.bsky.actor.defs#feedViewPref>;
        rdfs:range    <xsd:boolean>;
        rdfs:comment  "Hide replies in the feed." .

<https://atproto.social/ontology/app.bsky.actor.defs#feedViewPref/hideRepliesByUnfollowed>
        a             owl:DatatypeProperty;
        rdfs:domain   <https://atproto.social/ontology/app.bsky.actor.defs#feedViewPref>;
        rdfs:range    <xsd:boolean>;
        rdfs:comment  "Hide replies in the feed if they are not by followed users." .

<https://atproto.social/ontology/app.bsky.actor.defs#feedViewPref/hideRepliesByLikeCount>
        a             owl:DatatypeProperty;
        rdfs:domain   <https://atproto.social/ontology/app.bsky.actor.defs#feedViewPref>;
        rdfs:range    <xsd:integer>;
        rdfs:comment  "Hide replies in the feed if they do not have this number of likes." .

<https://atproto.social/ontology/app.bsky.actor.defs#feedViewPref/hideReposts>
        a             owl:DatatypeProperty;
        rdfs:domain   <https://atproto.social/ontology/app.bsky.actor.defs#feedViewPref>;
        rdfs:range    <xsd:boolean>;
        rdfs:comment  "Hide reposts in the feed." .

<https://atproto.social/ontology/app.bsky.actor.defs#feedViewPref/hideQuotePosts>
        a             owl:DatatypeProperty;
        rdfs:domain   <https://atproto.social/ontology/app.bsky.actor.defs#feedViewPref>;
        rdfs:range    <xsd:boolean>;
        rdfs:comment  "Hide quote posts in the feed." .

<https://atproto.social/ontology/app.bsky.actor.defs#profileViewBasic>
        a       owl:Class .

<https://atproto.social/ontology/app.bsky.actor.defs#profileViewBasic/displayName>
        a            owl:DatatypeProperty;
        rdfs:domain  <https://atproto.social/ontology/app.bsky.actor.defs#profileViewBasic>;
        rdfs:range   <xsd:string> .

<https://atproto.social/ontology/app.bsky.actor.defs#profileViewBasic/associated>
        a            owl:ObjectProperty;
        rdfs:domain  <https://atproto.social/ontology/app.bsky.actor.defs#profileViewBasic>;
        rdfs:range   <https://atproto.social/ontology/app.bsky.actor.defs#profileAssociated> .

<https://atproto.social/ontology/app.bsky.actor.defs#profileViewBasic/viewer>
        a            owl:ObjectProperty;
        rdfs:domain  <https://atproto.social/ontology/app.bsky.actor.defs#profileViewBasic>;
        rdfs:range   <https://atproto.social/ontology/app.bsky.actor.defs#viewerState> .

<https://atproto.social/ontology/app.bsky.actor.defs#profileViewBasic/labels>
        a            owl:ObjectProperty;
        rdfs:domain  <https://atproto.social/ontology/app.bsky.actor.defs#profileViewBasic>;
        rdfs:range   <https://atproto.social/ontology/com.atproto.label.defs#label> .

<https://atproto.social/ontology/app.bsky.actor.defs#profileViewBasic/verification>
        a            owl:ObjectProperty;
        rdfs:domain  <https://atproto.social/ontology/app.bsky.actor.defs#profileViewBasic>;
        rdfs:range   <https://atproto.social/ontology/app.bsky.actor.defs#verificationState> .

<https://atproto.social/ontology/app.bsky.actor.defs#profileViewBasic/did>
        a            owl:DatatypeProperty;
        rdfs:domain  <https://atproto.social/ontology/app.bsky.actor.defs#profileViewBasic>;
        rdfs:range   <xsd:string> .

<https://atproto.social/ontology/app.bsky.actor.defs#profileViewBasic/avatar>
        a            owl:DatatypeProperty;
        rdfs:domain  <https://atproto.social/ontology/app.bsky.actor.defs#profileViewBasic>;
        rdfs:range   <xsd:string> .

<https://atproto.social/ontology/app.bsky.actor.defs#profileViewBasic/createdAt>
        a            owl:DatatypeProperty;
        rdfs:domain  <https://atproto.social/ontology/app.bsky.actor.defs#profileViewBasic>;
        rdfs:range   <xsd:string> .

<https://atproto.social/ontology/app.bsky.actor.defs#profileViewBasic/status>
        a            owl:ObjectProperty;
        rdfs:domain  <https://atproto.social/ontology/app.bsky.actor.defs#profileViewBasic>;
        rdfs:range   <https://atproto.social/ontology/app.bsky.actor.defs#statusView> .

<https://atproto.social/ontology/app.bsky.actor.defs#profileViewBasic/handle>
        a            owl:DatatypeProperty;
        rdfs:domain  <https://atproto.social/ontology/app.bsky.actor.defs#profileViewBasic>;
        rdfs:range   <xsd:string> .

<https://atproto.social/ontology/app.bsky.actor.defs#profileView>
        a       owl:Class .

<https://atproto.social/ontology/app.bsky.actor.defs#profileView/createdAt>
        a            owl:DatatypeProperty;
        rdfs:domain  <https://atproto.social/ontology/app.bsky.actor.defs#profileView>;
        rdfs:range   <xsd:string> .

<https://atproto.social/ontology/app.bsky.actor.defs#profileView/verification>
        a            owl:ObjectProperty;
        rdfs:domain  <https://atproto.social/ontology/app.bsky.actor.defs#profileView>;
        rdfs:range   <https://atproto.social/ontology/app.bsky.actor.defs#verificationState> .

<https://atproto.social/ontology/app.bsky.actor.defs#profileView/status>
        a            owl:ObjectProperty;
        rdfs:domain  <https://atproto.social/ontology/app.bsky.actor.defs#profileView>;
        rdfs:range   <https://atproto.social/ontology/app.bsky.actor.defs#statusView> .

<https://atproto.social/ontology/app.bsky.actor.defs#profileView/did>
        a            owl:DatatypeProperty;
        rdfs:domain  <https://atproto.social/ontology/app.bsky.actor.defs#profileView>;
        rdfs:range   <xsd:string> .

<https://atproto.social/ontology/app.bsky.actor.defs#profileView/displayName>
        a            owl:DatatypeProperty;
        rdfs:domain  <https://atproto.social/ontology/app.bsky.actor.defs#profileView>;
        rdfs:range   <xsd:string> .

<https://atproto.social/ontology/app.bsky.actor.defs#profileView/avatar>
        a            owl:DatatypeProperty;
        rdfs:domain  <https://atproto.social/ontology/app.bsky.actor.defs#profileView>;
        rdfs:range   <xsd:string> .

<https://atproto.social/ontology/app.bsky.actor.defs#profileView/associated>
        a            owl:ObjectProperty;
        rdfs:domain  <https://atproto.social/ontology/app.bsky.actor.defs#profileView>;
        rdfs:range   <https://atproto.social/ontology/app.bsky.actor.defs#profileAssociated> .

<https://atproto.social/ontology/app.bsky.actor.defs#profileView/indexedAt>
        a            owl:DatatypeProperty;
        rdfs:domain  <https://atproto.social/ontology/app.bsky.actor.defs#profileView>;
        rdfs:range   <xsd:string> .

<https://atproto.social/ontology/app.bsky.actor.defs#profileView/viewer>
        a            owl:ObjectProperty;
        rdfs:domain  <https://atproto.social/ontology/app.bsky.actor.defs#profileView>;
        rdfs:range   <https://atproto.social/ontology/app.bsky.actor.defs#viewerState> .

<https://atproto.social/ontology/app.bsky.actor.defs#profileView/labels>
        a            owl:ObjectProperty;
        rdfs:domain  <https://atproto.social/ontology/app.bsky.actor.defs#profileView>;
        rdfs:range   <https://atproto.social/ontology/com.atproto.label.defs#label> .

<https://atproto.social/ontology/app.bsky.actor.defs#profileView/handle>
        a            owl:DatatypeProperty;
        rdfs:domain  <https://atproto.social/ontology/app.bsky.actor.defs#profileView>;
        rdfs:range   <xsd:string> .

<https://atproto.social/ontology/app.bsky.actor.defs#profileView/description>
        a            owl:DatatypeProperty;
        rdfs:domain  <https://atproto.social/ontology/app.bsky.actor.defs#profileView>;
        rdfs:range   <xsd:string> .

<https://atproto.social/ontology/app.bsky.actor.defs#profileViewDetailed>
        a       owl:Class .

<https://atproto.social/ontology/app.bsky.actor.defs#profileViewDetailed/verification>
        a            owl:ObjectProperty;
        rdfs:domain  <https://atproto.social/ontology/app.bsky.actor.defs#profileViewDetailed>;
        rdfs:range   <https://atproto.social/ontology/app.bsky.actor.defs#verificationState> .

<https://atproto.social/ontology/app.bsky.actor.defs#profileViewDetailed/viewer>
        a            owl:ObjectProperty;
        rdfs:domain  <https://atproto.social/ontology/app.bsky.actor.defs#profileViewDetailed>;
        rdfs:range   <https://atproto.social/ontology/app.bsky.actor.defs#viewerState> .

<https://atproto.social/ontology/app.bsky.actor.defs#profileViewDetailed/handle>
        a            owl:DatatypeProperty;
        rdfs:domain  <https://atproto.social/ontology/app.bsky.actor.defs#profileViewDetailed>;
        rdfs:range   <xsd:string> .

<https://atproto.social/ontology/app.bsky.actor.defs#profileViewDetailed/followsCount>
        a            owl:DatatypeProperty;
        rdfs:domain  <https://atproto.social/ontology/app.bsky.actor.defs#profileViewDetailed>;
        rdfs:range   <xsd:integer> .

<https://atproto.social/ontology/app.bsky.actor.defs#profileViewDetailed/postsCount>
        a            owl:DatatypeProperty;
        rdfs:domain  <https://atproto.social/ontology/app.bsky.actor.defs#profileViewDetailed>;
        rdfs:range   <xsd:integer> .

<https://atproto.social/ontology/app.bsky.actor.defs#profileViewDetailed/associated>
        a            owl:ObjectProperty;
        rdfs:domain  <https://atproto.social/ontology/app.bsky.actor.defs#profileViewDetailed>;
        rdfs:range   <https://atproto.social/ontology/app.bsky.actor.defs#profileAssociated> .

<https://atproto.social/ontology/app.bsky.actor.defs#profileViewDetailed/indexedAt>
        a            owl:DatatypeProperty;
        rdfs:domain  <https://atproto.social/ontology/app.bsky.actor.defs#profileViewDetailed>;
        rdfs:range   <xsd:string> .

<https://atproto.social/ontology/app.bsky.actor.defs#profileViewDetailed/createdAt>
        a            owl:DatatypeProperty;
        rdfs:domain  <https://atproto.social/ontology/app.bsky.actor.defs#profileViewDetailed>;
        rdfs:range   <xsd:string> .

<https://atproto.social/ontology/app.bsky.actor.defs#profileViewDetailed/displayName>
        a            owl:DatatypeProperty;
        rdfs:domain  <https://atproto.social/ontology/app.bsky.actor.defs#profileViewDetailed>;
        rdfs:range   <xsd:string> .

<https://atproto.social/ontology/app.bsky.actor.defs#profileViewDetailed/banner>
        a            owl:DatatypeProperty;
        rdfs:domain  <https://atproto.social/ontology/app.bsky.actor.defs#profileViewDetailed>;
        rdfs:range   <xsd:string> .

<https://atproto.social/ontology/app.bsky.actor.defs#profileViewDetailed/description>
        a            owl:DatatypeProperty;
        rdfs:domain  <https://atproto.social/ontology/app.bsky.actor.defs#profileViewDetailed>;
        rdfs:range   <xsd:string> .

<https://atproto.social/ontology/app.bsky.actor.defs#profileViewDetailed/followersCount>
        a            owl:DatatypeProperty;
        rdfs:domain  <https://atproto.social/ontology/app.bsky.actor.defs#profileViewDetailed>;
        rdfs:range   <xsd:integer> .

<https://atproto.social/ontology/app.bsky.actor.defs#profileViewDetailed/labels>
        a            owl:ObjectProperty;
        rdfs:domain  <https://atproto.social/ontology/app.bsky.actor.defs#profileViewDetailed>;
        rdfs:range   <https://atproto.social/ontology/com.atproto.label.defs#label> .

<https://atproto.social/ontology/app.bsky.actor.defs#profileViewDetailed/status>
        a            owl:ObjectProperty;
        rdfs:domain  <https://atproto.social/ontology/app.bsky.actor.defs#profileViewDetailed>;
        rdfs:range   <https://atproto.social/ontology/app.bsky.actor.defs#statusView> .

<https://atproto.social/ontology/app.bsky.actor.defs#profileViewDetailed/did>
        a            owl:DatatypeProperty;
        rdfs:domain  <https://atproto.social/ontology/app.bsky.actor.defs#profileViewDetailed>;
        rdfs:range   <xsd:string> .

<https://atproto.social/ontology/app.bsky.actor.defs#profileViewDetailed/avatar>
        a            owl:DatatypeProperty;
        rdfs:domain  <https://atproto.social/ontology/app.bsky.actor.defs#profileViewDetailed>;
        rdfs:range   <xsd:string> .

<https://atproto.social/ontology/app.bsky.actor.defs#profileViewDetailed/joinedViaStarterPack>
        a            owl:ObjectProperty;
        rdfs:domain  <https://atproto.social/ontology/app.bsky.actor.defs#profileViewDetailed>;
        rdfs:range   <https://atproto.social/ontology/app.bsky.graph.defs#starterPackViewBasic> .

<https://atproto.social/ontology/app.bsky.actor.defs#profileViewDetailed/pinnedPost>
        a            owl:ObjectProperty;
        rdfs:domain  <https://atproto.social/ontology/app.bsky.actor.defs#profileViewDetailed>;
        rdfs:range   <https://atproto.social/ontology/app.bsky.actor.defs#com.atproto.repo.strongRef> .

<https://atproto.social/ontology/app.bsky.actor.defs#savedFeedsPrefV2>
        a       owl:Class .

<https://atproto.social/ontology/app.bsky.actor.defs#savedFeedsPrefV2/items>
        a            owl:ObjectProperty;
        rdfs:domain  <https://atproto.social/ontology/app.bsky.actor.defs#savedFeedsPrefV2>;
        rdfs:range   <https://atproto.social/ontology/app.bsky.actor.defs#savedFeed> .

<https://atproto.social/ontology/app.bsky.actor.defs#savedFeedsPref>
        a       owl:Class .

<https://atproto.social/ontology/app.bsky.actor.defs#savedFeedsPref/saved>
        a            owl:DatatypeProperty;
        rdfs:domain  <https://atproto.social/ontology/app.bsky.actor.defs#savedFeedsPref>;
        rdfs:range   <xsd:string> .

<https://atproto.social/ontology/app.bsky.actor.defs#savedFeedsPref/timelineIndex>
        a            owl:DatatypeProperty;
        rdfs:domain  <https://atproto.social/ontology/app.bsky.actor.defs#savedFeedsPref>;
        rdfs:range   <xsd:integer> .

<https://atproto.social/ontology/app.bsky.actor.defs#savedFeedsPref/pinned>
        a            owl:DatatypeProperty;
        rdfs:domain  <https://atproto.social/ontology/app.bsky.actor.defs#savedFeedsPref>;
        rdfs:range   <xsd:string> .

<https://atproto.social/ontology/app.bsky.actor.defs#mutedWordsPref>
        a       owl:Class .

<https://atproto.social/ontology/app.bsky.actor.defs#mutedWordsPref/items>
        a             owl:ObjectProperty;
        rdfs:domain   <https://atproto.social/ontology/app.bsky.actor.defs#mutedWordsPref>;
        rdfs:range    <https://atproto.social/ontology/app.bsky.actor.defs#mutedWord>;
        rdfs:comment  "A list of words the account owner has muted." .

<https://atproto.social/ontology/app.bsky.actor.defs#hiddenPostsPref>
        a       owl:Class .

<https://atproto.social/ontology/app.bsky.actor.defs#hiddenPostsPref/items>
        a             owl:DatatypeProperty;
        rdfs:domain   <https://atproto.social/ontology/app.bsky.actor.defs#hiddenPostsPref>;
        rdfs:range    <xsd:string>;
        rdfs:comment  "A list of URIs of posts the account owner has hidden." .

<https://atproto.social/ontology/app.bsky.actor.defs#profileAssociatedChat>
        a       owl:Class .

<https://atproto.social/ontology/app.bsky.actor.defs#profileAssociatedChat/allowIncoming>
        a            owl:DatatypeProperty;
        rdfs:domain  <https://atproto.social/ontology/app.bsky.actor.defs#profileAssociatedChat>;
        rdfs:range   <xsd:string> .

<https://atproto.social/ontology/app.bsky.actor.defs#viewerState>
        a             owl:Class;
        rdfs:comment  "Metadata about the requesting account's relationship with the subject account. Only has meaningful content for authed requests." .

<https://atproto.social/ontology/app.bsky.actor.defs#viewerState/knownFollowers>
        a            owl:ObjectProperty;
        rdfs:domain  <https://atproto.social/ontology/app.bsky.actor.defs#viewerState>;
        rdfs:range   <https://atproto.social/ontology/app.bsky.actor.defs#knownFollowers> .

<https://atproto.social/ontology/app.bsky.actor.defs#viewerState/activitySubscription>
        a            owl:ObjectProperty;
        rdfs:domain  <https://atproto.social/ontology/app.bsky.actor.defs#viewerState>;
        rdfs:range   <https://atproto.social/ontology/app.bsky.notification.defs#activitySubscription> .

<https://atproto.social/ontology/app.bsky.actor.defs#viewerState/muted>
        a            owl:DatatypeProperty;
        rdfs:domain  <https://atproto.social/ontology/app.bsky.actor.defs#viewerState>;
        rdfs:range   <xsd:boolean> .

<https://atproto.social/ontology/app.bsky.actor.defs#viewerState/followedBy>
        a            owl:DatatypeProperty;
        rdfs:domain  <https://atproto.social/ontology/app.bsky.actor.defs#viewerState>;
        rdfs:range   <xsd:string> .

<https://atproto.social/ontology/app.bsky.actor.defs#viewerState/mutedByList>
        a            owl:ObjectProperty;
        rdfs:domain  <https://atproto.social/ontology/app.bsky.actor.defs#viewerState>;
        rdfs:range   <https://atproto.social/ontology/app.bsky.graph.defs#listViewBasic> .

<https://atproto.social/ontology/app.bsky.actor.defs#viewerState/blockedBy>
        a            owl:DatatypeProperty;
        rdfs:domain  <https://atproto.social/ontology/app.bsky.actor.defs#viewerState>;
        rdfs:range   <xsd:boolean> .

<https://atproto.social/ontology/app.bsky.actor.defs#viewerState/blocking>
        a            owl:DatatypeProperty;
        rdfs:domain  <https://atproto.social/ontology/app.bsky.actor.defs#viewerState>;
        rdfs:range   <xsd:string> .

<https://atproto.social/ontology/app.bsky.actor.defs#viewerState/blockingByList>
        a            owl:ObjectProperty;
        rdfs:domain  <https://atproto.social/ontology/app.bsky.actor.defs#viewerState>;
        rdfs:range   <https://atproto.social/ontology/app.bsky.graph.defs#listViewBasic> .

<https://atproto.social/ontology/app.bsky.actor.defs#viewerState/following>
        a            owl:DatatypeProperty;
        rdfs:domain  <https://atproto.social/ontology/app.bsky.actor.defs#viewerState>;
        rdfs:range   <xsd:string> .

<https://atproto.social/ontology/app.bsky.actor.defs#adultContentPref>
        a       owl:Class .

<https://atproto.social/ontology/app.bsky.actor.defs#adultContentPref/enabled>
        a            owl:DatatypeProperty;
        rdfs:domain  <https://atproto.social/ontology/app.bsky.actor.defs#adultContentPref>;
        rdfs:range   <xsd:boolean> .

<https://atproto.social/ontology/app.bsky.actor.defs#nux>
        a             owl:Class;
        rdfs:comment  "A new user experiences (NUX) storage object" .

<https://atproto.social/ontology/app.bsky.actor.defs#nux/completed>
        a            owl:DatatypeProperty;
        rdfs:domain  <https://atproto.social/ontology/app.bsky.actor.defs#nux>;
        rdfs:range   <xsd:boolean> .

<https://atproto.social/ontology/app.bsky.actor.defs#nux/data>
        a             owl:DatatypeProperty;
        rdfs:domain   <https://atproto.social/ontology/app.bsky.actor.defs#nux>;
        rdfs:range    <xsd:string>;
        rdfs:comment  "Arbitrary data for the NUX. The structure is defined by the NUX itself. Limited to 300 characters." .

<https://atproto.social/ontology/app.bsky.actor.defs#nux/expiresAt>
        a             owl:DatatypeProperty;
        rdfs:domain   <https://atproto.social/ontology/app.bsky.actor.defs#nux>;
        rdfs:range    <xsd:string>;
        rdfs:comment  "The date and time at which the NUX will expire and should be considered completed." .

<https://atproto.social/ontology/app.bsky.actor.defs#nux/id>
        a            owl:DatatypeProperty;
        rdfs:domain  <https://atproto.social/ontology/app.bsky.actor.defs#nux>;
        rdfs:range   <xsd:string> .

<https://atproto.social/ontology/app.bsky.actor.getPreferences#main>
        a             owl:Class;
        rdfs:comment  "Get private preferences attached to the current account. Expected use is synchronization between multiple devices, and import/export during account migration. Requires auth." .

<https://atproto.social/ontology/app.bsky.actor.getProfile#main>
        a             owl:Class;
        rdfs:comment  "Get detailed profile view of an actor. Does not require auth, but contains relevant metadata with auth." .

<https://atproto.social/ontology/app.bsky.actor.getProfiles#main>
        a             owl:Class;
        rdfs:comment  "Get detailed profile views of multiple actors." .

<https://atproto.social/ontology/app.bsky.actor.getSuggestions#main>
        a             owl:Class;
        rdfs:comment  "Get a list of suggested actors. Expected use is discovery of accounts to follow during new account onboarding." .

<https://atproto.social/ontology/app.bsky.actor.profile#main>
        a             owl:Class;
        rdfs:comment  "A declaration of a Bluesky account profile." .

<https://atproto.social/ontology/app.bsky.actor.putPreferences#main>
        a             owl:Class;
        rdfs:comment  "Set the private preferences attached to the account." .

<https://atproto.social/ontology/app.bsky.actor.searchActors#main>
        a             owl:Class;
        rdfs:comment  "Find actors (profiles) matching search criteria. Does not require auth." .

<https://atproto.social/ontology/app.bsky.actor.searchActorsTypeahead#main>
        a             owl:Class;
        rdfs:comment  "Find actor suggestions for a prefix search term. Expected use is for auto-completion during text field entry. Does not require auth." .

<https://atproto.social/ontology/app.bsky.actor.status#main>
        a             owl:Class;
        rdfs:comment  "A declaration of a Bluesky account status." .

<https://atproto.social/ontology/app.bsky.actor.status#live>
        a             owl:Class;
        rdfs:comment  "Advertises an account as currently offering live content." .

<https://atproto.social/ontology/app.bsky.embed.defs#aspectRatio>
        a             owl:Class;
        rdfs:comment  "width:height represents an aspect ratio. It may be approximate, and may not correspond to absolute dimensions in any given unit." .

<https://atproto.social/ontology/app.bsky.embed.defs#aspectRatio/width>
        a            owl:DatatypeProperty;
        rdfs:domain  <https://atproto.social/ontology/app.bsky.embed.defs#aspectRatio>;
        rdfs:range   <xsd:integer> .

<https://atproto.social/ontology/app.bsky.embed.defs#aspectRatio/height>
        a            owl:DatatypeProperty;
        rdfs:domain  <https://atproto.social/ontology/app.bsky.embed.defs#aspectRatio>;
        rdfs:range   <xsd:integer> .

<https://atproto.social/ontology/app.bsky.embed.external#view>
        a       owl:Class .

<https://atproto.social/ontology/app.bsky.embed.external#view/external>
        a            owl:ObjectProperty;
        rdfs:domain  <https://atproto.social/ontology/app.bsky.embed.external#view>;
        rdfs:range   <https://atproto.social/ontology/app.bsky.embed.external#viewExternal> .

<https://atproto.social/ontology/app.bsky.embed.external#viewExternal>
        a       owl:Class .

<https://atproto.social/ontology/app.bsky.embed.external#viewExternal/thumb>
        a            owl:DatatypeProperty;
        rdfs:domain  <https://atproto.social/ontology/app.bsky.embed.external#viewExternal>;
        rdfs:range   <xsd:string> .

<https://atproto.social/ontology/app.bsky.embed.external#viewExternal/uri>
        a            owl:DatatypeProperty;
        rdfs:domain  <https://atproto.social/ontology/app.bsky.embed.external#viewExternal>;
        rdfs:range   <xsd:string> .

<https://atproto.social/ontology/app.bsky.embed.external#viewExternal/title>
        a            owl:DatatypeProperty;
        rdfs:domain  <https://atproto.social/ontology/app.bsky.embed.external#viewExternal>;
        rdfs:range   <xsd:string> .

<https://atproto.social/ontology/app.bsky.embed.external#viewExternal/description>
        a            owl:DatatypeProperty;
        rdfs:domain  <https://atproto.social/ontology/app.bsky.embed.external#viewExternal>;
        rdfs:range   <xsd:string> .

<https://atproto.social/ontology/app.bsky.embed.external#main>
        a             owl:Class;
        rdfs:comment  "A representation of some externally linked content (eg, a URL and 'card'), embedded in a Bluesky record (eg, a post)." .

<https://atproto.social/ontology/app.bsky.embed.external#main/external>
        a            owl:ObjectProperty;
        rdfs:domain  <https://atproto.social/ontology/app.bsky.embed.external#main>;
        rdfs:range   <https://atproto.social/ontology/app.bsky.embed.external#external> .

<https://atproto.social/ontology/app.bsky.embed.external#external>
        a       owl:Class .

<https://atproto.social/ontology/app.bsky.embed.external#external/uri>
        a            owl:DatatypeProperty;
        rdfs:domain  <https://atproto.social/ontology/app.bsky.embed.external#external>;
        rdfs:range   <xsd:string> .

<https://atproto.social/ontology/app.bsky.embed.external#external/title>
        a            owl:DatatypeProperty;
        rdfs:domain  <https://atproto.social/ontology/app.bsky.embed.external#external>;
        rdfs:range   <xsd:string> .

<https://atproto.social/ontology/app.bsky.embed.external#external/description>
        a            owl:DatatypeProperty;
        rdfs:domain  <https://atproto.social/ontology/app.bsky.embed.external#external>;
        rdfs:range   <xsd:string> .

<https://atproto.social/ontology/app.bsky.embed.external#external/thumb>
        a            owl:ObjectProperty;
        rdfs:domain  <https://atproto.social/ontology/app.bsky.embed.external#external> .

<https://atproto.social/ontology/app.bsky.embed.images#main>
        a       owl:Class .

<https://atproto.social/ontology/app.bsky.embed.images#main/images>
        a            owl:ObjectProperty;
        rdfs:domain  <https://atproto.social/ontology/app.bsky.embed.images#main>;
        rdfs:range   <https://atproto.social/ontology/app.bsky.embed.images#image> .

<https://atproto.social/ontology/app.bsky.embed.images#image>
        a       owl:Class .

<https://atproto.social/ontology/app.bsky.embed.images#image/image>
        a            owl:ObjectProperty;
        rdfs:domain  <https://atproto.social/ontology/app.bsky.embed.images#image> .

<https://atproto.social/ontology/app.bsky.embed.images#image/alt>
        a             owl:DatatypeProperty;
        rdfs:domain   <https://atproto.social/ontology/app.bsky.embed.images#image>;
        rdfs:range    <xsd:string>;
        rdfs:comment  "Alt text description of the image, for accessibility." .

<https://atproto.social/ontology/app.bsky.embed.images#image/aspectRatio>
        a            owl:ObjectProperty;
        rdfs:domain  <https://atproto.social/ontology/app.bsky.embed.images#image>;
        rdfs:range   <https://atproto.social/ontology/app.bsky.embed.defs#aspectRatio> .

<https://atproto.social/ontology/app.bsky.embed.images#view>
        a       owl:Class .

<https://atproto.social/ontology/app.bsky.embed.images#view/images>
        a            owl:ObjectProperty;
        rdfs:domain  <https://atproto.social/ontology/app.bsky.embed.images#view>;
        rdfs:range   <https://atproto.social/ontology/app.bsky.embed.images#viewImage> .

<https://atproto.social/ontology/app.bsky.embed.images#viewImage>
        a       owl:Class .

<https://atproto.social/ontology/app.bsky.embed.images#viewImage/thumb>
        a             owl:DatatypeProperty;
        rdfs:domain   <https://atproto.social/ontology/app.bsky.embed.images#viewImage>;
        rdfs:range    <xsd:string>;
        rdfs:comment  "Fully-qualified URL where a thumbnail of the image can be fetched. For example, CDN location provided by the App View." .

<https://atproto.social/ontology/app.bsky.embed.images#viewImage/fullsize>
        a             owl:DatatypeProperty;
        rdfs:domain   <https://atproto.social/ontology/app.bsky.embed.images#viewImage>;
        rdfs:range    <xsd:string>;
        rdfs:comment  "Fully-qualified URL where a large version of the image can be fetched. May or may not be the exact original blob. For example, CDN location provided by the App View." .

<https://atproto.social/ontology/app.bsky.embed.images#viewImage/alt>
        a             owl:DatatypeProperty;
        rdfs:domain   <https://atproto.social/ontology/app.bsky.embed.images#viewImage>;
        rdfs:range    <xsd:string>;
        rdfs:comment  "Alt text description of the image, for accessibility." .

<https://atproto.social/ontology/app.bsky.embed.images#viewImage/aspectRatio>
        a            owl:ObjectProperty;
        rdfs:domain  <https://atproto.social/ontology/app.bsky.embed.images#viewImage>;
        rdfs:range   <https://atproto.social/ontology/app.bsky.embed.defs#aspectRatio> .

<https://atproto.social/ontology/app.bsky.embed.record#main>
        a       owl:Class .

<https://atproto.social/ontology/app.bsky.embed.record#main/record>
        a            owl:ObjectProperty;
        rdfs:domain  <https://atproto.social/ontology/app.bsky.embed.record#main>;
        rdfs:range   <https://atproto.social/ontology/app.bsky.embed.record#com.atproto.repo.strongRef> .

<https://atproto.social/ontology/app.bsky.embed.record#view>
        a       owl:Class .

<https://atproto.social/ontology/app.bsky.embed.record#view/record>
        a            owl:ObjectProperty;
        rdfs:domain  <https://atproto.social/ontology/app.bsky.embed.record#view> .

<https://atproto.social/ontology/app.bsky.embed.record#viewRecord>
        a       owl:Class .

<https://atproto.social/ontology/app.bsky.embed.record#viewRecord/uri>
        a            owl:DatatypeProperty;
        rdfs:domain  <https://atproto.social/ontology/app.bsky.embed.record#viewRecord>;
        rdfs:range   <xsd:string> .

<https://atproto.social/ontology/app.bsky.embed.record#viewRecord/cid>
        a            owl:DatatypeProperty;
        rdfs:domain  <https://atproto.social/ontology/app.bsky.embed.record#viewRecord>;
        rdfs:range   <xsd:string> .

<https://atproto.social/ontology/app.bsky.embed.record#viewRecord/author>
        a            owl:ObjectProperty;
        rdfs:domain  <https://atproto.social/ontology/app.bsky.embed.record#viewRecord>;
        rdfs:range   <https://atproto.social/ontology/app.bsky.actor.defs#profileViewBasic> .

<https://atproto.social/ontology/app.bsky.embed.record#viewRecord/value>
        a             owl:ObjectProperty;
        rdfs:domain   <https://atproto.social/ontology/app.bsky.embed.record#viewRecord>;
        rdfs:comment  "The record data itself." .

<https://atproto.social/ontology/app.bsky.embed.record#viewRecord/labels>
        a            owl:ObjectProperty;
        rdfs:domain  <https://atproto.social/ontology/app.bsky.embed.record#viewRecord>;
        rdfs:range   <https://atproto.social/ontology/com.atproto.label.defs#label> .

<https://atproto.social/ontology/app.bsky.embed.record#viewRecord/replyCount>
        a            owl:DatatypeProperty;
        rdfs:domain  <https://atproto.social/ontology/app.bsky.embed.record#viewRecord>;
        rdfs:range   <xsd:integer> .

<https://atproto.social/ontology/app.bsky.embed.record#viewRecord/repostCount>
        a            owl:DatatypeProperty;
        rdfs:domain  <https://atproto.social/ontology/app.bsky.embed.record#viewRecord>;
        rdfs:range   <xsd:integer> .

<https://atproto.social/ontology/app.bsky.embed.record#viewRecord/likeCount>
        a            owl:DatatypeProperty;
        rdfs:domain  <https://atproto.social/ontology/app.bsky.embed.record#viewRecord>;
        rdfs:range   <xsd:integer> .

<https://atproto.social/ontology/app.bsky.embed.record#viewRecord/quoteCount>
        a            owl:DatatypeProperty;
        rdfs:domain  <https://atproto.social/ontology/app.bsky.embed.record#viewRecord>;
        rdfs:range   <xsd:integer> .

<https://atproto.social/ontology/app.bsky.embed.record#viewRecord/embeds>
        a            owl:ObjectProperty;
        rdfs:domain  <https://atproto.social/ontology/app.bsky.embed.record#viewRecord> .

<https://atproto.social/ontology/app.bsky.embed.record#viewRecord/indexedAt>
        a            owl:DatatypeProperty;
        rdfs:domain  <https://atproto.social/ontology/app.bsky.embed.record#viewRecord>;
        rdfs:range   <xsd:string> .

<https://atproto.social/ontology/app.bsky.embed.record#viewNotFound>
        a       owl:Class .

<https://atproto.social/ontology/app.bsky.embed.record#viewNotFound/uri>
        a            owl:DatatypeProperty;
        rdfs:domain  <https://atproto.social/ontology/app.bsky.embed.record#viewNotFound>;
        rdfs:range   <xsd:string> .

<https://atproto.social/ontology/app.bsky.embed.record#viewNotFound/notFound>
        a            owl:DatatypeProperty;
        rdfs:domain  <https://atproto.social/ontology/app.bsky.embed.record#viewNotFound>;
        rdfs:range   <xsd:boolean> .

<https://atproto.social/ontology/app.bsky.embed.record#viewBlocked>
        a       owl:Class .

<https://atproto.social/ontology/app.bsky.embed.record#viewBlocked/uri>
        a            owl:DatatypeProperty;
        rdfs:domain  <https://atproto.social/ontology/app.bsky.embed.record#viewBlocked>;
        rdfs:range   <xsd:string> .

<https://atproto.social/ontology/app.bsky.embed.record#viewBlocked/blocked>
        a            owl:DatatypeProperty;
        rdfs:domain  <https://atproto.social/ontology/app.bsky.embed.record#viewBlocked>;
        rdfs:range   <xsd:boolean> .

<https://atproto.social/ontology/app.bsky.embed.record#viewBlocked/author>
        a            owl:ObjectProperty;
        rdfs:domain  <https://atproto.social/ontology/app.bsky.embed.record#viewBlocked>;
        rdfs:range   <https://atproto.social/ontology/app.bsky.feed.defs#blockedAuthor> .

<https://atproto.social/ontology/app.bsky.embed.record#viewDetached>
        a       owl:Class .

<https://atproto.social/ontology/app.bsky.embed.record#viewDetached/detached>
        a            owl:DatatypeProperty;
        rdfs:domain  <https://atproto.social/ontology/app.bsky.embed.record#viewDetached>;
        rdfs:range   <xsd:boolean> .

<https://atproto.social/ontology/app.bsky.embed.record#viewDetached/uri>
        a            owl:DatatypeProperty;
        rdfs:domain  <https://atproto.social/ontology/app.bsky.embed.record#viewDetached>;
        rdfs:range   <xsd:string> .

<https://atproto.social/ontology/app.bsky.embed.recordWithMedia#view>
        a       owl:Class .

<https://atproto.social/ontology/app.bsky.embed.recordWithMedia#view/record>
        a            owl:ObjectProperty;
        rdfs:domain  <https://atproto.social/ontology/app.bsky.embed.recordWithMedia#view>;
        rdfs:range   <https://atproto.social/ontology/app.bsky.embed.record#view> .

<https://atproto.social/ontology/app.bsky.embed.recordWithMedia#view/media>
        a            owl:ObjectProperty;
        rdfs:domain  <https://atproto.social/ontology/app.bsky.embed.recordWithMedia#view> .

<https://atproto.social/ontology/app.bsky.embed.recordWithMedia#main>
        a       owl:Class .

<https://atproto.social/ontology/app.bsky.embed.recordWithMedia#main/record>
        a            owl:ObjectProperty;
        rdfs:domain  <https://atproto.social/ontology/app.bsky.embed.recordWithMedia#main>;
        rdfs:range   <https://atproto.social/ontology/app.bsky.embed.recordWithMedia#app.bsky.embed.record> .

<https://atproto.social/ontology/app.bsky.embed.recordWithMedia#main/media>
        a            owl:ObjectProperty;
        rdfs:domain  <https://atproto.social/ontology/app.bsky.embed.recordWithMedia#main> .

<https://atproto.social/ontology/app.bsky.embed.video#main>
        a       owl:Class .

<https://atproto.social/ontology/app.bsky.embed.video#main/video>
        a             owl:ObjectProperty;
        rdfs:domain   <https://atproto.social/ontology/app.bsky.embed.video#main>;
        rdfs:comment  "The mp4 video file. May be up to 100mb, formerly limited to 50mb." .

<https://atproto.social/ontology/app.bsky.embed.video#main/captions>
        a            owl:ObjectProperty;
        rdfs:domain  <https://atproto.social/ontology/app.bsky.embed.video#main>;
        rdfs:range   <https://atproto.social/ontology/app.bsky.embed.video#caption> .

<https://atproto.social/ontology/app.bsky.embed.video#main/alt>
        a             owl:DatatypeProperty;
        rdfs:domain   <https://atproto.social/ontology/app.bsky.embed.video#main>;
        rdfs:range    <xsd:string>;
        rdfs:comment  "Alt text description of the video, for accessibility." .

<https://atproto.social/ontology/app.bsky.embed.video#main/aspectRatio>
        a            owl:ObjectProperty;
        rdfs:domain  <https://atproto.social/ontology/app.bsky.embed.video#main>;
        rdfs:range   <https://atproto.social/ontology/app.bsky.embed.defs#aspectRatio> .

<https://atproto.social/ontology/app.bsky.embed.video#caption>
        a       owl:Class .

<https://atproto.social/ontology/app.bsky.embed.video#caption/lang>
        a            owl:DatatypeProperty;
        rdfs:domain  <https://atproto.social/ontology/app.bsky.embed.video#caption>;
        rdfs:range   <xsd:string> .

<https://atproto.social/ontology/app.bsky.embed.video#caption/file>
        a            owl:ObjectProperty;
        rdfs:domain  <https://atproto.social/ontology/app.bsky.embed.video#caption> .

<https://atproto.social/ontology/app.bsky.embed.video#view>
        a       owl:Class .

<https://atproto.social/ontology/app.bsky.embed.video#view/cid>
        a            owl:DatatypeProperty;
        rdfs:domain  <https://atproto.social/ontology/app.bsky.embed.video#view>;
        rdfs:range   <xsd:string> .

<https://atproto.social/ontology/app.bsky.embed.video#view/playlist>
        a            owl:DatatypeProperty;
        rdfs:domain  <https://atproto.social/ontology/app.bsky.embed.video#view>;
        rdfs:range   <xsd:string> .

<https://atproto.social/ontology/app.bsky.embed.video#view/thumbnail>
        a            owl:DatatypeProperty;
        rdfs:domain  <https://atproto.social/ontology/app.bsky.embed.video#view>;
        rdfs:range   <xsd:string> .

<https://atproto.social/ontology/app.bsky.embed.video#view/alt>
        a            owl:DatatypeProperty;
        rdfs:domain  <https://atproto.social/ontology/app.bsky.embed.video#view>;
        rdfs:range   <xsd:string> .

<https://atproto.social/ontology/app.bsky.embed.video#view/aspectRatio>
        a            owl:ObjectProperty;
        rdfs:domain  <https://atproto.social/ontology/app.bsky.embed.video#view>;
        rdfs:range   <https://atproto.social/ontology/app.bsky.embed.defs#aspectRatio> .

<https://atproto.social/ontology/app.bsky.feed.defs#postView>
        a       owl:Class .

<https://atproto.social/ontology/app.bsky.feed.defs#postView/indexedAt>
        a            owl:DatatypeProperty;
        rdfs:domain  <https://atproto.social/ontology/app.bsky.feed.defs#postView>;
        rdfs:range   <xsd:string> .

<https://atproto.social/ontology/app.bsky.feed.defs#postView/viewer>
        a            owl:ObjectProperty;
        rdfs:domain  <https://atproto.social/ontology/app.bsky.feed.defs#postView>;
        rdfs:range   <https://atproto.social/ontology/app.bsky.feed.defs#viewerState> .

<https://atproto.social/ontology/app.bsky.feed.defs#postView/uri>
        a            owl:DatatypeProperty;
        rdfs:domain  <https://atproto.social/ontology/app.bsky.feed.defs#postView>;
        rdfs:range   <xsd:string> .

<https://atproto.social/ontology/app.bsky.feed.defs#postView/record>
        a            owl:ObjectProperty;
        rdfs:domain  <https://atproto.social/ontology/app.bsky.feed.defs#postView> .

<https://atproto.social/ontology/app.bsky.feed.defs#postView/replyCount>
        a            owl:DatatypeProperty;
        rdfs:domain  <https://atproto.social/ontology/app.bsky.feed.defs#postView>;
        rdfs:range   <xsd:integer> .

<https://atproto.social/ontology/app.bsky.feed.defs#postView/labels>
        a            owl:ObjectProperty;
        rdfs:domain  <https://atproto.social/ontology/app.bsky.feed.defs#postView>;
        rdfs:range   <https://atproto.social/ontology/com.atproto.label.defs#label> .

<https://atproto.social/ontology/app.bsky.feed.defs#postView/threadgate>
        a            owl:ObjectProperty;
        rdfs:domain  <https://atproto.social/ontology/app.bsky.feed.defs#postView>;
        rdfs:range   <https://atproto.social/ontology/app.bsky.feed.defs#threadgateView> .

<https://atproto.social/ontology/app.bsky.feed.defs#postView/cid>
        a            owl:DatatypeProperty;
        rdfs:domain  <https://atproto.social/ontology/app.bsky.feed.defs#postView>;
        rdfs:range   <xsd:string> .

<https://atproto.social/ontology/app.bsky.feed.defs#postView/author>
        a            owl:ObjectProperty;
        rdfs:domain  <https://atproto.social/ontology/app.bsky.feed.defs#postView>;
        rdfs:range   <https://atproto.social/ontology/app.bsky.actor.defs#profileViewBasic> .

<https://atproto.social/ontology/app.bsky.feed.defs#postView/embed>
        a            owl:ObjectProperty;
        rdfs:domain  <https://atproto.social/ontology/app.bsky.feed.defs#postView> .

<https://atproto.social/ontology/app.bsky.feed.defs#postView/repostCount>
        a            owl:DatatypeProperty;
        rdfs:domain  <https://atproto.social/ontology/app.bsky.feed.defs#postView>;
        rdfs:range   <xsd:integer> .

<https://atproto.social/ontology/app.bsky.feed.defs#postView/likeCount>
        a            owl:DatatypeProperty;
        rdfs:domain  <https://atproto.social/ontology/app.bsky.feed.defs#postView>;
        rdfs:range   <xsd:integer> .

<https://atproto.social/ontology/app.bsky.feed.defs#postView/quoteCount>
        a            owl:DatatypeProperty;
        rdfs:domain  <https://atproto.social/ontology/app.bsky.feed.defs#postView>;
        rdfs:range   <xsd:integer> .

<https://atproto.social/ontology/app.bsky.feed.defs#clickthroughAuthor>
        a             owl:Class;
        rdfs:comment  "User clicked through to the author of the feed item" .

<https://atproto.social/ontology/app.bsky.feed.defs#interactionLike>
        a             owl:Class;
        rdfs:comment  "User liked the feed item" .

<https://atproto.social/ontology/app.bsky.feed.defs#feedViewPost>
        a       owl:Class .

<https://atproto.social/ontology/app.bsky.feed.defs#feedViewPost/post>
        a            owl:ObjectProperty;
        rdfs:domain  <https://atproto.social/ontology/app.bsky.feed.defs#feedViewPost>;
        rdfs:range   <https://atproto.social/ontology/app.bsky.feed.defs#postView> .

<https://atproto.social/ontology/app.bsky.feed.defs#feedViewPost/reply>
        a            owl:ObjectProperty;
        rdfs:domain  <https://atproto.social/ontology/app.bsky.feed.defs#feedViewPost>;
        rdfs:range   <https://atproto.social/ontology/app.bsky.feed.defs#replyRef> .

<https://atproto.social/ontology/app.bsky.feed.defs#feedViewPost/reason>
        a            owl:ObjectProperty;
        rdfs:domain  <https://atproto.social/ontology/app.bsky.feed.defs#feedViewPost> .

<https://atproto.social/ontology/app.bsky.feed.defs#feedViewPost/feedContext>
        a             owl:DatatypeProperty;
        rdfs:domain   <https://atproto.social/ontology/app.bsky.feed.defs#feedViewPost>;
        rdfs:range    <xsd:string>;
        rdfs:comment  "Context provided by feed generator that may be passed back alongside interactions." .

<https://atproto.social/ontology/app.bsky.feed.defs#feedViewPost/reqId>
        a             owl:DatatypeProperty;
        rdfs:domain   <https://atproto.social/ontology/app.bsky.feed.defs#feedViewPost>;
        rdfs:range    <xsd:string>;
        rdfs:comment  "Unique identifier per request that may be passed back alongside interactions." .

<https://atproto.social/ontology/app.bsky.feed.defs#clickthroughReposter>
        a             owl:Class;
        rdfs:comment  "User clicked through to the reposter of the feed item" .

<https://atproto.social/ontology/app.bsky.feed.defs#reasonRepost>
        a       owl:Class .

<https://atproto.social/ontology/app.bsky.feed.defs#reasonRepost/by>
        a            owl:ObjectProperty;
        rdfs:domain  <https://atproto.social/ontology/app.bsky.feed.defs#reasonRepost>;
        rdfs:range   <https://atproto.social/ontology/app.bsky.actor.defs#profileViewBasic> .

<https://atproto.social/ontology/app.bsky.feed.defs#reasonRepost/uri>
        a            owl:DatatypeProperty;
        rdfs:domain  <https://atproto.social/ontology/app.bsky.feed.defs#reasonRepost>;
        rdfs:range   <xsd:string> .

<https://atproto.social/ontology/app.bsky.feed.defs#reasonRepost/cid>
        a            owl:DatatypeProperty;
        rdfs:domain  <https://atproto.social/ontology/app.bsky.feed.defs#reasonRepost>;
        rdfs:range   <xsd:string> .

<https://atproto.social/ontology/app.bsky.feed.defs#reasonRepost/indexedAt>
        a            owl:DatatypeProperty;
        rdfs:domain  <https://atproto.social/ontology/app.bsky.feed.defs#reasonRepost>;
        rdfs:range   <xsd:string> .

<https://atproto.social/ontology/app.bsky.feed.defs#blockedPost>
        a       owl:Class .

<https://atproto.social/ontology/app.bsky.feed.defs#blockedPost/author>
        a            owl:ObjectProperty;
        rdfs:domain  <https://atproto.social/ontology/app.bsky.feed.defs#blockedPost>;
        rdfs:range   <https://atproto.social/ontology/app.bsky.feed.defs#blockedAuthor> .

<https://atproto.social/ontology/app.bsky.feed.defs#blockedPost/uri>
        a            owl:DatatypeProperty;
        rdfs:domain  <https://atproto.social/ontology/app.bsky.feed.defs#blockedPost>;
        rdfs:range   <xsd:string> .

<https://atproto.social/ontology/app.bsky.feed.defs#blockedPost/blocked>
        a            owl:DatatypeProperty;
        rdfs:domain  <https://atproto.social/ontology/app.bsky.feed.defs#blockedPost>;
        rdfs:range   <xsd:boolean> .

<https://atproto.social/ontology/app.bsky.feed.defs#threadgateView>
        a       owl:Class .

<https://atproto.social/ontology/app.bsky.feed.defs#threadgateView/cid>
        a            owl:DatatypeProperty;
        rdfs:domain  <https://atproto.social/ontology/app.bsky.feed.defs#threadgateView>;
        rdfs:range   <xsd:string> .

<https://atproto.social/ontology/app.bsky.feed.defs#threadgateView/record>
        a            owl:ObjectProperty;
        rdfs:domain  <https://atproto.social/ontology/app.bsky.feed.defs#threadgateView> .

<https://atproto.social/ontology/app.bsky.feed.defs#threadgateView/lists>
        a            owl:ObjectProperty;
        rdfs:domain  <https://atproto.social/ontology/app.bsky.feed.defs#threadgateView>;
        rdfs:range   <https://atproto.social/ontology/app.bsky.graph.defs#listViewBasic> .

<https://atproto.social/ontology/app.bsky.feed.defs#threadgateView/uri>
        a            owl:DatatypeProperty;
        rdfs:domain  <https://atproto.social/ontology/app.bsky.feed.defs#threadgateView>;
        rdfs:range   <xsd:string> .

<https://atproto.social/ontology/app.bsky.feed.defs#clickthroughItem>
        a             owl:Class;
        rdfs:comment  "User clicked through to the feed item" .

<https://atproto.social/ontology/app.bsky.feed.defs#contentModeVideo>
        a             owl:Class;
        rdfs:comment  "Declares the feed generator returns posts containing app.bsky.embed.video embeds." .

<https://atproto.social/ontology/app.bsky.feed.defs#interactionReply>
        a             owl:Class;
        rdfs:comment  "User replied to the feed item" .

<https://atproto.social/ontology/app.bsky.feed.defs#generatorView>
        a       owl:Class .

<https://atproto.social/ontology/app.bsky.feed.defs#generatorView/uri>
        a            owl:DatatypeProperty;
        rdfs:domain  <https://atproto.social/ontology/app.bsky.feed.defs#generatorView>;
        rdfs:range   <xsd:string> .

<https://atproto.social/ontology/app.bsky.feed.defs#generatorView/cid>
        a            owl:DatatypeProperty;
        rdfs:domain  <https://atproto.social/ontology/app.bsky.feed.defs#generatorView>;
        rdfs:range   <xsd:string> .

<https://atproto.social/ontology/app.bsky.feed.defs#generatorView/displayName>
        a            owl:DatatypeProperty;
        rdfs:domain  <https://atproto.social/ontology/app.bsky.feed.defs#generatorView>;
        rdfs:range   <xsd:string> .

<https://atproto.social/ontology/app.bsky.feed.defs#generatorView/description>
        a            owl:DatatypeProperty;
        rdfs:domain  <https://atproto.social/ontology/app.bsky.feed.defs#generatorView>;
        rdfs:range   <xsd:string> .

<https://atproto.social/ontology/app.bsky.feed.defs#generatorView/avatar>
        a            owl:DatatypeProperty;
        rdfs:domain  <https://atproto.social/ontology/app.bsky.feed.defs#generatorView>;
        rdfs:range   <xsd:string> .

<https://atproto.social/ontology/app.bsky.feed.defs#generatorView/acceptsInteractions>
        a            owl:DatatypeProperty;
        rdfs:domain  <https://atproto.social/ontology/app.bsky.feed.defs#generatorView>;
        rdfs:range   <xsd:boolean> .

<https://atproto.social/ontology/app.bsky.feed.defs#generatorView/labels>
        a            owl:ObjectProperty;
        rdfs:domain  <https://atproto.social/ontology/app.bsky.feed.defs#generatorView>;
        rdfs:range   <https://atproto.social/ontology/com.atproto.label.defs#label> .

<https://atproto.social/ontology/app.bsky.feed.defs#generatorView/indexedAt>
        a            owl:DatatypeProperty;
        rdfs:domain  <https://atproto.social/ontology/app.bsky.feed.defs#generatorView>;
        rdfs:range   <xsd:string> .

<https://atproto.social/ontology/app.bsky.feed.defs#generatorView/did>
        a            owl:DatatypeProperty;
        rdfs:domain  <https://atproto.social/ontology/app.bsky.feed.defs#generatorView>;
        rdfs:range   <xsd:string> .

<https://atproto.social/ontology/app.bsky.feed.defs#generatorView/creator>
        a            owl:ObjectProperty;
        rdfs:domain  <https://atproto.social/ontology/app.bsky.feed.defs#generatorView>;
        rdfs:range   <https://atproto.social/ontology/app.bsky.actor.defs#profileView> .

<https://atproto.social/ontology/app.bsky.feed.defs#generatorView/descriptionFacets>
        a            owl:ObjectProperty;
        rdfs:domain  <https://atproto.social/ontology/app.bsky.feed.defs#generatorView>;
        rdfs:range   <https://atproto.social/ontology/app.bsky.feed.defs#app.bsky.richtext.facet> .

<https://atproto.social/ontology/app.bsky.feed.defs#generatorView/likeCount>
        a            owl:DatatypeProperty;
        rdfs:domain  <https://atproto.social/ontology/app.bsky.feed.defs#generatorView>;
        rdfs:range   <xsd:integer> .

<https://atproto.social/ontology/app.bsky.feed.defs#generatorView/viewer>
        a            owl:ObjectProperty;
        rdfs:domain  <https://atproto.social/ontology/app.bsky.feed.defs#generatorView>;
        rdfs:range   <https://atproto.social/ontology/app.bsky.feed.defs#generatorViewerState> .

<https://atproto.social/ontology/app.bsky.feed.defs#generatorView/contentMode>
        a            owl:DatatypeProperty;
        rdfs:domain  <https://atproto.social/ontology/app.bsky.feed.defs#generatorView>;
        rdfs:range   <xsd:string> .

<https://atproto.social/ontology/app.bsky.feed.defs#skeletonReasonRepost>
        a       owl:Class .

<https://atproto.social/ontology/app.bsky.feed.defs#skeletonReasonRepost/repost>
        a            owl:DatatypeProperty;
        rdfs:domain  <https://atproto.social/ontology/app.bsky.feed.defs#skeletonReasonRepost>;
        rdfs:range   <xsd:string> .

<https://atproto.social/ontology/app.bsky.feed.defs#interaction>
        a       owl:Class .

<https://atproto.social/ontology/app.bsky.feed.defs#interaction/item>
        a            owl:DatatypeProperty;
        rdfs:domain  <https://atproto.social/ontology/app.bsky.feed.defs#interaction>;
        rdfs:range   <xsd:string> .

<https://atproto.social/ontology/app.bsky.feed.defs#interaction/event>
        a            owl:DatatypeProperty;
        rdfs:domain  <https://atproto.social/ontology/app.bsky.feed.defs#interaction>;
        rdfs:range   <xsd:string> .

<https://atproto.social/ontology/app.bsky.feed.defs#interaction/feedContext>
        a             owl:DatatypeProperty;
        rdfs:domain   <https://atproto.social/ontology/app.bsky.feed.defs#interaction>;
        rdfs:range    <xsd:string>;
        rdfs:comment  "Context on a feed item that was originally supplied by the feed generator on getFeedSkeleton." .

<https://atproto.social/ontology/app.bsky.feed.defs#interaction/reqId>
        a             owl:DatatypeProperty;
        rdfs:domain   <https://atproto.social/ontology/app.bsky.feed.defs#interaction>;
        rdfs:range    <xsd:string>;
        rdfs:comment  "Unique identifier per request that may be passed back alongside interactions." .

<https://atproto.social/ontology/app.bsky.feed.defs#requestMore>
        a             owl:Class;
        rdfs:comment  "Request that more content like the given feed item be shown in the feed" .

<https://atproto.social/ontology/app.bsky.feed.defs#contentModeUnspecified>
        a             owl:Class;
        rdfs:comment  "Declares the feed generator returns any types of posts." .

<https://atproto.social/ontology/app.bsky.feed.defs#interactionSeen>
        a             owl:Class;
        rdfs:comment  "Feed item was seen by user" .

<https://atproto.social/ontology/app.bsky.feed.defs#blockedAuthor>
        a       owl:Class .

<https://atproto.social/ontology/app.bsky.feed.defs#blockedAuthor/did>
        a            owl:DatatypeProperty;
        rdfs:domain  <https://atproto.social/ontology/app.bsky.feed.defs#blockedAuthor>;
        rdfs:range   <xsd:string> .

<https://atproto.social/ontology/app.bsky.feed.defs#blockedAuthor/viewer>
        a            owl:ObjectProperty;
        rdfs:domain  <https://atproto.social/ontology/app.bsky.feed.defs#blockedAuthor>;
        rdfs:range   <https://atproto.social/ontology/app.bsky.actor.defs#viewerState> .

<https://atproto.social/ontology/app.bsky.feed.defs#generatorViewerState>
        a       owl:Class .

<https://atproto.social/ontology/app.bsky.feed.defs#generatorViewerState/like>
        a            owl:DatatypeProperty;
        rdfs:domain  <https://atproto.social/ontology/app.bsky.feed.defs#generatorViewerState>;
        rdfs:range   <xsd:string> .

<https://atproto.social/ontology/app.bsky.feed.defs#skeletonFeedPost>
        a       owl:Class .

<https://atproto.social/ontology/app.bsky.feed.defs#skeletonFeedPost/post>
        a            owl:DatatypeProperty;
        rdfs:domain  <https://atproto.social/ontology/app.bsky.feed.defs#skeletonFeedPost>;
        rdfs:range   <xsd:string> .

<https://atproto.social/ontology/app.bsky.feed.defs#skeletonFeedPost/reason>
        a            owl:ObjectProperty;
        rdfs:domain  <https://atproto.social/ontology/app.bsky.feed.defs#skeletonFeedPost> .

<https://atproto.social/ontology/app.bsky.feed.defs#skeletonFeedPost/feedContext>
        a             owl:DatatypeProperty;
        rdfs:domain   <https://atproto.social/ontology/app.bsky.feed.defs#skeletonFeedPost>;
        rdfs:range    <xsd:string>;
        rdfs:comment  "Context that will be passed through to client and may be passed to feed generator back alongside interactions." .

<https://atproto.social/ontology/app.bsky.feed.defs#requestLess>
        a             owl:Class;
        rdfs:comment  "Request that less content like the given feed item be shown in the feed" .

<https://atproto.social/ontology/app.bsky.feed.defs#interactionQuote>
        a             owl:Class;
        rdfs:comment  "User quoted the feed item" .

<https://atproto.social/ontology/app.bsky.feed.defs#replyRef>
        a       owl:Class .

<https://atproto.social/ontology/app.bsky.feed.defs#replyRef/root>
        a            owl:ObjectProperty;
        rdfs:domain  <https://atproto.social/ontology/app.bsky.feed.defs#replyRef> .

<https://atproto.social/ontology/app.bsky.feed.defs#replyRef/parent>
        a            owl:ObjectProperty;
        rdfs:domain  <https://atproto.social/ontology/app.bsky.feed.defs#replyRef> .

<https://atproto.social/ontology/app.bsky.feed.defs#replyRef/grandparentAuthor>
        a             owl:ObjectProperty;
        rdfs:domain   <https://atproto.social/ontology/app.bsky.feed.defs#replyRef>;
        rdfs:range    <https://atproto.social/ontology/app.bsky.actor.defs#profileViewBasic>;
        rdfs:comment  "When parent is a reply to another post, this is the author of that post." .

<https://atproto.social/ontology/app.bsky.feed.defs#interactionRepost>
        a             owl:Class;
        rdfs:comment  "User reposted the feed item" .

<https://atproto.social/ontology/app.bsky.feed.defs#viewerState>
        a             owl:Class;
        rdfs:comment  "Metadata about the requesting account's relationship with the subject content. Only has meaningful content for authed requests." .

<https://atproto.social/ontology/app.bsky.feed.defs#viewerState/pinned>
        a            owl:DatatypeProperty;
        rdfs:domain  <https://atproto.social/ontology/app.bsky.feed.defs#viewerState>;
        rdfs:range   <xsd:boolean> .

<https://atproto.social/ontology/app.bsky.feed.defs#viewerState/repost>
        a            owl:DatatypeProperty;
        rdfs:domain  <https://atproto.social/ontology/app.bsky.feed.defs#viewerState>;
        rdfs:range   <xsd:string> .

<https://atproto.social/ontology/app.bsky.feed.defs#viewerState/like>
        a            owl:DatatypeProperty;
        rdfs:domain  <https://atproto.social/ontology/app.bsky.feed.defs#viewerState>;
        rdfs:range   <xsd:string> .

<https://atproto.social/ontology/app.bsky.feed.defs#viewerState/threadMuted>
        a            owl:DatatypeProperty;
        rdfs:domain  <https://atproto.social/ontology/app.bsky.feed.defs#viewerState>;
        rdfs:range   <xsd:boolean> .

<https://atproto.social/ontology/app.bsky.feed.defs#viewerState/replyDisabled>
        a            owl:DatatypeProperty;
        rdfs:domain  <https://atproto.social/ontology/app.bsky.feed.defs#viewerState>;
        rdfs:range   <xsd:boolean> .

<https://atproto.social/ontology/app.bsky.feed.defs#viewerState/embeddingDisabled>
        a            owl:DatatypeProperty;
        rdfs:domain  <https://atproto.social/ontology/app.bsky.feed.defs#viewerState>;
        rdfs:range   <xsd:boolean> .

<https://atproto.social/ontology/app.bsky.feed.defs#threadViewPost>
        a       owl:Class .

<https://atproto.social/ontology/app.bsky.feed.defs#threadViewPost/replies>
        a            owl:ObjectProperty;
        rdfs:domain  <https://atproto.social/ontology/app.bsky.feed.defs#threadViewPost> .

<https://atproto.social/ontology/app.bsky.feed.defs#threadViewPost/threadContext>
        a            owl:ObjectProperty;
        rdfs:domain  <https://atproto.social/ontology/app.bsky.feed.defs#threadViewPost>;
        rdfs:range   <https://atproto.social/ontology/app.bsky.feed.defs#threadContext> .

<https://atproto.social/ontology/app.bsky.feed.defs#threadViewPost/post>
        a            owl:ObjectProperty;
        rdfs:domain  <https://atproto.social/ontology/app.bsky.feed.defs#threadViewPost>;
        rdfs:range   <https://atproto.social/ontology/app.bsky.feed.defs#postView> .

<https://atproto.social/ontology/app.bsky.feed.defs#threadViewPost/parent>
        a            owl:ObjectProperty;
        rdfs:domain  <https://atproto.social/ontology/app.bsky.feed.defs#threadViewPost> .

<https://atproto.social/ontology/app.bsky.feed.defs#clickthroughEmbed>
        a             owl:Class;
        rdfs:comment  "User clicked through to the embedded content of the feed item" .

<https://atproto.social/ontology/app.bsky.feed.defs#interactionShare>
        a             owl:Class;
        rdfs:comment  "User shared the feed item" .

<https://atproto.social/ontology/app.bsky.feed.defs#threadContext>
        a             owl:Class;
        rdfs:comment  "Metadata about this post within the context of the thread it is in." .

<https://atproto.social/ontology/app.bsky.feed.defs#threadContext/rootAuthorLike>
        a            owl:DatatypeProperty;
        rdfs:domain  <https://atproto.social/ontology/app.bsky.feed.defs#threadContext>;
        rdfs:range   <xsd:string> .

<https://atproto.social/ontology/app.bsky.feed.defs#reasonPin>
        a       owl:Class .

<https://atproto.social/ontology/app.bsky.feed.defs#notFoundPost>
        a       owl:Class .

<https://atproto.social/ontology/app.bsky.feed.defs#notFoundPost/uri>
        a            owl:DatatypeProperty;
        rdfs:domain  <https://atproto.social/ontology/app.bsky.feed.defs#notFoundPost>;
        rdfs:range   <xsd:string> .

<https://atproto.social/ontology/app.bsky.feed.defs#notFoundPost/notFound>
        a            owl:DatatypeProperty;
        rdfs:domain  <https://atproto.social/ontology/app.bsky.feed.defs#notFoundPost>;
        rdfs:range   <xsd:boolean> .

<https://atproto.social/ontology/app.bsky.feed.defs#skeletonReasonPin>
        a       owl:Class .

<https://atproto.social/ontology/app.bsky.feed.describeFeedGenerator#main>
        a             owl:Class;
        rdfs:comment  "Get information about a feed generator, including policies and offered feed URIs. Does not require auth; implemented by Feed Generator services (not App View)." .

<https://atproto.social/ontology/app.bsky.feed.describeFeedGenerator#feed>
        a       owl:Class .

<https://atproto.social/ontology/app.bsky.feed.describeFeedGenerator#feed/uri>
        a            owl:DatatypeProperty;
        rdfs:domain  <https://atproto.social/ontology/app.bsky.feed.describeFeedGenerator#feed>;
        rdfs:range   <xsd:string> .

<https://atproto.social/ontology/app.bsky.feed.describeFeedGenerator#links>
        a       owl:Class .

<https://atproto.social/ontology/app.bsky.feed.describeFeedGenerator#links/privacyPolicy>
        a            owl:DatatypeProperty;
        rdfs:domain  <https://atproto.social/ontology/app.bsky.feed.describeFeedGenerator#links>;
        rdfs:range   <xsd:string> .

<https://atproto.social/ontology/app.bsky.feed.describeFeedGenerator#links/termsOfService>
        a            owl:DatatypeProperty;
        rdfs:domain  <https://atproto.social/ontology/app.bsky.feed.describeFeedGenerator#links>;
        rdfs:range   <xsd:string> .

<https://atproto.social/ontology/app.bsky.feed.generator#main>
        a             owl:Class;
        rdfs:comment  "Record declaring of the existence of a feed generator, and containing metadata about it. The record can exist in any repository." .

<https://atproto.social/ontology/app.bsky.feed.getActorFeeds#main>
        a             owl:Class;
        rdfs:comment  "Get a list of feeds (feed generator records) created by the actor (in the actor's repo)." .

<https://atproto.social/ontology/app.bsky.feed.getActorLikes#main>
        a             owl:Class;
        rdfs:comment  "Get a list of posts liked by an actor. Requires auth, actor must be the requesting account." .

<https://atproto.social/ontology/app.bsky.feed.getAuthorFeed#main>
        a             owl:Class;
        rdfs:comment  "Get a view of an actor's 'author feed' (post and reposts by the author). Does not require auth." .

<https://atproto.social/ontology/app.bsky.feed.getFeed#main>
        a             owl:Class;
        rdfs:comment  "Get a hydrated feed from an actor's selected feed generator. Implemented by App View." .

<https://atproto.social/ontology/app.bsky.feed.getFeedGenerator#main>
        a             owl:Class;
        rdfs:comment  "Get information about a feed generator. Implemented by AppView." .

<https://atproto.social/ontology/app.bsky.feed.getFeedGenerators#main>
        a             owl:Class;
        rdfs:comment  "Get information about a list of feed generators." .

<https://atproto.social/ontology/app.bsky.feed.getFeedSkeleton#main>
        a             owl:Class;
        rdfs:comment  "Get a skeleton of a feed provided by a feed generator. Auth is optional, depending on provider requirements, and provides the DID of the requester. Implemented by Feed Generator Service." .

<https://atproto.social/ontology/app.bsky.feed.getLikes#main>
        a             owl:Class;
        rdfs:comment  "Get like records which reference a subject (by AT-URI and CID)." .

<https://atproto.social/ontology/app.bsky.feed.getLikes#like>
        a       owl:Class .

<https://atproto.social/ontology/app.bsky.feed.getLikes#like/indexedAt>
        a            owl:DatatypeProperty;
        rdfs:domain  <https://atproto.social/ontology/app.bsky.feed.getLikes#like>;
        rdfs:range   <xsd:string> .

<https://atproto.social/ontology/app.bsky.feed.getLikes#like/createdAt>
        a            owl:DatatypeProperty;
        rdfs:domain  <https://atproto.social/ontology/app.bsky.feed.getLikes#like>;
        rdfs:range   <xsd:string> .

<https://atproto.social/ontology/app.bsky.feed.getLikes#like/actor>
        a            owl:ObjectProperty;
        rdfs:domain  <https://atproto.social/ontology/app.bsky.feed.getLikes#like>;
        rdfs:range   <https://atproto.social/ontology/app.bsky.actor.defs#profileView> .

<https://atproto.social/ontology/app.bsky.feed.getListFeed#main>
        a             owl:Class;
        rdfs:comment  "Get a feed of recent posts from a list (posts and reposts from any actors on the list). Does not require auth." .

<https://atproto.social/ontology/app.bsky.feed.getPostThread#main>
        a             owl:Class;
        rdfs:comment  "Get posts in a thread. Does not require auth, but additional metadata and filtering will be applied for authed requests." .

<https://atproto.social/ontology/app.bsky.feed.getPosts#main>
        a             owl:Class;
        rdfs:comment  "Gets post views for a specified list of posts (by AT-URI). This is sometimes referred to as 'hydrating' a 'feed skeleton'." .

<https://atproto.social/ontology/app.bsky.feed.getQuotes#main>
        a             owl:Class;
        rdfs:comment  "Get a list of quotes for a given post." .

<https://atproto.social/ontology/app.bsky.feed.getRepostedBy#main>
        a             owl:Class;
        rdfs:comment  "Get a list of reposts for a given post." .

<https://atproto.social/ontology/app.bsky.feed.getSuggestedFeeds#main>
        a             owl:Class;
        rdfs:comment  "Get a list of suggested feeds (feed generators) for the requesting account." .

<https://atproto.social/ontology/app.bsky.feed.getTimeline#main>
        a             owl:Class;
        rdfs:comment  "Get a view of the requesting account's home timeline. This is expected to be some form of reverse-chronological feed." .

<https://atproto.social/ontology/app.bsky.feed.like#main>
        a             owl:Class;
        rdfs:comment  "Record declaring a 'like' of a piece of subject content." .

<https://atproto.social/ontology/app.bsky.feed.post#entity>
        a             owl:Class;
        rdfs:comment  "Deprecated: use facets instead." .

<https://atproto.social/ontology/app.bsky.feed.post#entity/type>
        a             owl:DatatypeProperty;
        rdfs:domain   <https://atproto.social/ontology/app.bsky.feed.post#entity>;
        rdfs:range    <xsd:string>;
        rdfs:comment  "Expected values are 'mention' and 'link'." .

<https://atproto.social/ontology/app.bsky.feed.post#entity/value>
        a            owl:DatatypeProperty;
        rdfs:domain  <https://atproto.social/ontology/app.bsky.feed.post#entity>;
        rdfs:range   <xsd:string> .

<https://atproto.social/ontology/app.bsky.feed.post#entity/index>
        a            owl:ObjectProperty;
        rdfs:domain  <https://atproto.social/ontology/app.bsky.feed.post#entity>;
        rdfs:range   <https://atproto.social/ontology/app.bsky.feed.post#textSlice> .

<https://atproto.social/ontology/app.bsky.feed.post#textSlice>
        a             owl:Class;
        rdfs:comment  "Deprecated. Use app.bsky.richtext instead -- A text segment. Start is inclusive, end is exclusive. Indices are for utf16-encoded strings." .

<https://atproto.social/ontology/app.bsky.feed.post#textSlice/start>
        a            owl:DatatypeProperty;
        rdfs:domain  <https://atproto.social/ontology/app.bsky.feed.post#textSlice>;
        rdfs:range   <xsd:integer> .

<https://atproto.social/ontology/app.bsky.feed.post#textSlice/end>
        a            owl:DatatypeProperty;
        rdfs:domain  <https://atproto.social/ontology/app.bsky.feed.post#textSlice>;
        rdfs:range   <xsd:integer> .

<https://atproto.social/ontology/app.bsky.feed.post#main>
        a             owl:Class;
        rdfs:comment  "Record containing a Bluesky post." .

<https://atproto.social/ontology/app.bsky.feed.post#replyRef>
        a       owl:Class .

<https://atproto.social/ontology/app.bsky.feed.post#replyRef/root>
        a            owl:ObjectProperty;
        rdfs:domain  <https://atproto.social/ontology/app.bsky.feed.post#replyRef>;
        rdfs:range   <https://atproto.social/ontology/app.bsky.feed.post#com.atproto.repo.strongRef> .

<https://atproto.social/ontology/app.bsky.feed.post#replyRef/parent>
        a            owl:ObjectProperty;
        rdfs:domain  <https://atproto.social/ontology/app.bsky.feed.post#replyRef>;
        rdfs:range   <https://atproto.social/ontology/app.bsky.feed.post#com.atproto.repo.strongRef> .

<https://atproto.social/ontology/app.bsky.feed.postgate#main>
        a             owl:Class;
        rdfs:comment  "Record defining interaction rules for a post. The record key (rkey) of the postgate record must match the record key of the post, and that record must be in the same repository." .

<https://atproto.social/ontology/app.bsky.feed.postgate#disableRule>
        a             owl:Class;
        rdfs:comment  "Disables embedding of this post." .

<https://atproto.social/ontology/app.bsky.feed.repost#main>
        a             owl:Class;
        rdfs:comment  "Record representing a 'repost' of an existing Bluesky post." .

<https://atproto.social/ontology/app.bsky.feed.searchPosts#main>
        a             owl:Class;
        rdfs:comment  "Find posts matching search criteria, returning views of those posts. Note that this API endpoint may require authentication (eg, not public) for some service providers and implementations." .

<https://atproto.social/ontology/app.bsky.feed.sendInteractions#main>
        a             owl:Class;
        rdfs:comment  "Send information about interactions with feed items back to the feed generator that served them." .

<https://atproto.social/ontology/app.bsky.feed.threadgate#followingRule>
        a             owl:Class;
        rdfs:comment  "Allow replies from actors you follow." .

<https://atproto.social/ontology/app.bsky.feed.threadgate#listRule>
        a             owl:Class;
        rdfs:comment  "Allow replies from actors on a list." .

<https://atproto.social/ontology/app.bsky.feed.threadgate#listRule/list>
        a            owl:DatatypeProperty;
        rdfs:domain  <https://atproto.social/ontology/app.bsky.feed.threadgate#listRule>;
        rdfs:range   <xsd:string> .

<https://atproto.social/ontology/app.bsky.feed.threadgate#main>
        a             owl:Class;
        rdfs:comment  "Record defining interaction gating rules for a thread (aka, reply controls). The record key (rkey) of the threadgate record must match the record key of the thread's root post, and that record must be in the same repository." .

<https://atproto.social/ontology/app.bsky.feed.threadgate#mentionRule>
        a             owl:Class;
        rdfs:comment  "Allow replies from actors mentioned in your post." .

<https://atproto.social/ontology/app.bsky.feed.threadgate#followerRule>
        a             owl:Class;
        rdfs:comment  "Allow replies from actors who follow you." .

<https://atproto.social/ontology/app.bsky.graph.block#main>
        a             owl:Class;
        rdfs:comment  "Record declaring a 'block' relationship against another account. NOTE: blocks are public in Bluesky; see blog posts for details." .

<https://atproto.social/ontology/app.bsky.graph.defs#listViewBasic>
        a       owl:Class .

<https://atproto.social/ontology/app.bsky.graph.defs#listViewBasic/name>
        a            owl:DatatypeProperty;
        rdfs:domain  <https://atproto.social/ontology/app.bsky.graph.defs#listViewBasic>;
        rdfs:range   <xsd:string> .

<https://atproto.social/ontology/app.bsky.graph.defs#listViewBasic/viewer>
        a            owl:ObjectProperty;
        rdfs:domain  <https://atproto.social/ontology/app.bsky.graph.defs#listViewBasic>;
        rdfs:range   <https://atproto.social/ontology/app.bsky.graph.defs#listViewerState> .

<https://atproto.social/ontology/app.bsky.graph.defs#listViewBasic/cid>
        a            owl:DatatypeProperty;
        rdfs:domain  <https://atproto.social/ontology/app.bsky.graph.defs#listViewBasic>;
        rdfs:range   <xsd:string> .

<https://atproto.social/ontology/app.bsky.graph.defs#listViewBasic/purpose>
        a            owl:ObjectProperty;
        rdfs:domain  <https://atproto.social/ontology/app.bsky.graph.defs#listViewBasic>;
        rdfs:range   <https://atproto.social/ontology/app.bsky.graph.defs#listPurpose> .

<https://atproto.social/ontology/app.bsky.graph.defs#listViewBasic/avatar>
        a            owl:DatatypeProperty;
        rdfs:domain  <https://atproto.social/ontology/app.bsky.graph.defs#listViewBasic>;
        rdfs:range   <xsd:string> .

<https://atproto.social/ontology/app.bsky.graph.defs#listViewBasic/listItemCount>
        a            owl:DatatypeProperty;
        rdfs:domain  <https://atproto.social/ontology/app.bsky.graph.defs#listViewBasic>;
        rdfs:range   <xsd:integer> .

<https://atproto.social/ontology/app.bsky.graph.defs#listViewBasic/labels>
        a            owl:ObjectProperty;
        rdfs:domain  <https://atproto.social/ontology/app.bsky.graph.defs#listViewBasic>;
        rdfs:range   <https://atproto.social/ontology/com.atproto.label.defs#label> .

<https://atproto.social/ontology/app.bsky.graph.defs#listViewBasic/indexedAt>
        a            owl:DatatypeProperty;
        rdfs:domain  <https://atproto.social/ontology/app.bsky.graph.defs#listViewBasic>;
        rdfs:range   <xsd:string> .

<https://atproto.social/ontology/app.bsky.graph.defs#listViewBasic/uri>
        a            owl:DatatypeProperty;
        rdfs:domain  <https://atproto.social/ontology/app.bsky.graph.defs#listViewBasic>;
        rdfs:range   <xsd:string> .

<https://atproto.social/ontology/app.bsky.graph.defs#listView>
        a       owl:Class .

<https://atproto.social/ontology/app.bsky.graph.defs#listView/cid>
        a            owl:DatatypeProperty;
        rdfs:domain  <https://atproto.social/ontology/app.bsky.graph.defs#listView>;
        rdfs:range   <xsd:string> .

<https://atproto.social/ontology/app.bsky.graph.defs#listView/name>
        a            owl:DatatypeProperty;
        rdfs:domain  <https://atproto.social/ontology/app.bsky.graph.defs#listView>;
        rdfs:range   <xsd:string> .

<https://atproto.social/ontology/app.bsky.graph.defs#listView/descriptionFacets>
        a            owl:ObjectProperty;
        rdfs:domain  <https://atproto.social/ontology/app.bsky.graph.defs#listView>;
        rdfs:range   <https://atproto.social/ontology/app.bsky.graph.defs#app.bsky.richtext.facet> .

<https://atproto.social/ontology/app.bsky.graph.defs#listView/viewer>
        a            owl:ObjectProperty;
        rdfs:domain  <https://atproto.social/ontology/app.bsky.graph.defs#listView>;
        rdfs:range   <https://atproto.social/ontology/app.bsky.graph.defs#listViewerState> .

<https://atproto.social/ontology/app.bsky.graph.defs#listView/indexedAt>
        a            owl:DatatypeProperty;
        rdfs:domain  <https://atproto.social/ontology/app.bsky.graph.defs#listView>;
        rdfs:range   <xsd:string> .

<https://atproto.social/ontology/app.bsky.graph.defs#listView/uri>
        a            owl:DatatypeProperty;
        rdfs:domain  <https://atproto.social/ontology/app.bsky.graph.defs#listView>;
        rdfs:range   <xsd:string> .

<https://atproto.social/ontology/app.bsky.graph.defs#listView/creator>
        a            owl:ObjectProperty;
        rdfs:domain  <https://atproto.social/ontology/app.bsky.graph.defs#listView>;
        rdfs:range   <https://atproto.social/ontology/app.bsky.actor.defs#profileView> .

<https://atproto.social/ontology/app.bsky.graph.defs#listView/purpose>
        a            owl:ObjectProperty;
        rdfs:domain  <https://atproto.social/ontology/app.bsky.graph.defs#listView>;
        rdfs:range   <https://atproto.social/ontology/app.bsky.graph.defs#listPurpose> .

<https://atproto.social/ontology/app.bsky.graph.defs#listView/description>
        a            owl:DatatypeProperty;
        rdfs:domain  <https://atproto.social/ontology/app.bsky.graph.defs#listView>;
        rdfs:range   <xsd:string> .

<https://atproto.social/ontology/app.bsky.graph.defs#listView/avatar>
        a            owl:DatatypeProperty;
        rdfs:domain  <https://atproto.social/ontology/app.bsky.graph.defs#listView>;
        rdfs:range   <xsd:string> .

<https://atproto.social/ontology/app.bsky.graph.defs#listView/listItemCount>
        a            owl:DatatypeProperty;
        rdfs:domain  <https://atproto.social/ontology/app.bsky.graph.defs#listView>;
        rdfs:range   <xsd:integer> .

<https://atproto.social/ontology/app.bsky.graph.defs#listView/labels>
        a            owl:ObjectProperty;
        rdfs:domain  <https://atproto.social/ontology/app.bsky.graph.defs#listView>;
        rdfs:range   <https://atproto.social/ontology/com.atproto.label.defs#label> .

<https://atproto.social/ontology/app.bsky.graph.defs#starterPackViewBasic>
        a       owl:Class .

<https://atproto.social/ontology/app.bsky.graph.defs#starterPackViewBasic/listItemCount>
        a            owl:DatatypeProperty;
        rdfs:domain  <https://atproto.social/ontology/app.bsky.graph.defs#starterPackViewBasic>;
        rdfs:range   <xsd:integer> .

<https://atproto.social/ontology/app.bsky.graph.defs#starterPackViewBasic/indexedAt>
        a            owl:DatatypeProperty;
        rdfs:domain  <https://atproto.social/ontology/app.bsky.graph.defs#starterPackViewBasic>;
        rdfs:range   <xsd:string> .

<https://atproto.social/ontology/app.bsky.graph.defs#starterPackViewBasic/uri>
        a            owl:DatatypeProperty;
        rdfs:domain  <https://atproto.social/ontology/app.bsky.graph.defs#starterPackViewBasic>;
        rdfs:range   <xsd:string> .

<https://atproto.social/ontology/app.bsky.graph.defs#starterPackViewBasic/cid>
        a            owl:DatatypeProperty;
        rdfs:domain  <https://atproto.social/ontology/app.bsky.graph.defs#starterPackViewBasic>;
        rdfs:range   <xsd:string> .

<https://atproto.social/ontology/app.bsky.graph.defs#starterPackViewBasic/joinedWeekCount>
        a            owl:DatatypeProperty;
        rdfs:domain  <https://atproto.social/ontology/app.bsky.graph.defs#starterPackViewBasic>;
        rdfs:range   <xsd:integer> .

<https://atproto.social/ontology/app.bsky.graph.defs#starterPackViewBasic/joinedAllTimeCount>
        a            owl:DatatypeProperty;
        rdfs:domain  <https://atproto.social/ontology/app.bsky.graph.defs#starterPackViewBasic>;
        rdfs:range   <xsd:integer> .

<https://atproto.social/ontology/app.bsky.graph.defs#starterPackViewBasic/labels>
        a            owl:ObjectProperty;
        rdfs:domain  <https://atproto.social/ontology/app.bsky.graph.defs#starterPackViewBasic>;
        rdfs:range   <https://atproto.social/ontology/com.atproto.label.defs#label> .

<https://atproto.social/ontology/app.bsky.graph.defs#starterPackViewBasic/record>
        a            owl:ObjectProperty;
        rdfs:domain  <https://atproto.social/ontology/app.bsky.graph.defs#starterPackViewBasic> .

<https://atproto.social/ontology/app.bsky.graph.defs#starterPackViewBasic/creator>
        a            owl:ObjectProperty;
        rdfs:domain  <https://atproto.social/ontology/app.bsky.graph.defs#starterPackViewBasic>;
        rdfs:range   <https://atproto.social/ontology/app.bsky.actor.defs#profileViewBasic> .

<https://atproto.social/ontology/app.bsky.graph.defs#listPurpose>
        a       owl:Class .

<https://atproto.social/ontology/app.bsky.graph.defs#modlist>
        a             owl:Class;
        rdfs:comment  "A list of actors to apply an aggregate moderation action (mute/block) on." .

<https://atproto.social/ontology/app.bsky.graph.defs#listViewerState>
        a       owl:Class .

<https://atproto.social/ontology/app.bsky.graph.defs#listViewerState/muted>
        a            owl:DatatypeProperty;
        rdfs:domain  <https://atproto.social/ontology/app.bsky.graph.defs#listViewerState>;
        rdfs:range   <xsd:boolean> .

<https://atproto.social/ontology/app.bsky.graph.defs#listViewerState/blocked>
        a            owl:DatatypeProperty;
        rdfs:domain  <https://atproto.social/ontology/app.bsky.graph.defs#listViewerState>;
        rdfs:range   <xsd:string> .

<https://atproto.social/ontology/app.bsky.graph.defs#relationship>
        a             owl:Class;
        rdfs:comment  "lists the bi-directional graph relationships between one actor (not indicated in the object), and the target actors (the DID included in the object)" .

<https://atproto.social/ontology/app.bsky.graph.defs#relationship/did>
        a            owl:DatatypeProperty;
        rdfs:domain  <https://atproto.social/ontology/app.bsky.graph.defs#relationship>;
        rdfs:range   <xsd:string> .

<https://atproto.social/ontology/app.bsky.graph.defs#relationship/following>
        a             owl:DatatypeProperty;
        rdfs:domain   <https://atproto.social/ontology/app.bsky.graph.defs#relationship>;
        rdfs:range    <xsd:string>;
        rdfs:comment  "if the actor follows this DID, this is the AT-URI of the follow record" .

<https://atproto.social/ontology/app.bsky.graph.defs#relationship/followedBy>
        a             owl:DatatypeProperty;
        rdfs:domain   <https://atproto.social/ontology/app.bsky.graph.defs#relationship>;
        rdfs:range    <xsd:string>;
        rdfs:comment  "if the actor is followed by this DID, contains the AT-URI of the follow record" .

<https://atproto.social/ontology/app.bsky.graph.defs#listItemView>
        a       owl:Class .

<https://atproto.social/ontology/app.bsky.graph.defs#listItemView/uri>
        a            owl:DatatypeProperty;
        rdfs:domain  <https://atproto.social/ontology/app.bsky.graph.defs#listItemView>;
        rdfs:range   <xsd:string> .

<https://atproto.social/ontology/app.bsky.graph.defs#listItemView/subject>
        a            owl:ObjectProperty;
        rdfs:domain  <https://atproto.social/ontology/app.bsky.graph.defs#listItemView>;
        rdfs:range   <https://atproto.social/ontology/app.bsky.actor.defs#profileView> .

<https://atproto.social/ontology/app.bsky.graph.defs#starterPackView>
        a       owl:Class .

<https://atproto.social/ontology/app.bsky.graph.defs#starterPackView/joinedAllTimeCount>
        a            owl:DatatypeProperty;
        rdfs:domain  <https://atproto.social/ontology/app.bsky.graph.defs#starterPackView>;
        rdfs:range   <xsd:integer> .

<https://atproto.social/ontology/app.bsky.graph.defs#starterPackView/uri>
        a            owl:DatatypeProperty;
        rdfs:domain  <https://atproto.social/ontology/app.bsky.graph.defs#starterPackView>;
        rdfs:range   <xsd:string> .

<https://atproto.social/ontology/app.bsky.graph.defs#starterPackView/cid>
        a            owl:DatatypeProperty;
        rdfs:domain  <https://atproto.social/ontology/app.bsky.graph.defs#starterPackView>;
        rdfs:range   <xsd:string> .

<https://atproto.social/ontology/app.bsky.graph.defs#starterPackView/listItemsSample>
        a            owl:ObjectProperty;
        rdfs:domain  <https://atproto.social/ontology/app.bsky.graph.defs#starterPackView>;
        rdfs:range   <https://atproto.social/ontology/app.bsky.graph.defs#listItemView> .

<https://atproto.social/ontology/app.bsky.graph.defs#starterPackView/feeds>
        a            owl:ObjectProperty;
        rdfs:domain  <https://atproto.social/ontology/app.bsky.graph.defs#starterPackView>;
        rdfs:range   <https://atproto.social/ontology/app.bsky.feed.defs#generatorView> .

<https://atproto.social/ontology/app.bsky.graph.defs#starterPackView/labels>
        a            owl:ObjectProperty;
        rdfs:domain  <https://atproto.social/ontology/app.bsky.graph.defs#starterPackView>;
        rdfs:range   <https://atproto.social/ontology/com.atproto.label.defs#label> .

<https://atproto.social/ontology/app.bsky.graph.defs#starterPackView/indexedAt>
        a            owl:DatatypeProperty;
        rdfs:domain  <https://atproto.social/ontology/app.bsky.graph.defs#starterPackView>;
        rdfs:range   <xsd:string> .

<https://atproto.social/ontology/app.bsky.graph.defs#starterPackView/record>
        a            owl:ObjectProperty;
        rdfs:domain  <https://atproto.social/ontology/app.bsky.graph.defs#starterPackView> .

<https://atproto.social/ontology/app.bsky.graph.defs#starterPackView/creator>
        a            owl:ObjectProperty;
        rdfs:domain  <https://atproto.social/ontology/app.bsky.graph.defs#starterPackView>;
        rdfs:range   <https://atproto.social/ontology/app.bsky.actor.defs#profileViewBasic> .

<https://atproto.social/ontology/app.bsky.graph.defs#starterPackView/list>
        a            owl:ObjectProperty;
        rdfs:domain  <https://atproto.social/ontology/app.bsky.graph.defs#starterPackView>;
        rdfs:range   <https://atproto.social/ontology/app.bsky.graph.defs#listViewBasic> .

<https://atproto.social/ontology/app.bsky.graph.defs#starterPackView/joinedWeekCount>
        a            owl:DatatypeProperty;
        rdfs:domain  <https://atproto.social/ontology/app.bsky.graph.defs#starterPackView>;
        rdfs:range   <xsd:integer> .

<https://atproto.social/ontology/app.bsky.graph.defs#curatelist>
        a             owl:Class;
        rdfs:comment  "A list of actors used for curation purposes such as list feeds or interaction gating." .

<https://atproto.social/ontology/app.bsky.graph.defs#referencelist>
        a             owl:Class;
        rdfs:comment  "A list of actors used for only for reference purposes such as within a starter pack." .

<https://atproto.social/ontology/app.bsky.graph.defs#notFoundActor>
        a             owl:Class;
        rdfs:comment  "indicates that a handle or DID could not be resolved" .

<https://atproto.social/ontology/app.bsky.graph.defs#notFoundActor/actor>
        a            owl:DatatypeProperty;
        rdfs:domain  <https://atproto.social/ontology/app.bsky.graph.defs#notFoundActor>;
        rdfs:range   <xsd:string> .

<https://atproto.social/ontology/app.bsky.graph.defs#notFoundActor/notFound>
        a            owl:DatatypeProperty;
        rdfs:domain  <https://atproto.social/ontology/app.bsky.graph.defs#notFoundActor>;
        rdfs:range   <xsd:boolean> .

<https://atproto.social/ontology/app.bsky.graph.follow#main>
        a             owl:Class;
        rdfs:comment  "Record declaring a social 'follow' relationship of another account. Duplicate follows will be ignored by the AppView." .

<https://atproto.social/ontology/app.bsky.graph.getActorStarterPacks#main>
        a             owl:Class;
        rdfs:comment  "Get a list of starter packs created by the actor." .

<https://atproto.social/ontology/app.bsky.graph.getBlocks#main>
        a             owl:Class;
        rdfs:comment  "Enumerates which accounts the requesting account is currently blocking. Requires auth." .

<https://atproto.social/ontology/app.bsky.graph.getFollowers#main>
        a             owl:Class;
        rdfs:comment  "Enumerates accounts which follow a specified account (actor)." .

<https://atproto.social/ontology/app.bsky.graph.getFollows#main>
        a             owl:Class;
        rdfs:comment  "Enumerates accounts which a specified account (actor) follows." .

<https://atproto.social/ontology/app.bsky.graph.getKnownFollowers#main>
        a             owl:Class;
        rdfs:comment  "Enumerates accounts which follow a specified account (actor) and are followed by the viewer." .

<https://atproto.social/ontology/app.bsky.graph.getList#main>
        a             owl:Class;
        rdfs:comment  "Gets a 'view' (with additional context) of a specified list." .

<https://atproto.social/ontology/app.bsky.graph.getListBlocks#main>
        a             owl:Class;
        rdfs:comment  "Get mod lists that the requesting account (actor) is blocking. Requires auth." .

<https://atproto.social/ontology/app.bsky.graph.getListMutes#main>
        a             owl:Class;
        rdfs:comment  "Enumerates mod lists that the requesting account (actor) currently has muted. Requires auth." .

<https://atproto.social/ontology/app.bsky.graph.getLists#main>
        a             owl:Class;
        rdfs:comment  "Enumerates the lists created by a specified account (actor)." .

<https://atproto.social/ontology/app.bsky.graph.getMutes#main>
        a             owl:Class;
        rdfs:comment  "Enumerates accounts that the requesting account (actor) currently has muted. Requires auth." .

<https://atproto.social/ontology/app.bsky.graph.getRelationships#main>
        a             owl:Class;
        rdfs:comment  "Enumerates public relationships between one account, and a list of other accounts. Does not require auth." .

<https://atproto.social/ontology/app.bsky.graph.getStarterPack#main>
        a             owl:Class;
        rdfs:comment  "Gets a view of a starter pack." .

<https://atproto.social/ontology/app.bsky.graph.getStarterPacks#main>
        a             owl:Class;
        rdfs:comment  "Get views for a list of starter packs." .

<https://atproto.social/ontology/app.bsky.graph.getSuggestedFollowsByActor#main>
        a             owl:Class;
        rdfs:comment  "Enumerates follows similar to a given account (actor). Expected use is to recommend additional accounts immediately after following one account." .

<https://atproto.social/ontology/app.bsky.graph.list#main>
        a             owl:Class;
        rdfs:comment  "Record representing a list of accounts (actors). Scope includes both moderation-oriented lists and curration-oriented lists." .

<https://atproto.social/ontology/app.bsky.graph.listblock#main>
        a             owl:Class;
        rdfs:comment  "Record representing a block relationship against an entire an entire list of accounts (actors)." .

<https://atproto.social/ontology/app.bsky.graph.listitem#main>
        a             owl:Class;
        rdfs:comment  "Record representing an account's inclusion on a specific list. The AppView will ignore duplicate listitem records." .

<https://atproto.social/ontology/app.bsky.graph.muteActor#main>
        a             owl:Class;
        rdfs:comment  "Creates a mute relationship for the specified account. Mutes are private in Bluesky. Requires auth." .

<https://atproto.social/ontology/app.bsky.graph.muteActorList#main>
        a             owl:Class;
        rdfs:comment  "Creates a mute relationship for the specified list of accounts. Mutes are private in Bluesky. Requires auth." .

<https://atproto.social/ontology/app.bsky.graph.muteThread#main>
        a             owl:Class;
        rdfs:comment  "Mutes a thread preventing notifications from the thread and any of its children. Mutes are private in Bluesky. Requires auth." .

<https://atproto.social/ontology/app.bsky.graph.searchStarterPacks#main>
        a             owl:Class;
        rdfs:comment  "Find starter packs matching search criteria. Does not require auth." .

<https://atproto.social/ontology/app.bsky.graph.starterpack#main>
        a             owl:Class;
        rdfs:comment  "Record defining a starter pack of actors and feeds for new users." .

<https://atproto.social/ontology/app.bsky.graph.starterpack#feedItem>
        a       owl:Class .

<https://atproto.social/ontology/app.bsky.graph.starterpack#feedItem/uri>
        a            owl:DatatypeProperty;
        rdfs:domain  <https://atproto.social/ontology/app.bsky.graph.starterpack#feedItem>;
        rdfs:range   <xsd:string> .

<https://atproto.social/ontology/app.bsky.graph.unmuteActor#main>
        a             owl:Class;
        rdfs:comment  "Unmutes the specified account. Requires auth." .

<https://atproto.social/ontology/app.bsky.graph.unmuteActorList#main>
        a             owl:Class;
        rdfs:comment  "Unmutes the specified list of accounts. Requires auth." .

<https://atproto.social/ontology/app.bsky.graph.unmuteThread#main>
        a             owl:Class;
        rdfs:comment  "Unmutes the specified thread. Requires auth." .

<https://atproto.social/ontology/app.bsky.graph.verification#main>
        a             owl:Class;
        rdfs:comment  "Record declaring a verification relationship between two accounts. Verifications are only considered valid by an app if issued by an account the app considers trusted." .

<https://atproto.social/ontology/app.bsky.labeler.defs#labelerView>
        a       owl:Class .

<https://atproto.social/ontology/app.bsky.labeler.defs#labelerView/labels>
        a            owl:ObjectProperty;
        rdfs:domain  <https://atproto.social/ontology/app.bsky.labeler.defs#labelerView>;
        rdfs:range   <https://atproto.social/ontology/com.atproto.label.defs#label> .

<https://atproto.social/ontology/app.bsky.labeler.defs#labelerView/uri>
        a            owl:DatatypeProperty;
        rdfs:domain  <https://atproto.social/ontology/app.bsky.labeler.defs#labelerView>;
        rdfs:range   <xsd:string> .

<https://atproto.social/ontology/app.bsky.labeler.defs#labelerView/cid>
        a            owl:DatatypeProperty;
        rdfs:domain  <https://atproto.social/ontology/app.bsky.labeler.defs#labelerView>;
        rdfs:range   <xsd:string> .

<https://atproto.social/ontology/app.bsky.labeler.defs#labelerView/creator>
        a            owl:ObjectProperty;
        rdfs:domain  <https://atproto.social/ontology/app.bsky.labeler.defs#labelerView>;
        rdfs:range   <https://atproto.social/ontology/app.bsky.actor.defs#profileView> .

<https://atproto.social/ontology/app.bsky.labeler.defs#labelerView/likeCount>
        a            owl:DatatypeProperty;
        rdfs:domain  <https://atproto.social/ontology/app.bsky.labeler.defs#labelerView>;
        rdfs:range   <xsd:integer> .

<https://atproto.social/ontology/app.bsky.labeler.defs#labelerView/viewer>
        a            owl:ObjectProperty;
        rdfs:domain  <https://atproto.social/ontology/app.bsky.labeler.defs#labelerView>;
        rdfs:range   <https://atproto.social/ontology/app.bsky.labeler.defs#labelerViewerState> .

<https://atproto.social/ontology/app.bsky.labeler.defs#labelerView/indexedAt>
        a            owl:DatatypeProperty;
        rdfs:domain  <https://atproto.social/ontology/app.bsky.labeler.defs#labelerView>;
        rdfs:range   <xsd:string> .

<https://atproto.social/ontology/app.bsky.labeler.defs#labelerViewDetailed>
        a       owl:Class .

<https://atproto.social/ontology/app.bsky.labeler.defs#labelerViewDetailed/cid>
        a            owl:DatatypeProperty;
        rdfs:domain  <https://atproto.social/ontology/app.bsky.labeler.defs#labelerViewDetailed>;
        rdfs:range   <xsd:string> .

<https://atproto.social/ontology/app.bsky.labeler.defs#labelerViewDetailed/viewer>
        a            owl:ObjectProperty;
        rdfs:domain  <https://atproto.social/ontology/app.bsky.labeler.defs#labelerViewDetailed>;
        rdfs:range   <https://atproto.social/ontology/app.bsky.labeler.defs#labelerViewerState> .

<https://atproto.social/ontology/app.bsky.labeler.defs#labelerViewDetailed/labels>
        a            owl:ObjectProperty;
        rdfs:domain  <https://atproto.social/ontology/app.bsky.labeler.defs#labelerViewDetailed>;
        rdfs:range   <https://atproto.social/ontology/com.atproto.label.defs#label> .

<https://atproto.social/ontology/app.bsky.labeler.defs#labelerViewDetailed/reasonTypes>
        a             owl:ObjectProperty;
        rdfs:domain   <https://atproto.social/ontology/app.bsky.labeler.defs#labelerViewDetailed>;
        rdfs:range    <https://atproto.social/ontology/com.atproto.moderation.defs#reasonType>;
        rdfs:comment  "The set of report reason 'codes' which are in-scope for this service to review and action. These usually align to policy categories. If not defined (distinct from empty array), all reason types are allowed." .

<https://atproto.social/ontology/app.bsky.labeler.defs#labelerViewDetailed/creator>
        a            owl:ObjectProperty;
        rdfs:domain  <https://atproto.social/ontology/app.bsky.labeler.defs#labelerViewDetailed>;
        rdfs:range   <https://atproto.social/ontology/app.bsky.actor.defs#profileView> .

<https://atproto.social/ontology/app.bsky.labeler.defs#labelerViewDetailed/policies>
        a            owl:ObjectProperty;
        rdfs:domain  <https://atproto.social/ontology/app.bsky.labeler.defs#labelerViewDetailed>;
        rdfs:range   <https://atproto.social/ontology/app.bsky.labeler.defs#labelerPolicies> .

<https://atproto.social/ontology/app.bsky.labeler.defs#labelerViewDetailed/likeCount>
        a            owl:DatatypeProperty;
        rdfs:domain  <https://atproto.social/ontology/app.bsky.labeler.defs#labelerViewDetailed>;
        rdfs:range   <xsd:integer> .

<https://atproto.social/ontology/app.bsky.labeler.defs#labelerViewDetailed/indexedAt>
        a            owl:DatatypeProperty;
        rdfs:domain  <https://atproto.social/ontology/app.bsky.labeler.defs#labelerViewDetailed>;
        rdfs:range   <xsd:string> .

<https://atproto.social/ontology/app.bsky.labeler.defs#labelerViewDetailed/subjectTypes>
        a             owl:ObjectProperty;
        rdfs:domain   <https://atproto.social/ontology/app.bsky.labeler.defs#labelerViewDetailed>;
        rdfs:range    <https://atproto.social/ontology/com.atproto.moderation.defs#subjectType>;
        rdfs:comment  "The set of subject types (account, record, etc) this service accepts reports on." .

<https://atproto.social/ontology/app.bsky.labeler.defs#labelerViewDetailed/subjectCollections>
        a             owl:DatatypeProperty;
        rdfs:domain   <https://atproto.social/ontology/app.bsky.labeler.defs#labelerViewDetailed>;
        rdfs:range    <xsd:string>;
        rdfs:comment  "Set of record types (collection NSIDs) which can be reported to this service. If not defined (distinct from empty array), default is any record type." .

<https://atproto.social/ontology/app.bsky.labeler.defs#labelerViewDetailed/uri>
        a            owl:DatatypeProperty;
        rdfs:domain  <https://atproto.social/ontology/app.bsky.labeler.defs#labelerViewDetailed>;
        rdfs:range   <xsd:string> .

<https://atproto.social/ontology/app.bsky.labeler.defs#labelerViewerState>
        a       owl:Class .

<https://atproto.social/ontology/app.bsky.labeler.defs#labelerViewerState/like>
        a            owl:DatatypeProperty;
        rdfs:domain  <https://atproto.social/ontology/app.bsky.labeler.defs#labelerViewerState>;
        rdfs:range   <xsd:string> .

<https://atproto.social/ontology/app.bsky.labeler.defs#labelerPolicies>
        a       owl:Class .

<https://atproto.social/ontology/app.bsky.labeler.defs#labelerPolicies/labelValueDefinitions>
        a             owl:ObjectProperty;
        rdfs:domain   <https://atproto.social/ontology/app.bsky.labeler.defs#labelerPolicies>;
        rdfs:range    <https://atproto.social/ontology/com.atproto.label.defs#labelValueDefinition>;
        rdfs:comment  "Label values created by this labeler and scoped exclusively to it. Labels defined here will override global label definitions for this labeler." .

<https://atproto.social/ontology/app.bsky.labeler.defs#labelerPolicies/labelValues>
        a             owl:ObjectProperty;
        rdfs:domain   <https://atproto.social/ontology/app.bsky.labeler.defs#labelerPolicies>;
        rdfs:range    <https://atproto.social/ontology/com.atproto.label.defs#labelValue>;
        rdfs:comment  "The label values which this labeler publishes. May include global or custom labels." .

<https://atproto.social/ontology/app.bsky.labeler.getServices#main>
        a             owl:Class;
        rdfs:comment  "Get information about a list of labeler services." .

<https://atproto.social/ontology/app.bsky.labeler.service#main>
        a             owl:Class;
        rdfs:comment  "A declaration of the existence of labeler service." .

<https://atproto.social/ontology/app.bsky.notification.declaration#main>
        a             owl:Class;
        rdfs:comment  "A declaration of the user's choices related to notifications that can be produced by them." .

<https://atproto.social/ontology/app.bsky.notification.defs#recordDeleted>
        a       owl:Class .

<https://atproto.social/ontology/app.bsky.notification.defs#chatPreference>
        a       owl:Class .

<https://atproto.social/ontology/app.bsky.notification.defs#chatPreference/include>
        a            owl:DatatypeProperty;
        rdfs:domain  <https://atproto.social/ontology/app.bsky.notification.defs#chatPreference>;
        rdfs:range   <xsd:string> .

<https://atproto.social/ontology/app.bsky.notification.defs#chatPreference/push>
        a            owl:DatatypeProperty;
        rdfs:domain  <https://atproto.social/ontology/app.bsky.notification.defs#chatPreference>;
        rdfs:range   <xsd:boolean> .

<https://atproto.social/ontology/app.bsky.notification.defs#filterablePreference>
        a       owl:Class .

<https://atproto.social/ontology/app.bsky.notification.defs#filterablePreference/include>
        a            owl:DatatypeProperty;
        rdfs:domain  <https://atproto.social/ontology/app.bsky.notification.defs#filterablePreference>;
        rdfs:range   <xsd:string> .

<https://atproto.social/ontology/app.bsky.notification.defs#filterablePreference/list>
        a            owl:DatatypeProperty;
        rdfs:domain  <https://atproto.social/ontology/app.bsky.notification.defs#filterablePreference>;
        rdfs:range   <xsd:boolean> .

<https://atproto.social/ontology/app.bsky.notification.defs#filterablePreference/push>
        a            owl:DatatypeProperty;
        rdfs:domain  <https://atproto.social/ontology/app.bsky.notification.defs#filterablePreference>;
        rdfs:range   <xsd:boolean> .

<https://atproto.social/ontology/app.bsky.notification.defs#preference>
        a       owl:Class .

<https://atproto.social/ontology/app.bsky.notification.defs#preference/list>
        a            owl:DatatypeProperty;
        rdfs:domain  <https://atproto.social/ontology/app.bsky.notification.defs#preference>;
        rdfs:range   <xsd:boolean> .

<https://atproto.social/ontology/app.bsky.notification.defs#preference/push>
        a            owl:DatatypeProperty;
        rdfs:domain  <https://atproto.social/ontology/app.bsky.notification.defs#preference>;
        rdfs:range   <xsd:boolean> .

<https://atproto.social/ontology/app.bsky.notification.defs#preferences>
        a       owl:Class .

<https://atproto.social/ontology/app.bsky.notification.defs#preferences/like>
        a            owl:ObjectProperty;
        rdfs:domain  <https://atproto.social/ontology/app.bsky.notification.defs#preferences>;
        rdfs:range   <https://atproto.social/ontology/app.bsky.notification.defs#filterablePreference> .

<https://atproto.social/ontology/app.bsky.notification.defs#preferences/mention>
        a            owl:ObjectProperty;
        rdfs:domain  <https://atproto.social/ontology/app.bsky.notification.defs#preferences>;
        rdfs:range   <https://atproto.social/ontology/app.bsky.notification.defs#filterablePreference> .

<https://atproto.social/ontology/app.bsky.notification.defs#preferences/repostViaRepost>
        a            owl:ObjectProperty;
        rdfs:domain  <https://atproto.social/ontology/app.bsky.notification.defs#preferences>;
        rdfs:range   <https://atproto.social/ontology/app.bsky.notification.defs#filterablePreference> .

<https://atproto.social/ontology/app.bsky.notification.defs#preferences/subscribedPost>
        a            owl:ObjectProperty;
        rdfs:domain  <https://atproto.social/ontology/app.bsky.notification.defs#preferences>;
        rdfs:range   <https://atproto.social/ontology/app.bsky.notification.defs#preference> .

<https://atproto.social/ontology/app.bsky.notification.defs#preferences/unverified>
        a            owl:ObjectProperty;
        rdfs:domain  <https://atproto.social/ontology/app.bsky.notification.defs#preferences>;
        rdfs:range   <https://atproto.social/ontology/app.bsky.notification.defs#preference> .

<https://atproto.social/ontology/app.bsky.notification.defs#preferences/follow>
        a            owl:ObjectProperty;
        rdfs:domain  <https://atproto.social/ontology/app.bsky.notification.defs#preferences>;
        rdfs:range   <https://atproto.social/ontology/app.bsky.notification.defs#filterablePreference> .

<https://atproto.social/ontology/app.bsky.notification.defs#preferences/likeViaRepost>
        a            owl:ObjectProperty;
        rdfs:domain  <https://atproto.social/ontology/app.bsky.notification.defs#preferences>;
        rdfs:range   <https://atproto.social/ontology/app.bsky.notification.defs#filterablePreference> .

<https://atproto.social/ontology/app.bsky.notification.defs#preferences/quote>
        a            owl:ObjectProperty;
        rdfs:domain  <https://atproto.social/ontology/app.bsky.notification.defs#preferences>;
        rdfs:range   <https://atproto.social/ontology/app.bsky.notification.defs#filterablePreference> .

<https://atproto.social/ontology/app.bsky.notification.defs#preferences/reply>
        a            owl:ObjectProperty;
        rdfs:domain  <https://atproto.social/ontology/app.bsky.notification.defs#preferences>;
        rdfs:range   <https://atproto.social/ontology/app.bsky.notification.defs#filterablePreference> .

<https://atproto.social/ontology/app.bsky.notification.defs#preferences/repost>
        a            owl:ObjectProperty;
        rdfs:domain  <https://atproto.social/ontology/app.bsky.notification.defs#preferences>;
        rdfs:range   <https://atproto.social/ontology/app.bsky.notification.defs#filterablePreference> .

<https://atproto.social/ontology/app.bsky.notification.defs#preferences/starterpackJoined>
        a            owl:ObjectProperty;
        rdfs:domain  <https://atproto.social/ontology/app.bsky.notification.defs#preferences>;
        rdfs:range   <https://atproto.social/ontology/app.bsky.notification.defs#preference> .

<https://atproto.social/ontology/app.bsky.notification.defs#preferences/verified>
        a            owl:ObjectProperty;
        rdfs:domain  <https://atproto.social/ontology/app.bsky.notification.defs#preferences>;
        rdfs:range   <https://atproto.social/ontology/app.bsky.notification.defs#preference> .

<https://atproto.social/ontology/app.bsky.notification.defs#preferences/chat>
        a            owl:ObjectProperty;
        rdfs:domain  <https://atproto.social/ontology/app.bsky.notification.defs#preferences>;
        rdfs:range   <https://atproto.social/ontology/app.bsky.notification.defs#chatPreference> .

<https://atproto.social/ontology/app.bsky.notification.defs#activitySubscription>
        a       owl:Class .

<https://atproto.social/ontology/app.bsky.notification.defs#activitySubscription/reply>
        a            owl:DatatypeProperty;
        rdfs:domain  <https://atproto.social/ontology/app.bsky.notification.defs#activitySubscription>;
        rdfs:range   <xsd:boolean> .

<https://atproto.social/ontology/app.bsky.notification.defs#activitySubscription/post>
        a            owl:DatatypeProperty;
        rdfs:domain  <https://atproto.social/ontology/app.bsky.notification.defs#activitySubscription>;
        rdfs:range   <xsd:boolean> .

<https://atproto.social/ontology/app.bsky.notification.defs#subjectActivitySubscription>
        a             owl:Class;
        rdfs:comment  "Object used to store activity subscription data in stash." .

<https://atproto.social/ontology/app.bsky.notification.defs#subjectActivitySubscription/subject>
        a            owl:DatatypeProperty;
        rdfs:domain  <https://atproto.social/ontology/app.bsky.notification.defs#subjectActivitySubscription>;
        rdfs:range   <xsd:string> .

<https://atproto.social/ontology/app.bsky.notification.defs#subjectActivitySubscription/activitySubscription>
        a            owl:ObjectProperty;
        rdfs:domain  <https://atproto.social/ontology/app.bsky.notification.defs#subjectActivitySubscription>;
        rdfs:range   <https://atproto.social/ontology/app.bsky.notification.defs#activitySubscription> .

<https://atproto.social/ontology/app.bsky.notification.getPreferences#main>
        a             owl:Class;
        rdfs:comment  "Get notification-related preferences for an account. Requires auth." .

<https://atproto.social/ontology/app.bsky.notification.getUnreadCount#main>
        a             owl:Class;
        rdfs:comment  "Count the number of unread notifications for the requesting account. Requires auth." .

<https://atproto.social/ontology/app.bsky.notification.listActivitySubscriptions#main>
        a             owl:Class;
        rdfs:comment  "Enumerate all accounts to which the requesting account is subscribed to receive notifications for. Requires auth." .

<https://atproto.social/ontology/app.bsky.notification.listNotifications#main>
        a             owl:Class;
        rdfs:comment  "Enumerate notifications for the requesting account. Requires auth." .

<https://atproto.social/ontology/app.bsky.notification.listNotifications#notification>
        a       owl:Class .

<https://atproto.social/ontology/app.bsky.notification.listNotifications#notification/uri>
        a            owl:DatatypeProperty;
        rdfs:domain  <https://atproto.social/ontology/app.bsky.notification.listNotifications#notification>;
        rdfs:range   <xsd:string> .

<https://atproto.social/ontology/app.bsky.notification.listNotifications#notification/author>
        a            owl:ObjectProperty;
        rdfs:domain  <https://atproto.social/ontology/app.bsky.notification.listNotifications#notification>;
        rdfs:range   <https://atproto.social/ontology/app.bsky.actor.defs#profileView> .

<https://atproto.social/ontology/app.bsky.notification.listNotifications#notification/reason>
        a             owl:DatatypeProperty;
        rdfs:domain   <https://atproto.social/ontology/app.bsky.notification.listNotifications#notification>;
        rdfs:range    <xsd:string>;
        rdfs:comment  "The reason why this notification was delivered - e.g. your post was liked, or you received a new follower." .

<https://atproto.social/ontology/app.bsky.notification.listNotifications#notification/reasonSubject>
        a            owl:DatatypeProperty;
        rdfs:domain  <https://atproto.social/ontology/app.bsky.notification.listNotifications#notification>;
        rdfs:range   <xsd:string> .

<https://atproto.social/ontology/app.bsky.notification.listNotifications#notification/isRead>
        a            owl:DatatypeProperty;
        rdfs:domain  <https://atproto.social/ontology/app.bsky.notification.listNotifications#notification>;
        rdfs:range   <xsd:boolean> .

<https://atproto.social/ontology/app.bsky.notification.listNotifications#notification/indexedAt>
        a            owl:DatatypeProperty;
        rdfs:domain  <https://atproto.social/ontology/app.bsky.notification.listNotifications#notification>;
        rdfs:range   <xsd:string> .

<https://atproto.social/ontology/app.bsky.notification.listNotifications#notification/labels>
        a            owl:ObjectProperty;
        rdfs:domain  <https://atproto.social/ontology/app.bsky.notification.listNotifications#notification>;
        rdfs:range   <https://atproto.social/ontology/com.atproto.label.defs#label> .

<https://atproto.social/ontology/app.bsky.notification.listNotifications#notification/cid>
        a            owl:DatatypeProperty;
        rdfs:domain  <https://atproto.social/ontology/app.bsky.notification.listNotifications#notification>;
        rdfs:range   <xsd:string> .

<https://atproto.social/ontology/app.bsky.notification.listNotifications#notification/record>
        a            owl:ObjectProperty;
        rdfs:domain  <https://atproto.social/ontology/app.bsky.notification.listNotifications#notification> .

<https://atproto.social/ontology/app.bsky.notification.putActivitySubscription#main>
        a             owl:Class;
        rdfs:comment  "Puts an activity subscription entry. The key should be omitted for creation and provided for updates. Requires auth." .

<https://atproto.social/ontology/app.bsky.notification.putPreferences#main>
        a             owl:Class;
        rdfs:comment  "Set notification-related preferences for an account. Requires auth." .

<https://atproto.social/ontology/app.bsky.notification.putPreferencesV2#main>
        a             owl:Class;
        rdfs:comment  "Set notification-related preferences for an account. Requires auth." .

<https://atproto.social/ontology/app.bsky.notification.registerPush#main>
        a             owl:Class;
        rdfs:comment  "Register to receive push notifications, via a specified service, for the requesting account. Requires auth." .

<https://atproto.social/ontology/app.bsky.notification.updateSeen#main>
        a             owl:Class;
        rdfs:comment  "Notify server that the requesting account has seen notifications. Requires auth." .

<https://atproto.social/ontology/app.bsky.richtext.facet#mention>
        a             owl:Class;
        rdfs:comment  "Facet feature for mention of another account. The text is usually a handle, including a '@' prefix, but the facet reference is a DID." .

<https://atproto.social/ontology/app.bsky.richtext.facet#mention/did>
        a            owl:DatatypeProperty;
        rdfs:domain  <https://atproto.social/ontology/app.bsky.richtext.facet#mention>;
        rdfs:range   <xsd:string> .

<https://atproto.social/ontology/app.bsky.richtext.facet#link>
        a             owl:Class;
        rdfs:comment  "Facet feature for a URL. The text URL may have been simplified or truncated, but the facet reference should be a complete URL." .

<https://atproto.social/ontology/app.bsky.richtext.facet#link/uri>
        a            owl:DatatypeProperty;
        rdfs:domain  <https://atproto.social/ontology/app.bsky.richtext.facet#link>;
        rdfs:range   <xsd:string> .

<https://atproto.social/ontology/app.bsky.richtext.facet#tag>
        a             owl:Class;
        rdfs:comment  "Facet feature for a hashtag. The text usually includes a '#' prefix, but the facet reference should not (except in the case of 'double hash tags')." .

<https://atproto.social/ontology/app.bsky.richtext.facet#tag/tag>
        a            owl:DatatypeProperty;
        rdfs:domain  <https://atproto.social/ontology/app.bsky.richtext.facet#tag>;
        rdfs:range   <xsd:string> .

<https://atproto.social/ontology/app.bsky.richtext.facet#byteSlice>
        a             owl:Class;
        rdfs:comment  "Specifies the sub-string range a facet feature applies to. Start index is inclusive, end index is exclusive. Indices are zero-indexed, counting bytes of the UTF-8 encoded text. NOTE: some languages, like Javascript, use UTF-16 or Unicode codepoints for string slice indexing; in these languages, convert to byte arrays before working with facets." .

<https://atproto.social/ontology/app.bsky.richtext.facet#byteSlice/byteStart>
        a            owl:DatatypeProperty;
        rdfs:domain  <https://atproto.social/ontology/app.bsky.richtext.facet#byteSlice>;
        rdfs:range   <xsd:integer> .

<https://atproto.social/ontology/app.bsky.richtext.facet#byteSlice/byteEnd>
        a            owl:DatatypeProperty;
        rdfs:domain  <https://atproto.social/ontology/app.bsky.richtext.facet#byteSlice>;
        rdfs:range   <xsd:integer> .

<https://atproto.social/ontology/app.bsky.richtext.facet#main>
        a             owl:Class;
        rdfs:comment  "Annotation of a sub-string within rich text." .

<https://atproto.social/ontology/app.bsky.richtext.facet#main/index>
        a            owl:ObjectProperty;
        rdfs:domain  <https://atproto.social/ontology/app.bsky.richtext.facet#main>;
        rdfs:range   <https://atproto.social/ontology/app.bsky.richtext.facet#byteSlice> .

<https://atproto.social/ontology/app.bsky.richtext.facet#main/features>
        a            owl:ObjectProperty;
        rdfs:domain  <https://atproto.social/ontology/app.bsky.richtext.facet#main> .

<https://atproto.social/ontology/app.bsky.unspecced.defs#skeletonSearchStarterPack>
        a       owl:Class .

<https://atproto.social/ontology/app.bsky.unspecced.defs#skeletonSearchStarterPack/uri>
        a            owl:DatatypeProperty;
        rdfs:domain  <https://atproto.social/ontology/app.bsky.unspecced.defs#skeletonSearchStarterPack>;
        rdfs:range   <xsd:string> .

<https://atproto.social/ontology/app.bsky.unspecced.defs#trendingTopic>
        a       owl:Class .

<https://atproto.social/ontology/app.bsky.unspecced.defs#trendingTopic/topic>
        a            owl:DatatypeProperty;
        rdfs:domain  <https://atproto.social/ontology/app.bsky.unspecced.defs#trendingTopic>;
        rdfs:range   <xsd:string> .

<https://atproto.social/ontology/app.bsky.unspecced.defs#trendingTopic/displayName>
        a            owl:DatatypeProperty;
        rdfs:domain  <https://atproto.social/ontology/app.bsky.unspecced.defs#trendingTopic>;
        rdfs:range   <xsd:string> .

<https://atproto.social/ontology/app.bsky.unspecced.defs#trendingTopic/description>
        a            owl:DatatypeProperty;
        rdfs:domain  <https://atproto.social/ontology/app.bsky.unspecced.defs#trendingTopic>;
        rdfs:range   <xsd:string> .

<https://atproto.social/ontology/app.bsky.unspecced.defs#trendingTopic/link>
        a            owl:DatatypeProperty;
        rdfs:domain  <https://atproto.social/ontology/app.bsky.unspecced.defs#trendingTopic>;
        rdfs:range   <xsd:string> .

<https://atproto.social/ontology/app.bsky.unspecced.defs#threadItemNoUnauthenticated>
        a       owl:Class .

<https://atproto.social/ontology/app.bsky.unspecced.defs#threadItemNotFound>
        a       owl:Class .

<https://atproto.social/ontology/app.bsky.unspecced.defs#skeletonSearchPost>
        a       owl:Class .

<https://atproto.social/ontology/app.bsky.unspecced.defs#skeletonSearchPost/uri>
        a            owl:DatatypeProperty;
        rdfs:domain  <https://atproto.social/ontology/app.bsky.unspecced.defs#skeletonSearchPost>;
        rdfs:range   <xsd:string> .

<https://atproto.social/ontology/app.bsky.unspecced.defs#skeletonSearchActor>
        a       owl:Class .

<https://atproto.social/ontology/app.bsky.unspecced.defs#skeletonSearchActor/did>
        a            owl:DatatypeProperty;
        rdfs:domain  <https://atproto.social/ontology/app.bsky.unspecced.defs#skeletonSearchActor>;
        rdfs:range   <xsd:string> .

<https://atproto.social/ontology/app.bsky.unspecced.defs#skeletonTrend>
        a       owl:Class .

<https://atproto.social/ontology/app.bsky.unspecced.defs#skeletonTrend/dids>
        a            owl:DatatypeProperty;
        rdfs:domain  <https://atproto.social/ontology/app.bsky.unspecced.defs#skeletonTrend>;
        rdfs:range   <xsd:string> .

<https://atproto.social/ontology/app.bsky.unspecced.defs#skeletonTrend/topic>
        a            owl:DatatypeProperty;
        rdfs:domain  <https://atproto.social/ontology/app.bsky.unspecced.defs#skeletonTrend>;
        rdfs:range   <xsd:string> .

<https://atproto.social/ontology/app.bsky.unspecced.defs#skeletonTrend/displayName>
        a            owl:DatatypeProperty;
        rdfs:domain  <https://atproto.social/ontology/app.bsky.unspecced.defs#skeletonTrend>;
        rdfs:range   <xsd:string> .

<https://atproto.social/ontology/app.bsky.unspecced.defs#skeletonTrend/link>
        a            owl:DatatypeProperty;
        rdfs:domain  <https://atproto.social/ontology/app.bsky.unspecced.defs#skeletonTrend>;
        rdfs:range   <xsd:string> .

<https://atproto.social/ontology/app.bsky.unspecced.defs#skeletonTrend/startedAt>
        a            owl:DatatypeProperty;
        rdfs:domain  <https://atproto.social/ontology/app.bsky.unspecced.defs#skeletonTrend>;
        rdfs:range   <xsd:string> .

<https://atproto.social/ontology/app.bsky.unspecced.defs#skeletonTrend/postCount>
        a            owl:DatatypeProperty;
        rdfs:domain  <https://atproto.social/ontology/app.bsky.unspecced.defs#skeletonTrend>;
        rdfs:range   <xsd:integer> .

<https://atproto.social/ontology/app.bsky.unspecced.defs#skeletonTrend/status>
        a            owl:DatatypeProperty;
        rdfs:domain  <https://atproto.social/ontology/app.bsky.unspecced.defs#skeletonTrend>;
        rdfs:range   <xsd:string> .

<https://atproto.social/ontology/app.bsky.unspecced.defs#skeletonTrend/category>
        a            owl:DatatypeProperty;
        rdfs:domain  <https://atproto.social/ontology/app.bsky.unspecced.defs#skeletonTrend>;
        rdfs:range   <xsd:string> .

<https://atproto.social/ontology/app.bsky.unspecced.defs#trendView>
        a       owl:Class .

<https://atproto.social/ontology/app.bsky.unspecced.defs#trendView/displayName>
        a            owl:DatatypeProperty;
        rdfs:domain  <https://atproto.social/ontology/app.bsky.unspecced.defs#trendView>;
        rdfs:range   <xsd:string> .

<https://atproto.social/ontology/app.bsky.unspecced.defs#trendView/link>
        a            owl:DatatypeProperty;
        rdfs:domain  <https://atproto.social/ontology/app.bsky.unspecced.defs#trendView>;
        rdfs:range   <xsd:string> .

<https://atproto.social/ontology/app.bsky.unspecced.defs#trendView/startedAt>
        a            owl:DatatypeProperty;
        rdfs:domain  <https://atproto.social/ontology/app.bsky.unspecced.defs#trendView>;
        rdfs:range   <xsd:string> .

<https://atproto.social/ontology/app.bsky.unspecced.defs#trendView/postCount>
        a            owl:DatatypeProperty;
        rdfs:domain  <https://atproto.social/ontology/app.bsky.unspecced.defs#trendView>;
        rdfs:range   <xsd:integer> .

<https://atproto.social/ontology/app.bsky.unspecced.defs#trendView/status>
        a            owl:DatatypeProperty;
        rdfs:domain  <https://atproto.social/ontology/app.bsky.unspecced.defs#trendView>;
        rdfs:range   <xsd:string> .

<https://atproto.social/ontology/app.bsky.unspecced.defs#trendView/category>
        a            owl:DatatypeProperty;
        rdfs:domain  <https://atproto.social/ontology/app.bsky.unspecced.defs#trendView>;
        rdfs:range   <xsd:string> .

<https://atproto.social/ontology/app.bsky.unspecced.defs#trendView/actors>
        a            owl:ObjectProperty;
        rdfs:domain  <https://atproto.social/ontology/app.bsky.unspecced.defs#trendView>;
        rdfs:range   <https://atproto.social/ontology/app.bsky.actor.defs#profileViewBasic> .

<https://atproto.social/ontology/app.bsky.unspecced.defs#trendView/topic>
        a            owl:DatatypeProperty;
        rdfs:domain  <https://atproto.social/ontology/app.bsky.unspecced.defs#trendView>;
        rdfs:range   <xsd:string> .

<https://atproto.social/ontology/app.bsky.unspecced.defs#threadItemPost>
        a       owl:Class .

<https://atproto.social/ontology/app.bsky.unspecced.defs#threadItemPost/post>
        a            owl:ObjectProperty;
        rdfs:domain  <https://atproto.social/ontology/app.bsky.unspecced.defs#threadItemPost>;
        rdfs:range   <https://atproto.social/ontology/app.bsky.feed.defs#postView> .

<https://atproto.social/ontology/app.bsky.unspecced.defs#threadItemPost/moreParents>
        a             owl:DatatypeProperty;
        rdfs:domain   <https://atproto.social/ontology/app.bsky.unspecced.defs#threadItemPost>;
        rdfs:range    <xsd:boolean>;
        rdfs:comment  "This post has more parents that were not present in the response. This is just a boolean, without the number of parents." .

<https://atproto.social/ontology/app.bsky.unspecced.defs#threadItemPost/moreReplies>
        a             owl:DatatypeProperty;
        rdfs:domain   <https://atproto.social/ontology/app.bsky.unspecced.defs#threadItemPost>;
        rdfs:range    <xsd:integer>;
        rdfs:comment  "This post has more replies that were not present in the response. This is a numeric value, which is best-effort and might not be accurate." .

<https://atproto.social/ontology/app.bsky.unspecced.defs#threadItemPost/opThread>
        a             owl:DatatypeProperty;
        rdfs:domain   <https://atproto.social/ontology/app.bsky.unspecced.defs#threadItemPost>;
        rdfs:range    <xsd:boolean>;
        rdfs:comment  "This post is part of a contiguous thread by the OP from the thread root. Many different OP threads can happen in the same thread." .

<https://atproto.social/ontology/app.bsky.unspecced.defs#threadItemPost/hiddenByThreadgate>
        a             owl:DatatypeProperty;
        rdfs:domain   <https://atproto.social/ontology/app.bsky.unspecced.defs#threadItemPost>;
        rdfs:range    <xsd:boolean>;
        rdfs:comment  "The threadgate created by the author indicates this post as a reply to be hidden for everyone consuming the thread." .

<https://atproto.social/ontology/app.bsky.unspecced.defs#threadItemPost/mutedByViewer>
        a             owl:DatatypeProperty;
        rdfs:domain   <https://atproto.social/ontology/app.bsky.unspecced.defs#threadItemPost>;
        rdfs:range    <xsd:boolean>;
        rdfs:comment  "This is by an account muted by the viewer requesting it." .

<https://atproto.social/ontology/app.bsky.unspecced.defs#threadItemBlocked>
        a       owl:Class .

<https://atproto.social/ontology/app.bsky.unspecced.defs#threadItemBlocked/author>
        a            owl:ObjectProperty;
        rdfs:domain  <https://atproto.social/ontology/app.bsky.unspecced.defs#threadItemBlocked>;
        rdfs:range   <https://atproto.social/ontology/app.bsky.feed.defs#blockedAuthor> .

<https://atproto.social/ontology/app.bsky.unspecced.getConfig#main>
        a             owl:Class;
        rdfs:comment  "Get miscellaneous runtime configuration." .

<https://atproto.social/ontology/app.bsky.unspecced.getConfig#liveNowConfig>
        a       owl:Class .

<https://atproto.social/ontology/app.bsky.unspecced.getConfig#liveNowConfig/did>
        a            owl:DatatypeProperty;
        rdfs:domain  <https://atproto.social/ontology/app.bsky.unspecced.getConfig#liveNowConfig>;
        rdfs:range   <xsd:string> .

<https://atproto.social/ontology/app.bsky.unspecced.getConfig#liveNowConfig/domains>
        a            owl:DatatypeProperty;
        rdfs:domain  <https://atproto.social/ontology/app.bsky.unspecced.getConfig#liveNowConfig>;
        rdfs:range   <xsd:string> .

<https://atproto.social/ontology/app.bsky.unspecced.getPopularFeedGenerators#main>
        a             owl:Class;
        rdfs:comment  "An unspecced view of globally popular feed generators." .

<https://atproto.social/ontology/app.bsky.unspecced.getPostThreadOtherV2#threadItem>
        a       owl:Class .

<https://atproto.social/ontology/app.bsky.unspecced.getPostThreadOtherV2#threadItem/uri>
        a            owl:DatatypeProperty;
        rdfs:domain  <https://atproto.social/ontology/app.bsky.unspecced.getPostThreadOtherV2#threadItem>;
        rdfs:range   <xsd:string> .

<https://atproto.social/ontology/app.bsky.unspecced.getPostThreadOtherV2#threadItem/depth>
        a             owl:DatatypeProperty;
        rdfs:domain   <https://atproto.social/ontology/app.bsky.unspecced.getPostThreadOtherV2#threadItem>;
        rdfs:range    <xsd:integer>;
        rdfs:comment  "The nesting level of this item in the thread. Depth 0 means the anchor item. Items above have negative depths, items below have positive depths." .

<https://atproto.social/ontology/app.bsky.unspecced.getPostThreadOtherV2#threadItem/value>
        a            owl:ObjectProperty;
        rdfs:domain  <https://atproto.social/ontology/app.bsky.unspecced.getPostThreadOtherV2#threadItem> .

<https://atproto.social/ontology/app.bsky.unspecced.getPostThreadOtherV2#main>
        a             owl:Class;
        rdfs:comment  "(NOTE: this endpoint is under development and WILL change without notice. Don't use it until it is moved out of `unspecced` or your application WILL break) Get additional posts under a thread e.g. replies hidden by threadgate. Based on an anchor post at any depth of the tree, returns top-level replies below that anchor. It does not include ancestors nor the anchor itself. This should be called after exhausting `app.bsky.unspecced.getPostThreadV2`. Does not require auth, but additional metadata and filtering will be applied for authed requests." .

<https://atproto.social/ontology/app.bsky.unspecced.getPostThreadV2#main>
        a             owl:Class;
        rdfs:comment  "(NOTE: this endpoint is under development and WILL change without notice. Don't use it until it is moved out of `unspecced` or your application WILL break) Get posts in a thread. It is based in an anchor post at any depth of the tree, and returns posts above it (recursively resolving the parent, without further branching to their replies) and below it (recursive replies, with branching to their replies). Does not require auth, but additional metadata and filtering will be applied for authed requests." .

<https://atproto.social/ontology/app.bsky.unspecced.getPostThreadV2#threadItem>
        a       owl:Class .

<https://atproto.social/ontology/app.bsky.unspecced.getPostThreadV2#threadItem/uri>
        a            owl:DatatypeProperty;
        rdfs:domain  <https://atproto.social/ontology/app.bsky.unspecced.getPostThreadV2#threadItem>;
        rdfs:range   <xsd:string> .

<https://atproto.social/ontology/app.bsky.unspecced.getPostThreadV2#threadItem/depth>
        a             owl:DatatypeProperty;
        rdfs:domain   <https://atproto.social/ontology/app.bsky.unspecced.getPostThreadV2#threadItem>;
        rdfs:range    <xsd:integer>;
        rdfs:comment  "The nesting level of this item in the thread. Depth 0 means the anchor item. Items above have negative depths, items below have positive depths." .

<https://atproto.social/ontology/app.bsky.unspecced.getPostThreadV2#threadItem/value>
        a            owl:ObjectProperty;
        rdfs:domain  <https://atproto.social/ontology/app.bsky.unspecced.getPostThreadV2#threadItem> .

<https://atproto.social/ontology/app.bsky.unspecced.getSuggestedFeeds#main>
        a             owl:Class;
        rdfs:comment  "Get a list of suggested feeds" .

<https://atproto.social/ontology/app.bsky.unspecced.getSuggestedFeedsSkeleton#main>
        a             owl:Class;
        rdfs:comment  "Get a skeleton of suggested feeds. Intended to be called and hydrated by app.bsky.unspecced.getSuggestedFeeds" .

<https://atproto.social/ontology/app.bsky.unspecced.getSuggestedStarterPacks#main>
        a             owl:Class;
        rdfs:comment  "Get a list of suggested starterpacks" .

<https://atproto.social/ontology/app.bsky.unspecced.getSuggestedStarterPacksSkeleton#main>
        a             owl:Class;
        rdfs:comment  "Get a skeleton of suggested starterpacks. Intended to be called and hydrated by app.bsky.unspecced.getSuggestedStarterpacks" .

<https://atproto.social/ontology/app.bsky.unspecced.getSuggestedUsers#main>
        a             owl:Class;
        rdfs:comment  "Get a list of suggested users" .

<https://atproto.social/ontology/app.bsky.unspecced.getSuggestedUsersSkeleton#main>
        a             owl:Class;
        rdfs:comment  "Get a skeleton of suggested users. Intended to be called and hydrated by app.bsky.unspecced.getSuggestedUsers" .

<https://atproto.social/ontology/app.bsky.unspecced.getSuggestionsSkeleton#main>
        a             owl:Class;
        rdfs:comment  "Get a skeleton of suggested actors. Intended to be called and then hydrated through app.bsky.actor.getSuggestions" .

<https://atproto.social/ontology/app.bsky.unspecced.getTaggedSuggestions#main>
        a             owl:Class;
        rdfs:comment  "Get a list of suggestions (feeds and users) tagged with categories" .

<https://atproto.social/ontology/app.bsky.unspecced.getTaggedSuggestions#suggestion>
        a       owl:Class .

<https://atproto.social/ontology/app.bsky.unspecced.getTaggedSuggestions#suggestion/subjectType>
        a            owl:DatatypeProperty;
        rdfs:domain  <https://atproto.social/ontology/app.bsky.unspecced.getTaggedSuggestions#suggestion>;
        rdfs:range   <xsd:string> .

<https://atproto.social/ontology/app.bsky.unspecced.getTaggedSuggestions#suggestion/subject>
        a            owl:DatatypeProperty;
        rdfs:domain  <https://atproto.social/ontology/app.bsky.unspecced.getTaggedSuggestions#suggestion>;
        rdfs:range   <xsd:string> .

<https://atproto.social/ontology/app.bsky.unspecced.getTaggedSuggestions#suggestion/tag>
        a            owl:DatatypeProperty;
        rdfs:domain  <https://atproto.social/ontology/app.bsky.unspecced.getTaggedSuggestions#suggestion>;
        rdfs:range   <xsd:string> .

<https://atproto.social/ontology/app.bsky.unspecced.getTrendingTopics#main>
        a             owl:Class;
        rdfs:comment  "Get a list of trending topics" .

<https://atproto.social/ontology/app.bsky.unspecced.getTrends#main>
        a             owl:Class;
        rdfs:comment  "Get the current trends on the network" .

<https://atproto.social/ontology/app.bsky.unspecced.getTrendsSkeleton#main>
        a             owl:Class;
        rdfs:comment  "Get the skeleton of trends on the network. Intended to be called and then hydrated through app.bsky.unspecced.getTrends" .

<https://atproto.social/ontology/app.bsky.unspecced.searchActorsSkeleton#main>
        a             owl:Class;
        rdfs:comment  "Backend Actors (profile) search, returns only skeleton." .

<https://atproto.social/ontology/app.bsky.unspecced.searchPostsSkeleton#main>
        a             owl:Class;
        rdfs:comment  "Backend Posts search, returns only skeleton" .

<https://atproto.social/ontology/app.bsky.unspecced.searchStarterPacksSkeleton#main>
        a             owl:Class;
        rdfs:comment  "Backend Starter Pack search, returns only skeleton." .

<https://atproto.social/ontology/app.bsky.video.defs#jobStatus>
        a       owl:Class .

<https://atproto.social/ontology/app.bsky.video.defs#jobStatus/jobId>
        a            owl:DatatypeProperty;
        rdfs:domain  <https://atproto.social/ontology/app.bsky.video.defs#jobStatus>;
        rdfs:range   <xsd:string> .

<https://atproto.social/ontology/app.bsky.video.defs#jobStatus/did>
        a            owl:DatatypeProperty;
        rdfs:domain  <https://atproto.social/ontology/app.bsky.video.defs#jobStatus>;
        rdfs:range   <xsd:string> .

<https://atproto.social/ontology/app.bsky.video.defs#jobStatus/state>
        a             owl:DatatypeProperty;
        rdfs:domain   <https://atproto.social/ontology/app.bsky.video.defs#jobStatus>;
        rdfs:range    <xsd:string>;
        rdfs:comment  "The state of the video processing job. All values not listed as a known value indicate that the job is in process." .

<https://atproto.social/ontology/app.bsky.video.defs#jobStatus/progress>
        a             owl:DatatypeProperty;
        rdfs:domain   <https://atproto.social/ontology/app.bsky.video.defs#jobStatus>;
        rdfs:range    <xsd:integer>;
        rdfs:comment  "Progress within the current processing state." .

<https://atproto.social/ontology/app.bsky.video.defs#jobStatus/blob>
        a            owl:ObjectProperty;
        rdfs:domain  <https://atproto.social/ontology/app.bsky.video.defs#jobStatus> .

<https://atproto.social/ontology/app.bsky.video.defs#jobStatus/error>
        a            owl:DatatypeProperty;
        rdfs:domain  <https://atproto.social/ontology/app.bsky.video.defs#jobStatus>;
        rdfs:range   <xsd:string> .

<https://atproto.social/ontology/app.bsky.video.defs#jobStatus/message>
        a            owl:DatatypeProperty;
        rdfs:domain  <https://atproto.social/ontology/app.bsky.video.defs#jobStatus>;
        rdfs:range   <xsd:string> .

<https://atproto.social/ontology/app.bsky.video.getJobStatus#main>
        a             owl:Class;
        rdfs:comment  "Get status details for a video processing job." .

<https://atproto.social/ontology/app.bsky.video.getUploadLimits#main>
        a             owl:Class;
        rdfs:comment  "Get video upload limits for the authenticated user." .

<https://atproto.social/ontology/app.bsky.video.uploadVideo#main>
        a             owl:Class;
        rdfs:comment  "Upload a video to be processed then stored on the PDS." .

<https://atproto.social/ontology/chat.bsky.actor.declaration#main>
        a             owl:Class;
        rdfs:comment  "A declaration of a Bluesky chat account." .

<https://atproto.social/ontology/chat.bsky.actor.defs#profileViewBasic>
        a       owl:Class .

<https://atproto.social/ontology/chat.bsky.actor.defs#profileViewBasic/did>
        a            owl:DatatypeProperty;
        rdfs:domain  <https://atproto.social/ontology/chat.bsky.actor.defs#profileViewBasic>;
        rdfs:range   <xsd:string> .

<https://atproto.social/ontology/chat.bsky.actor.defs#profileViewBasic/handle>
        a            owl:DatatypeProperty;
        rdfs:domain  <https://atproto.social/ontology/chat.bsky.actor.defs#profileViewBasic>;
        rdfs:range   <xsd:string> .

<https://atproto.social/ontology/chat.bsky.actor.defs#profileViewBasic/labels>
        a            owl:ObjectProperty;
        rdfs:domain  <https://atproto.social/ontology/chat.bsky.actor.defs#profileViewBasic>;
        rdfs:range   <https://atproto.social/ontology/com.atproto.label.defs#label> .

<https://atproto.social/ontology/chat.bsky.actor.defs#profileViewBasic/chatDisabled>
        a             owl:DatatypeProperty;
        rdfs:domain   <https://atproto.social/ontology/chat.bsky.actor.defs#profileViewBasic>;
        rdfs:range    <xsd:boolean>;
        rdfs:comment  "Set to true when the actor cannot actively participate in conversations" .

<https://atproto.social/ontology/chat.bsky.actor.defs#profileViewBasic/verification>
        a            owl:ObjectProperty;
        rdfs:domain  <https://atproto.social/ontology/chat.bsky.actor.defs#profileViewBasic>;
        rdfs:range   <https://atproto.social/ontology/app.bsky.actor.defs#verificationState> .

<https://atproto.social/ontology/chat.bsky.actor.defs#profileViewBasic/displayName>
        a            owl:DatatypeProperty;
        rdfs:domain  <https://atproto.social/ontology/chat.bsky.actor.defs#profileViewBasic>;
        rdfs:range   <xsd:string> .

<https://atproto.social/ontology/chat.bsky.actor.defs#profileViewBasic/avatar>
        a            owl:DatatypeProperty;
        rdfs:domain  <https://atproto.social/ontology/chat.bsky.actor.defs#profileViewBasic>;
        rdfs:range   <xsd:string> .

<https://atproto.social/ontology/chat.bsky.actor.defs#profileViewBasic/associated>
        a            owl:ObjectProperty;
        rdfs:domain  <https://atproto.social/ontology/chat.bsky.actor.defs#profileViewBasic>;
        rdfs:range   <https://atproto.social/ontology/app.bsky.actor.defs#profileAssociated> .

<https://atproto.social/ontology/chat.bsky.actor.defs#profileViewBasic/viewer>
        a            owl:ObjectProperty;
        rdfs:domain  <https://atproto.social/ontology/chat.bsky.actor.defs#profileViewBasic>;
        rdfs:range   <https://atproto.social/ontology/app.bsky.actor.defs#viewerState> .

<https://atproto.social/ontology/chat.bsky.actor.deleteAccount#main>
        a       owl:Class .

<https://atproto.social/ontology/chat.bsky.actor.exportAccountData#main>
        a       owl:Class .

<https://atproto.social/ontology/chat.bsky.convo.acceptConvo#main>
        a       owl:Class .

<https://atproto.social/ontology/chat.bsky.convo.addReaction#main>
        a             owl:Class;
        rdfs:comment  "Adds an emoji reaction to a message. Requires authentication. It is idempotent, so multiple calls from the same user with the same emoji result in a single reaction." .

<https://atproto.social/ontology/chat.bsky.convo.defs#reactionView>
        a       owl:Class .

<https://atproto.social/ontology/chat.bsky.convo.defs#reactionView/value>
        a            owl:DatatypeProperty;
        rdfs:domain  <https://atproto.social/ontology/chat.bsky.convo.defs#reactionView>;
        rdfs:range   <xsd:string> .

<https://atproto.social/ontology/chat.bsky.convo.defs#reactionView/sender>
        a            owl:ObjectProperty;
        rdfs:domain  <https://atproto.social/ontology/chat.bsky.convo.defs#reactionView>;
        rdfs:range   <https://atproto.social/ontology/chat.bsky.convo.defs#reactionViewSender> .

<https://atproto.social/ontology/chat.bsky.convo.defs#reactionView/createdAt>
        a            owl:DatatypeProperty;
        rdfs:domain  <https://atproto.social/ontology/chat.bsky.convo.defs#reactionView>;
        rdfs:range   <xsd:string> .

<https://atproto.social/ontology/chat.bsky.convo.defs#reactionViewSender>
        a       owl:Class .

<https://atproto.social/ontology/chat.bsky.convo.defs#reactionViewSender/did>
        a            owl:DatatypeProperty;
        rdfs:domain  <https://atproto.social/ontology/chat.bsky.convo.defs#reactionViewSender>;
        rdfs:range   <xsd:string> .

<https://atproto.social/ontology/chat.bsky.convo.defs#messageAndReactionView>
        a       owl:Class .

<https://atproto.social/ontology/chat.bsky.convo.defs#messageAndReactionView/message>
        a            owl:ObjectProperty;
        rdfs:domain  <https://atproto.social/ontology/chat.bsky.convo.defs#messageAndReactionView>;
        rdfs:range   <https://atproto.social/ontology/chat.bsky.convo.defs#messageView> .

<https://atproto.social/ontology/chat.bsky.convo.defs#messageAndReactionView/reaction>
        a            owl:ObjectProperty;
        rdfs:domain  <https://atproto.social/ontology/chat.bsky.convo.defs#messageAndReactionView>;
        rdfs:range   <https://atproto.social/ontology/chat.bsky.convo.defs#reactionView> .

<https://atproto.social/ontology/chat.bsky.convo.defs#logLeaveConvo>
        a       owl:Class .

<https://atproto.social/ontology/chat.bsky.convo.defs#logLeaveConvo/rev>
        a            owl:DatatypeProperty;
        rdfs:domain  <https://atproto.social/ontology/chat.bsky.convo.defs#logLeaveConvo>;
        rdfs:range   <xsd:string> .

<https://atproto.social/ontology/chat.bsky.convo.defs#logLeaveConvo/convoId>
        a            owl:DatatypeProperty;
        rdfs:domain  <https://atproto.social/ontology/chat.bsky.convo.defs#logLeaveConvo>;
        rdfs:range   <xsd:string> .

<https://atproto.social/ontology/chat.bsky.convo.defs#logUnmuteConvo>
        a       owl:Class .

<https://atproto.social/ontology/chat.bsky.convo.defs#logUnmuteConvo/rev>
        a            owl:DatatypeProperty;
        rdfs:domain  <https://atproto.social/ontology/chat.bsky.convo.defs#logUnmuteConvo>;
        rdfs:range   <xsd:string> .

<https://atproto.social/ontology/chat.bsky.convo.defs#logUnmuteConvo/convoId>
        a            owl:DatatypeProperty;
        rdfs:domain  <https://atproto.social/ontology/chat.bsky.convo.defs#logUnmuteConvo>;
        rdfs:range   <xsd:string> .

<https://atproto.social/ontology/chat.bsky.convo.defs#logCreateMessage>
        a       owl:Class .

<https://atproto.social/ontology/chat.bsky.convo.defs#logCreateMessage/rev>
        a            owl:DatatypeProperty;
        rdfs:domain  <https://atproto.social/ontology/chat.bsky.convo.defs#logCreateMessage>;
        rdfs:range   <xsd:string> .

<https://atproto.social/ontology/chat.bsky.convo.defs#logCreateMessage/convoId>
        a            owl:DatatypeProperty;
        rdfs:domain  <https://atproto.social/ontology/chat.bsky.convo.defs#logCreateMessage>;
        rdfs:range   <xsd:string> .

<https://atproto.social/ontology/chat.bsky.convo.defs#logCreateMessage/message>
        a            owl:ObjectProperty;
        rdfs:domain  <https://atproto.social/ontology/chat.bsky.convo.defs#logCreateMessage> .

<https://atproto.social/ontology/chat.bsky.convo.defs#logDeleteMessage>
        a       owl:Class .

<https://atproto.social/ontology/chat.bsky.convo.defs#logDeleteMessage/rev>
        a            owl:DatatypeProperty;
        rdfs:domain  <https://atproto.social/ontology/chat.bsky.convo.defs#logDeleteMessage>;
        rdfs:range   <xsd:string> .

<https://atproto.social/ontology/chat.bsky.convo.defs#logDeleteMessage/convoId>
        a            owl:DatatypeProperty;
        rdfs:domain  <https://atproto.social/ontology/chat.bsky.convo.defs#logDeleteMessage>;
        rdfs:range   <xsd:string> .

<https://atproto.social/ontology/chat.bsky.convo.defs#logDeleteMessage/message>
        a            owl:ObjectProperty;
        rdfs:domain  <https://atproto.social/ontology/chat.bsky.convo.defs#logDeleteMessage> .

<https://atproto.social/ontology/chat.bsky.convo.defs#logReadMessage>
        a       owl:Class .

<https://atproto.social/ontology/chat.bsky.convo.defs#logReadMessage/rev>
        a            owl:DatatypeProperty;
        rdfs:domain  <https://atproto.social/ontology/chat.bsky.convo.defs#logReadMessage>;
        rdfs:range   <xsd:string> .

<https://atproto.social/ontology/chat.bsky.convo.defs#logReadMessage/convoId>
        a            owl:DatatypeProperty;
        rdfs:domain  <https://atproto.social/ontology/chat.bsky.convo.defs#logReadMessage>;
        rdfs:range   <xsd:string> .

<https://atproto.social/ontology/chat.bsky.convo.defs#logReadMessage/message>
        a            owl:ObjectProperty;
        rdfs:domain  <https://atproto.social/ontology/chat.bsky.convo.defs#logReadMessage> .

<https://atproto.social/ontology/chat.bsky.convo.defs#messageRef>
        a       owl:Class .

<https://atproto.social/ontology/chat.bsky.convo.defs#messageRef/did>
        a            owl:DatatypeProperty;
        rdfs:domain  <https://atproto.social/ontology/chat.bsky.convo.defs#messageRef>;
        rdfs:range   <xsd:string> .

<https://atproto.social/ontology/chat.bsky.convo.defs#messageRef/convoId>
        a            owl:DatatypeProperty;
        rdfs:domain  <https://atproto.social/ontology/chat.bsky.convo.defs#messageRef>;
        rdfs:range   <xsd:string> .

<https://atproto.social/ontology/chat.bsky.convo.defs#messageRef/messageId>
        a            owl:DatatypeProperty;
        rdfs:domain  <https://atproto.social/ontology/chat.bsky.convo.defs#messageRef>;
        rdfs:range   <xsd:string> .

<https://atproto.social/ontology/chat.bsky.convo.defs#messageView>
        a       owl:Class .

<https://atproto.social/ontology/chat.bsky.convo.defs#messageView/text>
        a            owl:DatatypeProperty;
        rdfs:domain  <https://atproto.social/ontology/chat.bsky.convo.defs#messageView>;
        rdfs:range   <xsd:string> .

<https://atproto.social/ontology/chat.bsky.convo.defs#messageView/facets>
        a             owl:ObjectProperty;
        rdfs:domain   <https://atproto.social/ontology/chat.bsky.convo.defs#messageView>;
        rdfs:range    <https://atproto.social/ontology/chat.bsky.convo.defs#app.bsky.richtext.facet>;
        rdfs:comment  "Annotations of text (mentions, URLs, hashtags, etc)" .

<https://atproto.social/ontology/chat.bsky.convo.defs#messageView/embed>
        a            owl:ObjectProperty;
        rdfs:domain  <https://atproto.social/ontology/chat.bsky.convo.defs#messageView> .

<https://atproto.social/ontology/chat.bsky.convo.defs#messageView/reactions>
        a             owl:ObjectProperty;
        rdfs:domain   <https://atproto.social/ontology/chat.bsky.convo.defs#messageView>;
        rdfs:range    <https://atproto.social/ontology/chat.bsky.convo.defs#reactionView>;
        rdfs:comment  "Reactions to this message, in ascending order of creation time." .

<https://atproto.social/ontology/chat.bsky.convo.defs#messageView/sender>
        a            owl:ObjectProperty;
        rdfs:domain  <https://atproto.social/ontology/chat.bsky.convo.defs#messageView>;
        rdfs:range   <https://atproto.social/ontology/chat.bsky.convo.defs#messageViewSender> .

<https://atproto.social/ontology/chat.bsky.convo.defs#messageView/sentAt>
        a            owl:DatatypeProperty;
        rdfs:domain  <https://atproto.social/ontology/chat.bsky.convo.defs#messageView>;
        rdfs:range   <xsd:string> .

<https://atproto.social/ontology/chat.bsky.convo.defs#messageView/id>
        a            owl:DatatypeProperty;
        rdfs:domain  <https://atproto.social/ontology/chat.bsky.convo.defs#messageView>;
        rdfs:range   <xsd:string> .

<https://atproto.social/ontology/chat.bsky.convo.defs#messageView/rev>
        a            owl:DatatypeProperty;
        rdfs:domain  <https://atproto.social/ontology/chat.bsky.convo.defs#messageView>;
        rdfs:range   <xsd:string> .

<https://atproto.social/ontology/chat.bsky.convo.defs#logAddReaction>
        a       owl:Class .

<https://atproto.social/ontology/chat.bsky.convo.defs#logAddReaction/rev>
        a            owl:DatatypeProperty;
        rdfs:domain  <https://atproto.social/ontology/chat.bsky.convo.defs#logAddReaction>;
        rdfs:range   <xsd:string> .

<https://atproto.social/ontology/chat.bsky.convo.defs#logAddReaction/convoId>
        a            owl:DatatypeProperty;
        rdfs:domain  <https://atproto.social/ontology/chat.bsky.convo.defs#logAddReaction>;
        rdfs:range   <xsd:string> .

<https://atproto.social/ontology/chat.bsky.convo.defs#logAddReaction/message>
        a            owl:ObjectProperty;
        rdfs:domain  <https://atproto.social/ontology/chat.bsky.convo.defs#logAddReaction> .

<https://atproto.social/ontology/chat.bsky.convo.defs#logAddReaction/reaction>
        a            owl:ObjectProperty;
        rdfs:domain  <https://atproto.social/ontology/chat.bsky.convo.defs#logAddReaction>;
        rdfs:range   <https://atproto.social/ontology/chat.bsky.convo.defs#reactionView> .

<https://atproto.social/ontology/chat.bsky.convo.defs#deletedMessageView>
        a       owl:Class .

<https://atproto.social/ontology/chat.bsky.convo.defs#deletedMessageView/id>
        a            owl:DatatypeProperty;
        rdfs:domain  <https://atproto.social/ontology/chat.bsky.convo.defs#deletedMessageView>;
        rdfs:range   <xsd:string> .

<https://atproto.social/ontology/chat.bsky.convo.defs#deletedMessageView/rev>
        a            owl:DatatypeProperty;
        rdfs:domain  <https://atproto.social/ontology/chat.bsky.convo.defs#deletedMessageView>;
        rdfs:range   <xsd:string> .

<https://atproto.social/ontology/chat.bsky.convo.defs#deletedMessageView/sender>
        a            owl:ObjectProperty;
        rdfs:domain  <https://atproto.social/ontology/chat.bsky.convo.defs#deletedMessageView>;
        rdfs:range   <https://atproto.social/ontology/chat.bsky.convo.defs#messageViewSender> .

<https://atproto.social/ontology/chat.bsky.convo.defs#deletedMessageView/sentAt>
        a            owl:DatatypeProperty;
        rdfs:domain  <https://atproto.social/ontology/chat.bsky.convo.defs#deletedMessageView>;
        rdfs:range   <xsd:string> .

<https://atproto.social/ontology/chat.bsky.convo.defs#messageViewSender>
        a       owl:Class .

<https://atproto.social/ontology/chat.bsky.convo.defs#messageViewSender/did>
        a            owl:DatatypeProperty;
        rdfs:domain  <https://atproto.social/ontology/chat.bsky.convo.defs#messageViewSender>;
        rdfs:range   <xsd:string> .

<https://atproto.social/ontology/chat.bsky.convo.defs#convoView>
        a       owl:Class .

<https://atproto.social/ontology/chat.bsky.convo.defs#convoView/status>
        a            owl:DatatypeProperty;
        rdfs:domain  <https://atproto.social/ontology/chat.bsky.convo.defs#convoView>;
        rdfs:range   <xsd:string> .

<https://atproto.social/ontology/chat.bsky.convo.defs#convoView/unreadCount>
        a            owl:DatatypeProperty;
        rdfs:domain  <https://atproto.social/ontology/chat.bsky.convo.defs#convoView>;
        rdfs:range   <xsd:integer> .

<https://atproto.social/ontology/chat.bsky.convo.defs#convoView/id>
        a            owl:DatatypeProperty;
        rdfs:domain  <https://atproto.social/ontology/chat.bsky.convo.defs#convoView>;
        rdfs:range   <xsd:string> .

<https://atproto.social/ontology/chat.bsky.convo.defs#convoView/rev>
        a            owl:DatatypeProperty;
        rdfs:domain  <https://atproto.social/ontology/chat.bsky.convo.defs#convoView>;
        rdfs:range   <xsd:string> .

<https://atproto.social/ontology/chat.bsky.convo.defs#convoView/members>
        a            owl:ObjectProperty;
        rdfs:domain  <https://atproto.social/ontology/chat.bsky.convo.defs#convoView>;
        rdfs:range   <https://atproto.social/ontology/chat.bsky.actor.defs#profileViewBasic> .

<https://atproto.social/ontology/chat.bsky.convo.defs#convoView/lastMessage>
        a            owl:ObjectProperty;
        rdfs:domain  <https://atproto.social/ontology/chat.bsky.convo.defs#convoView> .

<https://atproto.social/ontology/chat.bsky.convo.defs#convoView/lastReaction>
        a            owl:ObjectProperty;
        rdfs:domain  <https://atproto.social/ontology/chat.bsky.convo.defs#convoView> .

<https://atproto.social/ontology/chat.bsky.convo.defs#convoView/muted>
        a            owl:DatatypeProperty;
        rdfs:domain  <https://atproto.social/ontology/chat.bsky.convo.defs#convoView>;
        rdfs:range   <xsd:boolean> .

<https://atproto.social/ontology/chat.bsky.convo.defs#logBeginConvo>
        a       owl:Class .

<https://atproto.social/ontology/chat.bsky.convo.defs#logBeginConvo/rev>
        a            owl:DatatypeProperty;
        rdfs:domain  <https://atproto.social/ontology/chat.bsky.convo.defs#logBeginConvo>;
        rdfs:range   <xsd:string> .

<https://atproto.social/ontology/chat.bsky.convo.defs#logBeginConvo/convoId>
        a            owl:DatatypeProperty;
        rdfs:domain  <https://atproto.social/ontology/chat.bsky.convo.defs#logBeginConvo>;
        rdfs:range   <xsd:string> .

<https://atproto.social/ontology/chat.bsky.convo.defs#logAcceptConvo>
        a       owl:Class .

<https://atproto.social/ontology/chat.bsky.convo.defs#logAcceptConvo/rev>
        a            owl:DatatypeProperty;
        rdfs:domain  <https://atproto.social/ontology/chat.bsky.convo.defs#logAcceptConvo>;
        rdfs:range   <xsd:string> .

<https://atproto.social/ontology/chat.bsky.convo.defs#logAcceptConvo/convoId>
        a            owl:DatatypeProperty;
        rdfs:domain  <https://atproto.social/ontology/chat.bsky.convo.defs#logAcceptConvo>;
        rdfs:range   <xsd:string> .

<https://atproto.social/ontology/chat.bsky.convo.defs#logMuteConvo>
        a       owl:Class .

<https://atproto.social/ontology/chat.bsky.convo.defs#logMuteConvo/rev>
        a            owl:DatatypeProperty;
        rdfs:domain  <https://atproto.social/ontology/chat.bsky.convo.defs#logMuteConvo>;
        rdfs:range   <xsd:string> .

<https://atproto.social/ontology/chat.bsky.convo.defs#logMuteConvo/convoId>
        a            owl:DatatypeProperty;
        rdfs:domain  <https://atproto.social/ontology/chat.bsky.convo.defs#logMuteConvo>;
        rdfs:range   <xsd:string> .

<https://atproto.social/ontology/chat.bsky.convo.defs#logRemoveReaction>
        a       owl:Class .

<https://atproto.social/ontology/chat.bsky.convo.defs#logRemoveReaction/rev>
        a            owl:DatatypeProperty;
        rdfs:domain  <https://atproto.social/ontology/chat.bsky.convo.defs#logRemoveReaction>;
        rdfs:range   <xsd:string> .

<https://atproto.social/ontology/chat.bsky.convo.defs#logRemoveReaction/convoId>
        a            owl:DatatypeProperty;
        rdfs:domain  <https://atproto.social/ontology/chat.bsky.convo.defs#logRemoveReaction>;
        rdfs:range   <xsd:string> .

<https://atproto.social/ontology/chat.bsky.convo.defs#logRemoveReaction/message>
        a            owl:ObjectProperty;
        rdfs:domain  <https://atproto.social/ontology/chat.bsky.convo.defs#logRemoveReaction> .

<https://atproto.social/ontology/chat.bsky.convo.defs#logRemoveReaction/reaction>
        a            owl:ObjectProperty;
        rdfs:domain  <https://atproto.social/ontology/chat.bsky.convo.defs#logRemoveReaction>;
        rdfs:range   <https://atproto.social/ontology/chat.bsky.convo.defs#reactionView> .

<https://atproto.social/ontology/chat.bsky.convo.defs#messageInput>
        a       owl:Class .

<https://atproto.social/ontology/chat.bsky.convo.defs#messageInput/text>
        a            owl:DatatypeProperty;
        rdfs:domain  <https://atproto.social/ontology/chat.bsky.convo.defs#messageInput>;
        rdfs:range   <xsd:string> .

<https://atproto.social/ontology/chat.bsky.convo.defs#messageInput/facets>
        a             owl:ObjectProperty;
        rdfs:domain   <https://atproto.social/ontology/chat.bsky.convo.defs#messageInput>;
        rdfs:range    <https://atproto.social/ontology/chat.bsky.convo.defs#app.bsky.richtext.facet>;
        rdfs:comment  "Annotations of text (mentions, URLs, hashtags, etc)" .

<https://atproto.social/ontology/chat.bsky.convo.defs#messageInput/embed>
        a            owl:ObjectProperty;
        rdfs:domain  <https://atproto.social/ontology/chat.bsky.convo.defs#messageInput> .

<https://atproto.social/ontology/chat.bsky.convo.deleteMessageForSelf#main>
        a       owl:Class .

<https://atproto.social/ontology/chat.bsky.convo.getConvo#main>
        a       owl:Class .

<https://atproto.social/ontology/chat.bsky.convo.getConvoAvailability#main>
        a             owl:Class;
        rdfs:comment  "Get whether the requester and the other members can chat. If an existing convo is found for these members, it is returned." .

<https://atproto.social/ontology/chat.bsky.convo.getConvoForMembers#main>
        a       owl:Class .

<https://atproto.social/ontology/chat.bsky.convo.getLog#main>
        a       owl:Class .

<https://atproto.social/ontology/chat.bsky.convo.getMessages#main>
        a       owl:Class .

<https://atproto.social/ontology/chat.bsky.convo.leaveConvo#main>
        a       owl:Class .

<https://atproto.social/ontology/chat.bsky.convo.listConvos#main>
        a       owl:Class .

<https://atproto.social/ontology/chat.bsky.convo.muteConvo#main>
        a       owl:Class .

<https://atproto.social/ontology/chat.bsky.convo.removeReaction#main>
        a             owl:Class;
        rdfs:comment  "Removes an emoji reaction from a message. Requires authentication. It is idempotent, so multiple calls from the same user with the same emoji result in that reaction not being present, even if it already wasn't." .

<https://atproto.social/ontology/chat.bsky.convo.sendMessage#main>
        a       owl:Class .

<https://atproto.social/ontology/chat.bsky.convo.sendMessageBatch#main>
        a       owl:Class .

<https://atproto.social/ontology/chat.bsky.convo.sendMessageBatch#batchItem>
        a       owl:Class .

<https://atproto.social/ontology/chat.bsky.convo.sendMessageBatch#batchItem/convoId>
        a            owl:DatatypeProperty;
        rdfs:domain  <https://atproto.social/ontology/chat.bsky.convo.sendMessageBatch#batchItem>;
        rdfs:range   <xsd:string> .

<https://atproto.social/ontology/chat.bsky.convo.sendMessageBatch#batchItem/message>
        a            owl:ObjectProperty;
        rdfs:domain  <https://atproto.social/ontology/chat.bsky.convo.sendMessageBatch#batchItem>;
        rdfs:range   <https://atproto.social/ontology/chat.bsky.convo.defs#messageInput> .

<https://atproto.social/ontology/chat.bsky.convo.unmuteConvo#main>
        a       owl:Class .

<https://atproto.social/ontology/chat.bsky.convo.updateAllRead#main>
        a       owl:Class .

<https://atproto.social/ontology/chat.bsky.convo.updateRead#main>
        a       owl:Class .

<https://atproto.social/ontology/chat.bsky.moderation.getActorMetadata#main>
        a       owl:Class .

<https://atproto.social/ontology/chat.bsky.moderation.getActorMetadata#metadata>
        a       owl:Class .

<https://atproto.social/ontology/chat.bsky.moderation.getActorMetadata#metadata/messagesReceived>
        a            owl:DatatypeProperty;
        rdfs:domain  <https://atproto.social/ontology/chat.bsky.moderation.getActorMetadata#metadata>;
        rdfs:range   <xsd:integer> .

<https://atproto.social/ontology/chat.bsky.moderation.getActorMetadata#metadata/convos>
        a            owl:DatatypeProperty;
        rdfs:domain  <https://atproto.social/ontology/chat.bsky.moderation.getActorMetadata#metadata>;
        rdfs:range   <xsd:integer> .

<https://atproto.social/ontology/chat.bsky.moderation.getActorMetadata#metadata/convosStarted>
        a            owl:DatatypeProperty;
        rdfs:domain  <https://atproto.social/ontology/chat.bsky.moderation.getActorMetadata#metadata>;
        rdfs:range   <xsd:integer> .

<https://atproto.social/ontology/chat.bsky.moderation.getActorMetadata#metadata/messagesSent>
        a            owl:DatatypeProperty;
        rdfs:domain  <https://atproto.social/ontology/chat.bsky.moderation.getActorMetadata#metadata>;
        rdfs:range   <xsd:integer> .

<https://atproto.social/ontology/chat.bsky.moderation.getMessageContext#main>
        a       owl:Class .

<https://atproto.social/ontology/chat.bsky.moderation.updateActorAccess#main>
        a       owl:Class .

<https://atproto.social/ontology/com.atproto.admin.defs#statusAttr>
        a       owl:Class .

<https://atproto.social/ontology/com.atproto.admin.defs#statusAttr/applied>
        a            owl:DatatypeProperty;
        rdfs:domain  <https://atproto.social/ontology/com.atproto.admin.defs#statusAttr>;
        rdfs:range   <xsd:boolean> .

<https://atproto.social/ontology/com.atproto.admin.defs#statusAttr/ref>
        a            owl:DatatypeProperty;
        rdfs:domain  <https://atproto.social/ontology/com.atproto.admin.defs#statusAttr>;
        rdfs:range   <xsd:string> .

<https://atproto.social/ontology/com.atproto.admin.defs#accountView>
        a       owl:Class .

<https://atproto.social/ontology/com.atproto.admin.defs#accountView/invitesDisabled>
        a            owl:DatatypeProperty;
        rdfs:domain  <https://atproto.social/ontology/com.atproto.admin.defs#accountView>;
        rdfs:range   <xsd:boolean> .

<https://atproto.social/ontology/com.atproto.admin.defs#accountView/inviteNote>
        a            owl:DatatypeProperty;
        rdfs:domain  <https://atproto.social/ontology/com.atproto.admin.defs#accountView>;
        rdfs:range   <xsd:string> .

<https://atproto.social/ontology/com.atproto.admin.defs#accountView/deactivatedAt>
        a            owl:DatatypeProperty;
        rdfs:domain  <https://atproto.social/ontology/com.atproto.admin.defs#accountView>;
        rdfs:range   <xsd:string> .

<https://atproto.social/ontology/com.atproto.admin.defs#accountView/indexedAt>
        a            owl:DatatypeProperty;
        rdfs:domain  <https://atproto.social/ontology/com.atproto.admin.defs#accountView>;
        rdfs:range   <xsd:string> .

<https://atproto.social/ontology/com.atproto.admin.defs#accountView/invites>
        a            owl:ObjectProperty;
        rdfs:domain  <https://atproto.social/ontology/com.atproto.admin.defs#accountView>;
        rdfs:range   <https://atproto.social/ontology/com.atproto.server.defs#inviteCode> .

<https://atproto.social/ontology/com.atproto.admin.defs#accountView/emailConfirmedAt>
        a            owl:DatatypeProperty;
        rdfs:domain  <https://atproto.social/ontology/com.atproto.admin.defs#accountView>;
        rdfs:range   <xsd:string> .

<https://atproto.social/ontology/com.atproto.admin.defs#accountView/threatSignatures>
        a            owl:ObjectProperty;
        rdfs:domain  <https://atproto.social/ontology/com.atproto.admin.defs#accountView>;
        rdfs:range   <https://atproto.social/ontology/com.atproto.admin.defs#threatSignature> .

<https://atproto.social/ontology/com.atproto.admin.defs#accountView/did>
        a            owl:DatatypeProperty;
        rdfs:domain  <https://atproto.social/ontology/com.atproto.admin.defs#accountView>;
        rdfs:range   <xsd:string> .

<https://atproto.social/ontology/com.atproto.admin.defs#accountView/handle>
        a            owl:DatatypeProperty;
        rdfs:domain  <https://atproto.social/ontology/com.atproto.admin.defs#accountView>;
        rdfs:range   <xsd:string> .

<https://atproto.social/ontology/com.atproto.admin.defs#accountView/email>
        a            owl:DatatypeProperty;
        rdfs:domain  <https://atproto.social/ontology/com.atproto.admin.defs#accountView>;
        rdfs:range   <xsd:string> .

<https://atproto.social/ontology/com.atproto.admin.defs#accountView/relatedRecords>
        a            owl:ObjectProperty;
        rdfs:domain  <https://atproto.social/ontology/com.atproto.admin.defs#accountView> .

<https://atproto.social/ontology/com.atproto.admin.defs#accountView/invitedBy>
        a            owl:ObjectProperty;
        rdfs:domain  <https://atproto.social/ontology/com.atproto.admin.defs#accountView>;
        rdfs:range   <https://atproto.social/ontology/com.atproto.server.defs#inviteCode> .

<https://atproto.social/ontology/com.atproto.admin.defs#repoRef>
        a       owl:Class .

<https://atproto.social/ontology/com.atproto.admin.defs#repoRef/did>
        a            owl:DatatypeProperty;
        rdfs:domain  <https://atproto.social/ontology/com.atproto.admin.defs#repoRef>;
        rdfs:range   <xsd:string> .

<https://atproto.social/ontology/com.atproto.admin.defs#repoBlobRef>
        a       owl:Class .

<https://atproto.social/ontology/com.atproto.admin.defs#repoBlobRef/did>
        a            owl:DatatypeProperty;
        rdfs:domain  <https://atproto.social/ontology/com.atproto.admin.defs#repoBlobRef>;
        rdfs:range   <xsd:string> .

<https://atproto.social/ontology/com.atproto.admin.defs#repoBlobRef/cid>
        a            owl:DatatypeProperty;
        rdfs:domain  <https://atproto.social/ontology/com.atproto.admin.defs#repoBlobRef>;
        rdfs:range   <xsd:string> .

<https://atproto.social/ontology/com.atproto.admin.defs#repoBlobRef/recordUri>
        a            owl:DatatypeProperty;
        rdfs:domain  <https://atproto.social/ontology/com.atproto.admin.defs#repoBlobRef>;
        rdfs:range   <xsd:string> .

<https://atproto.social/ontology/com.atproto.admin.defs#threatSignature>
        a       owl:Class .

<https://atproto.social/ontology/com.atproto.admin.defs#threatSignature/property>
        a            owl:DatatypeProperty;
        rdfs:domain  <https://atproto.social/ontology/com.atproto.admin.defs#threatSignature>;
        rdfs:range   <xsd:string> .

<https://atproto.social/ontology/com.atproto.admin.defs#threatSignature/value>
        a            owl:DatatypeProperty;
        rdfs:domain  <https://atproto.social/ontology/com.atproto.admin.defs#threatSignature>;
        rdfs:range   <xsd:string> .

<https://atproto.social/ontology/com.atproto.admin.deleteAccount#main>
        a             owl:Class;
        rdfs:comment  "Delete a user account as an administrator." .

<https://atproto.social/ontology/com.atproto.admin.disableAccountInvites#main>
        a             owl:Class;
        rdfs:comment  "Disable an account from receiving new invite codes, but does not invalidate existing codes." .

<https://atproto.social/ontology/com.atproto.admin.disableInviteCodes#main>
        a             owl:Class;
        rdfs:comment  "Disable some set of codes and/or all codes associated with a set of users." .

<https://atproto.social/ontology/com.atproto.admin.enableAccountInvites#main>
        a             owl:Class;
        rdfs:comment  "Re-enable an account's ability to receive invite codes." .

<https://atproto.social/ontology/com.atproto.admin.getAccountInfo#main>
        a             owl:Class;
        rdfs:comment  "Get details about an account." .

<https://atproto.social/ontology/com.atproto.admin.getAccountInfos#main>
        a             owl:Class;
        rdfs:comment  "Get details about some accounts." .

<https://atproto.social/ontology/com.atproto.admin.getInviteCodes#main>
        a             owl:Class;
        rdfs:comment  "Get an admin view of invite codes." .

<https://atproto.social/ontology/com.atproto.admin.getSubjectStatus#main>
        a             owl:Class;
        rdfs:comment  "Get the service-specific admin status of a subject (account, record, or blob)." .

<https://atproto.social/ontology/com.atproto.admin.searchAccounts#main>
        a             owl:Class;
        rdfs:comment  "Get list of accounts that matches your search query." .

<https://atproto.social/ontology/com.atproto.admin.sendEmail#main>
        a             owl:Class;
        rdfs:comment  "Send email to a user's account email address." .

<https://atproto.social/ontology/com.atproto.admin.updateAccountEmail#main>
        a             owl:Class;
        rdfs:comment  "Administrative action to update an account's email." .

<https://atproto.social/ontology/com.atproto.admin.updateAccountHandle#main>
        a             owl:Class;
        rdfs:comment  "Administrative action to update an account's handle." .

<https://atproto.social/ontology/com.atproto.admin.updateAccountPassword#main>
        a             owl:Class;
        rdfs:comment  "Update the password for a user account as an administrator." .

<https://atproto.social/ontology/com.atproto.admin.updateAccountSigningKey#main>
        a             owl:Class;
        rdfs:comment  "Administrative action to update an account's signing key in their Did document." .

<https://atproto.social/ontology/com.atproto.admin.updateSubjectStatus#main>
        a             owl:Class;
        rdfs:comment  "Update the service-specific admin status of a subject (account, record, or blob)." .

<https://atproto.social/ontology/com.atproto.identity.defs#identityInfo>
        a       owl:Class .

<https://atproto.social/ontology/com.atproto.identity.defs#identityInfo/handle>
        a             owl:DatatypeProperty;
        rdfs:domain   <https://atproto.social/ontology/com.atproto.identity.defs#identityInfo>;
        rdfs:range    <xsd:string>;
        rdfs:comment  "The validated handle of the account; or 'handle.invalid' if the handle did not bi-directionally match the DID document." .

<https://atproto.social/ontology/com.atproto.identity.defs#identityInfo/didDoc>
        a             owl:ObjectProperty;
        rdfs:domain   <https://atproto.social/ontology/com.atproto.identity.defs#identityInfo>;
        rdfs:comment  "The complete DID document for the identity." .

<https://atproto.social/ontology/com.atproto.identity.defs#identityInfo/did>
        a            owl:DatatypeProperty;
        rdfs:domain  <https://atproto.social/ontology/com.atproto.identity.defs#identityInfo>;
        rdfs:range   <xsd:string> .

<https://atproto.social/ontology/com.atproto.identity.getRecommendedDidCredentials#main>
        a             owl:Class;
        rdfs:comment  "Describe the credentials that should be included in the DID doc of an account that is migrating to this service." .

<https://atproto.social/ontology/com.atproto.identity.refreshIdentity#main>
        a             owl:Class;
        rdfs:comment  "Request that the server re-resolve an identity (DID and handle). The server may ignore this request, or require authentication, depending on the role, implementation, and policy of the server." .

<https://atproto.social/ontology/com.atproto.identity.requestPlcOperationSignature#main>
        a             owl:Class;
        rdfs:comment  "Request an email with a code to in order to request a signed PLC operation. Requires Auth." .

<https://atproto.social/ontology/com.atproto.identity.resolveDid#main>
        a             owl:Class;
        rdfs:comment  "Resolves DID to DID document. Does not bi-directionally verify handle." .

<https://atproto.social/ontology/com.atproto.identity.resolveHandle#main>
        a             owl:Class;
        rdfs:comment  "Resolves an atproto handle (hostname) to a DID. Does not necessarily bi-directionally verify against the the DID document." .

<https://atproto.social/ontology/com.atproto.identity.resolveIdentity#main>
        a             owl:Class;
        rdfs:comment  "Resolves an identity (DID or Handle) to a full identity (DID document and verified handle)." .

<https://atproto.social/ontology/com.atproto.identity.signPlcOperation#main>
        a             owl:Class;
        rdfs:comment  "Signs a PLC operation to update some value(s) in the requesting DID's document." .

<https://atproto.social/ontology/com.atproto.identity.submitPlcOperation#main>
        a             owl:Class;
        rdfs:comment  "Validates a PLC operation to ensure that it doesn't violate a service's constraints or get the identity into a bad state, then submits it to the PLC registry" .

<https://atproto.social/ontology/com.atproto.identity.updateHandle#main>
        a             owl:Class;
        rdfs:comment  "Updates the current account's handle. Verifies handle validity, and updates did:plc document if necessary. Implemented by PDS, and requires auth." .

<https://atproto.social/ontology/com.atproto.label.defs#selfLabels>
        a             owl:Class;
        rdfs:comment  "Metadata tags on an atproto record, published by the author within the record." .

<https://atproto.social/ontology/com.atproto.label.defs#selfLabels/values>
        a            owl:ObjectProperty;
        rdfs:domain  <https://atproto.social/ontology/com.atproto.label.defs#selfLabels>;
        rdfs:range   <https://atproto.social/ontology/com.atproto.label.defs#selfLabel> .

<https://atproto.social/ontology/com.atproto.label.defs#selfLabel>
        a             owl:Class;
        rdfs:comment  "Metadata tag on an atproto record, published by the author within the record. Note that schemas should use #selfLabels, not #selfLabel." .

<https://atproto.social/ontology/com.atproto.label.defs#selfLabel/val>
        a             owl:DatatypeProperty;
        rdfs:domain   <https://atproto.social/ontology/com.atproto.label.defs#selfLabel>;
        rdfs:range    <xsd:string>;
        rdfs:comment  "The short string name of the value or type of this label." .

<https://atproto.social/ontology/com.atproto.label.defs#labelValueDefinition>
        a             owl:Class;
        rdfs:comment  "Declares a label value and its expected interpretations and behaviors." .

<https://atproto.social/ontology/com.atproto.label.defs#labelValueDefinition/identifier>
        a             owl:DatatypeProperty;
        rdfs:domain   <https://atproto.social/ontology/com.atproto.label.defs#labelValueDefinition>;
        rdfs:range    <xsd:string>;
        rdfs:comment  "The value of the label being defined. Must only include lowercase ascii and the '-' character ([a-z-]+)." .

<https://atproto.social/ontology/com.atproto.label.defs#labelValueDefinition/severity>
        a             owl:DatatypeProperty;
        rdfs:domain   <https://atproto.social/ontology/com.atproto.label.defs#labelValueDefinition>;
        rdfs:range    <xsd:string>;
        rdfs:comment  "How should a client visually convey this label? 'inform' means neutral and informational; 'alert' means negative and warning; 'none' means show nothing." .

<https://atproto.social/ontology/com.atproto.label.defs#labelValueDefinition/blurs>
        a             owl:DatatypeProperty;
        rdfs:domain   <https://atproto.social/ontology/com.atproto.label.defs#labelValueDefinition>;
        rdfs:range    <xsd:string>;
        rdfs:comment  "What should this label hide in the UI, if applied? 'content' hides all of the target; 'media' hides the images/video/audio; 'none' hides nothing." .

<https://atproto.social/ontology/com.atproto.label.defs#labelValueDefinition/defaultSetting>
        a             owl:DatatypeProperty;
        rdfs:domain   <https://atproto.social/ontology/com.atproto.label.defs#labelValueDefinition>;
        rdfs:range    <xsd:string>;
        rdfs:comment  "The default setting for this label." .

<https://atproto.social/ontology/com.atproto.label.defs#labelValueDefinition/adultOnly>
        a             owl:DatatypeProperty;
        rdfs:domain   <https://atproto.social/ontology/com.atproto.label.defs#labelValueDefinition>;
        rdfs:range    <xsd:boolean>;
        rdfs:comment  "Does the user need to have adult content enabled in order to configure this label?" .

<https://atproto.social/ontology/com.atproto.label.defs#labelValueDefinition/locales>
        a            owl:ObjectProperty;
        rdfs:domain  <https://atproto.social/ontology/com.atproto.label.defs#labelValueDefinition>;
        rdfs:range   <https://atproto.social/ontology/com.atproto.label.defs#labelValueDefinitionStrings> .

<https://atproto.social/ontology/com.atproto.label.defs#labelValueDefinitionStrings>
        a             owl:Class;
        rdfs:comment  "Strings which describe the label in the UI, localized into a specific language." .

<https://atproto.social/ontology/com.atproto.label.defs#labelValueDefinitionStrings/lang>
        a             owl:DatatypeProperty;
        rdfs:domain   <https://atproto.social/ontology/com.atproto.label.defs#labelValueDefinitionStrings>;
        rdfs:range    <xsd:string>;
        rdfs:comment  "The code of the language these strings are written in." .

<https://atproto.social/ontology/com.atproto.label.defs#labelValueDefinitionStrings/name>
        a             owl:DatatypeProperty;
        rdfs:domain   <https://atproto.social/ontology/com.atproto.label.defs#labelValueDefinitionStrings>;
        rdfs:range    <xsd:string>;
        rdfs:comment  "A short human-readable name for the label." .

<https://atproto.social/ontology/com.atproto.label.defs#labelValueDefinitionStrings/description>
        a             owl:DatatypeProperty;
        rdfs:domain   <https://atproto.social/ontology/com.atproto.label.defs#labelValueDefinitionStrings>;
        rdfs:range    <xsd:string>;
        rdfs:comment  "A longer description of what the label means and why it might be applied." .

<https://atproto.social/ontology/com.atproto.label.defs#labelValue>
        a       owl:Class .

<https://atproto.social/ontology/com.atproto.label.defs#label>
        a             owl:Class;
        rdfs:comment  "Metadata tag on an atproto resource (eg, repo or record)." .

<https://atproto.social/ontology/com.atproto.label.defs#label/uri>
        a             owl:DatatypeProperty;
        rdfs:domain   <https://atproto.social/ontology/com.atproto.label.defs#label>;
        rdfs:range    <xsd:string>;
        rdfs:comment  "AT URI of the record, repository (account), or other resource that this label applies to." .

<https://atproto.social/ontology/com.atproto.label.defs#label/neg>
        a             owl:DatatypeProperty;
        rdfs:domain   <https://atproto.social/ontology/com.atproto.label.defs#label>;
        rdfs:range    <xsd:boolean>;
        rdfs:comment  "If true, this is a negation label, overwriting a previous label." .

<https://atproto.social/ontology/com.atproto.label.defs#label/cts>
        a             owl:DatatypeProperty;
        rdfs:domain   <https://atproto.social/ontology/com.atproto.label.defs#label>;
        rdfs:range    <xsd:string>;
        rdfs:comment  "Timestamp when this label was created." .

<https://atproto.social/ontology/com.atproto.label.defs#label/exp>
        a             owl:DatatypeProperty;
        rdfs:domain   <https://atproto.social/ontology/com.atproto.label.defs#label>;
        rdfs:range    <xsd:string>;
        rdfs:comment  "Timestamp at which this label expires (no longer applies)." .

<https://atproto.social/ontology/com.atproto.label.defs#label/ver>
        a             owl:DatatypeProperty;
        rdfs:domain   <https://atproto.social/ontology/com.atproto.label.defs#label>;
        rdfs:range    <xsd:integer>;
        rdfs:comment  "The AT Protocol version of the label object." .

<https://atproto.social/ontology/com.atproto.label.defs#label/src>
        a             owl:DatatypeProperty;
        rdfs:domain   <https://atproto.social/ontology/com.atproto.label.defs#label>;
        rdfs:range    <xsd:string>;
        rdfs:comment  "DID of the actor who created this label." .

<https://atproto.social/ontology/com.atproto.label.defs#label/cid>
        a             owl:DatatypeProperty;
        rdfs:domain   <https://atproto.social/ontology/com.atproto.label.defs#label>;
        rdfs:range    <xsd:string>;
        rdfs:comment  "Optionally, CID specifying the specific version of 'uri' resource this label applies to." .

<https://atproto.social/ontology/com.atproto.label.defs#label/val>
        a             owl:DatatypeProperty;
        rdfs:domain   <https://atproto.social/ontology/com.atproto.label.defs#label>;
        rdfs:range    <xsd:string>;
        rdfs:comment  "The short string name of the value or type of this label." .

<https://atproto.social/ontology/com.atproto.label.defs#label/sig>
        a             owl:ObjectProperty;
        rdfs:domain   <https://atproto.social/ontology/com.atproto.label.defs#label>;
        rdfs:comment  "Signature of dag-cbor encoded label." .

<https://atproto.social/ontology/com.atproto.label.queryLabels#main>
        a             owl:Class;
        rdfs:comment  "Find labels relevant to the provided AT-URI patterns. Public endpoint for moderation services, though may return different or additional results with auth." .

<https://atproto.social/ontology/com.atproto.label.subscribeLabels#labels>
        a       owl:Class .

<https://atproto.social/ontology/com.atproto.label.subscribeLabels#labels/seq>
        a            owl:DatatypeProperty;
        rdfs:domain  <https://atproto.social/ontology/com.atproto.label.subscribeLabels#labels>;
        rdfs:range   <xsd:integer> .

<https://atproto.social/ontology/com.atproto.label.subscribeLabels#labels/labels>
        a            owl:ObjectProperty;
        rdfs:domain  <https://atproto.social/ontology/com.atproto.label.subscribeLabels#labels>;
        rdfs:range   <https://atproto.social/ontology/com.atproto.label.defs#label> .

<https://atproto.social/ontology/com.atproto.label.subscribeLabels#info>
        a       owl:Class .

<https://atproto.social/ontology/com.atproto.label.subscribeLabels#info/message>
        a            owl:DatatypeProperty;
        rdfs:domain  <https://atproto.social/ontology/com.atproto.label.subscribeLabels#info>;
        rdfs:range   <xsd:string> .

<https://atproto.social/ontology/com.atproto.label.subscribeLabels#info/name>
        a            owl:DatatypeProperty;
        rdfs:domain  <https://atproto.social/ontology/com.atproto.label.subscribeLabels#info>;
        rdfs:range   <xsd:string> .

<https://atproto.social/ontology/com.atproto.label.subscribeLabels#main>
        a             owl:Class;
        rdfs:comment  "Subscribe to stream of labels (and negations). Public endpoint implemented by mod services. Uses same sequencing scheme as repo event stream." .

<https://atproto.social/ontology/com.atproto.lexicon.schema#main>
        a             owl:Class;
        rdfs:comment  "Representation of Lexicon schemas themselves, when published as atproto records. Note that the schema language is not defined in Lexicon; this meta schema currently only includes a single version field ('lexicon'). See the atproto specifications for description of the other expected top-level fields ('id', 'defs', etc)." .

<https://atproto.social/ontology/com.atproto.moderation.createReport#main>
        a             owl:Class;
        rdfs:comment  "Submit a moderation report regarding an atproto account or record. Implemented by moderation services (with PDS proxying), and requires auth." .

<https://atproto.social/ontology/com.atproto.moderation.defs#reasonType>
        a       owl:Class .

<https://atproto.social/ontology/com.atproto.moderation.defs#reasonViolation>
        a             owl:Class;
        rdfs:comment  "Direct violation of server rules, laws, terms of service" .

<https://atproto.social/ontology/com.atproto.moderation.defs#reasonMisleading>
        a             owl:Class;
        rdfs:comment  "Misleading identity, affiliation, or content" .

<https://atproto.social/ontology/com.atproto.moderation.defs#reasonOther>
        a             owl:Class;
        rdfs:comment  "Other: reports not falling under another report category" .

<https://atproto.social/ontology/com.atproto.moderation.defs#reasonAppeal>
        a             owl:Class;
        rdfs:comment  "Appeal: appeal a previously taken moderation action" .

<https://atproto.social/ontology/com.atproto.moderation.defs#reasonSpam>
        a             owl:Class;
        rdfs:comment  "Spam: frequent unwanted promotion, replies, mentions" .

<https://atproto.social/ontology/com.atproto.moderation.defs#reasonSexual>
        a             owl:Class;
        rdfs:comment  "Unwanted or mislabeled sexual content" .

<https://atproto.social/ontology/com.atproto.moderation.defs#reasonRude>
        a             owl:Class;
        rdfs:comment  "Rude, harassing, explicit, or otherwise unwelcoming behavior" .

<https://atproto.social/ontology/com.atproto.moderation.defs#subjectType>
        a             owl:Class;
        rdfs:comment  "Tag describing a type of subject that might be reported." .

<https://atproto.social/ontology/com.atproto.repo.applyWrites#main>
        a             owl:Class;
        rdfs:comment  "Apply a batch transaction of repository creates, updates, and deletes. Requires auth, implemented by PDS." .

<https://atproto.social/ontology/com.atproto.repo.applyWrites#create>
        a             owl:Class;
        rdfs:comment  "Operation which creates a new record." .

<https://atproto.social/ontology/com.atproto.repo.applyWrites#create/value>
        a            owl:ObjectProperty;
        rdfs:domain  <https://atproto.social/ontology/com.atproto.repo.applyWrites#create> .

<https://atproto.social/ontology/com.atproto.repo.applyWrites#create/collection>
        a            owl:DatatypeProperty;
        rdfs:domain  <https://atproto.social/ontology/com.atproto.repo.applyWrites#create>;
        rdfs:range   <xsd:string> .

<https://atproto.social/ontology/com.atproto.repo.applyWrites#create/rkey>
        a             owl:DatatypeProperty;
        rdfs:domain   <https://atproto.social/ontology/com.atproto.repo.applyWrites#create>;
        rdfs:range    <xsd:string>;
        rdfs:comment  "NOTE: maxLength is redundant with record-key format. Keeping it temporarily to ensure backwards compatibility." .

<https://atproto.social/ontology/com.atproto.repo.applyWrites#update>
        a             owl:Class;
        rdfs:comment  "Operation which updates an existing record." .

<https://atproto.social/ontology/com.atproto.repo.applyWrites#update/collection>
        a            owl:DatatypeProperty;
        rdfs:domain  <https://atproto.social/ontology/com.atproto.repo.applyWrites#update>;
        rdfs:range   <xsd:string> .

<https://atproto.social/ontology/com.atproto.repo.applyWrites#update/rkey>
        a            owl:DatatypeProperty;
        rdfs:domain  <https://atproto.social/ontology/com.atproto.repo.applyWrites#update>;
        rdfs:range   <xsd:string> .

<https://atproto.social/ontology/com.atproto.repo.applyWrites#update/value>
        a            owl:ObjectProperty;
        rdfs:domain  <https://atproto.social/ontology/com.atproto.repo.applyWrites#update> .

<https://atproto.social/ontology/com.atproto.repo.applyWrites#delete>
        a             owl:Class;
        rdfs:comment  "Operation which deletes an existing record." .

<https://atproto.social/ontology/com.atproto.repo.applyWrites#delete/collection>
        a            owl:DatatypeProperty;
        rdfs:domain  <https://atproto.social/ontology/com.atproto.repo.applyWrites#delete>;
        rdfs:range   <xsd:string> .

<https://atproto.social/ontology/com.atproto.repo.applyWrites#delete/rkey>
        a            owl:DatatypeProperty;
        rdfs:domain  <https://atproto.social/ontology/com.atproto.repo.applyWrites#delete>;
        rdfs:range   <xsd:string> .

<https://atproto.social/ontology/com.atproto.repo.applyWrites#createResult>
        a       owl:Class .

<https://atproto.social/ontology/com.atproto.repo.applyWrites#createResult/uri>
        a            owl:DatatypeProperty;
        rdfs:domain  <https://atproto.social/ontology/com.atproto.repo.applyWrites#createResult>;
        rdfs:range   <xsd:string> .

<https://atproto.social/ontology/com.atproto.repo.applyWrites#createResult/cid>
        a            owl:DatatypeProperty;
        rdfs:domain  <https://atproto.social/ontology/com.atproto.repo.applyWrites#createResult>;
        rdfs:range   <xsd:string> .

<https://atproto.social/ontology/com.atproto.repo.applyWrites#createResult/validationStatus>
        a            owl:DatatypeProperty;
        rdfs:domain  <https://atproto.social/ontology/com.atproto.repo.applyWrites#createResult>;
        rdfs:range   <xsd:string> .

<https://atproto.social/ontology/com.atproto.repo.applyWrites#updateResult>
        a       owl:Class .

<https://atproto.social/ontology/com.atproto.repo.applyWrites#updateResult/uri>
        a            owl:DatatypeProperty;
        rdfs:domain  <https://atproto.social/ontology/com.atproto.repo.applyWrites#updateResult>;
        rdfs:range   <xsd:string> .

<https://atproto.social/ontology/com.atproto.repo.applyWrites#updateResult/cid>
        a            owl:DatatypeProperty;
        rdfs:domain  <https://atproto.social/ontology/com.atproto.repo.applyWrites#updateResult>;
        rdfs:range   <xsd:string> .

<https://atproto.social/ontology/com.atproto.repo.applyWrites#updateResult/validationStatus>
        a            owl:DatatypeProperty;
        rdfs:domain  <https://atproto.social/ontology/com.atproto.repo.applyWrites#updateResult>;
        rdfs:range   <xsd:string> .

<https://atproto.social/ontology/com.atproto.repo.applyWrites#deleteResult>
        a       owl:Class .

<https://atproto.social/ontology/com.atproto.repo.createRecord#main>
        a             owl:Class;
        rdfs:comment  "Create a single new repository record. Requires auth, implemented by PDS." .

<https://atproto.social/ontology/com.atproto.repo.defs#commitMeta>
        a       owl:Class .

<https://atproto.social/ontology/com.atproto.repo.defs#commitMeta/cid>
        a            owl:DatatypeProperty;
        rdfs:domain  <https://atproto.social/ontology/com.atproto.repo.defs#commitMeta>;
        rdfs:range   <xsd:string> .

<https://atproto.social/ontology/com.atproto.repo.defs#commitMeta/rev>
        a            owl:DatatypeProperty;
        rdfs:domain  <https://atproto.social/ontology/com.atproto.repo.defs#commitMeta>;
        rdfs:range   <xsd:string> .

<https://atproto.social/ontology/com.atproto.repo.deleteRecord#main>
        a             owl:Class;
        rdfs:comment  "Delete a repository record, or ensure it doesn't exist. Requires auth, implemented by PDS." .

<https://atproto.social/ontology/com.atproto.repo.describeRepo#main>
        a             owl:Class;
        rdfs:comment  "Get information about an account and repository, including the list of collections. Does not require auth." .

<https://atproto.social/ontology/com.atproto.repo.getRecord#main>
        a             owl:Class;
        rdfs:comment  "Get a single record from a repository. Does not require auth." .

<https://atproto.social/ontology/com.atproto.repo.importRepo#main>
        a             owl:Class;
        rdfs:comment  "Import a repo in the form of a CAR file. Requires Content-Length HTTP header to be set." .

<https://atproto.social/ontology/com.atproto.repo.listMissingBlobs#recordBlob>
        a       owl:Class .

<https://atproto.social/ontology/com.atproto.repo.listMissingBlobs#recordBlob/cid>
        a            owl:DatatypeProperty;
        rdfs:domain  <https://atproto.social/ontology/com.atproto.repo.listMissingBlobs#recordBlob>;
        rdfs:range   <xsd:string> .

<https://atproto.social/ontology/com.atproto.repo.listMissingBlobs#recordBlob/recordUri>
        a            owl:DatatypeProperty;
        rdfs:domain  <https://atproto.social/ontology/com.atproto.repo.listMissingBlobs#recordBlob>;
        rdfs:range   <xsd:string> .

<https://atproto.social/ontology/com.atproto.repo.listMissingBlobs#main>
        a             owl:Class;
        rdfs:comment  "Returns a list of missing blobs for the requesting account. Intended to be used in the account migration flow." .

<https://atproto.social/ontology/com.atproto.repo.listRecords#main>
        a             owl:Class;
        rdfs:comment  "List a range of records in a repository, matching a specific collection. Does not require auth." .

<https://atproto.social/ontology/com.atproto.repo.listRecords#record>
        a       owl:Class .

<https://atproto.social/ontology/com.atproto.repo.listRecords#record/cid>
        a            owl:DatatypeProperty;
        rdfs:domain  <https://atproto.social/ontology/com.atproto.repo.listRecords#record>;
        rdfs:range   <xsd:string> .

<https://atproto.social/ontology/com.atproto.repo.listRecords#record/value>
        a            owl:ObjectProperty;
        rdfs:domain  <https://atproto.social/ontology/com.atproto.repo.listRecords#record> .

<https://atproto.social/ontology/com.atproto.repo.listRecords#record/uri>
        a            owl:DatatypeProperty;
        rdfs:domain  <https://atproto.social/ontology/com.atproto.repo.listRecords#record>;
        rdfs:range   <xsd:string> .

<https://atproto.social/ontology/com.atproto.repo.putRecord#main>
        a             owl:Class;
        rdfs:comment  "Write a repository record, creating or updating it as needed. Requires auth, implemented by PDS." .

<https://atproto.social/ontology/com.atproto.repo.strongRef#main>
        a       owl:Class .

<https://atproto.social/ontology/com.atproto.repo.strongRef#main/uri>
        a            owl:DatatypeProperty;
        rdfs:domain  <https://atproto.social/ontology/com.atproto.repo.strongRef#main>;
        rdfs:range   <xsd:string> .

<https://atproto.social/ontology/com.atproto.repo.strongRef#main/cid>
        a            owl:DatatypeProperty;
        rdfs:domain  <https://atproto.social/ontology/com.atproto.repo.strongRef#main>;
        rdfs:range   <xsd:string> .

<https://atproto.social/ontology/com.atproto.repo.uploadBlob#main>
        a             owl:Class;
        rdfs:comment  "Upload a new blob, to be referenced from a repository record. The blob will be deleted if it is not referenced within a time window (eg, minutes). Blob restrictions (mimetype, size, etc) are enforced when the reference is created. Requires auth, implemented by PDS." .

<https://atproto.social/ontology/com.atproto.server.activateAccount#main>
        a             owl:Class;
        rdfs:comment  "Activates a currently deactivated account. Used to finalize account migration after the account's repo is imported and identity is setup." .

<https://atproto.social/ontology/com.atproto.server.checkAccountStatus#main>
        a             owl:Class;
        rdfs:comment  "Returns the status of an account, especially as pertaining to import or recovery. Can be called many times over the course of an account migration. Requires auth and can only be called pertaining to oneself." .

<https://atproto.social/ontology/com.atproto.server.confirmEmail#main>
        a             owl:Class;
        rdfs:comment  "Confirm an email using a token from com.atproto.server.requestEmailConfirmation." .

<https://atproto.social/ontology/com.atproto.server.createAccount#main>
        a             owl:Class;
        rdfs:comment  "Create an account. Implemented by PDS." .

<https://atproto.social/ontology/com.atproto.server.createAppPassword#main>
        a             owl:Class;
        rdfs:comment  "Create an App Password." .

<https://atproto.social/ontology/com.atproto.server.createAppPassword#appPassword>
        a       owl:Class .

<https://atproto.social/ontology/com.atproto.server.createAppPassword#appPassword/privileged>
        a            owl:DatatypeProperty;
        rdfs:domain  <https://atproto.social/ontology/com.atproto.server.createAppPassword#appPassword>;
        rdfs:range   <xsd:boolean> .

<https://atproto.social/ontology/com.atproto.server.createAppPassword#appPassword/name>
        a            owl:DatatypeProperty;
        rdfs:domain  <https://atproto.social/ontology/com.atproto.server.createAppPassword#appPassword>;
        rdfs:range   <xsd:string> .

<https://atproto.social/ontology/com.atproto.server.createAppPassword#appPassword/password>
        a            owl:DatatypeProperty;
        rdfs:domain  <https://atproto.social/ontology/com.atproto.server.createAppPassword#appPassword>;
        rdfs:range   <xsd:string> .

<https://atproto.social/ontology/com.atproto.server.createAppPassword#appPassword/createdAt>
        a            owl:DatatypeProperty;
        rdfs:domain  <https://atproto.social/ontology/com.atproto.server.createAppPassword#appPassword>;
        rdfs:range   <xsd:string> .

<https://atproto.social/ontology/com.atproto.server.createInviteCode#main>
        a             owl:Class;
        rdfs:comment  "Create an invite code." .

<https://atproto.social/ontology/com.atproto.server.createInviteCodes#main>
        a             owl:Class;
        rdfs:comment  "Create invite codes." .

<https://atproto.social/ontology/com.atproto.server.createInviteCodes#accountCodes>
        a       owl:Class .

<https://atproto.social/ontology/com.atproto.server.createInviteCodes#accountCodes/account>
        a            owl:DatatypeProperty;
        rdfs:domain  <https://atproto.social/ontology/com.atproto.server.createInviteCodes#accountCodes>;
        rdfs:range   <xsd:string> .

<https://atproto.social/ontology/com.atproto.server.createInviteCodes#accountCodes/codes>
        a            owl:DatatypeProperty;
        rdfs:domain  <https://atproto.social/ontology/com.atproto.server.createInviteCodes#accountCodes>;
        rdfs:range   <xsd:string> .

<https://atproto.social/ontology/com.atproto.server.createSession#main>
        a             owl:Class;
        rdfs:comment  "Create an authentication session." .

<https://atproto.social/ontology/com.atproto.server.deactivateAccount#main>
        a             owl:Class;
        rdfs:comment  "Deactivates a currently active account. Stops serving of repo, and future writes to repo until reactivated. Used to finalize account migration with the old host after the account has been activated on the new host." .

<https://atproto.social/ontology/com.atproto.server.defs#inviteCode>
        a       owl:Class .

<https://atproto.social/ontology/com.atproto.server.defs#inviteCode/code>
        a            owl:DatatypeProperty;
        rdfs:domain  <https://atproto.social/ontology/com.atproto.server.defs#inviteCode>;
        rdfs:range   <xsd:string> .

<https://atproto.social/ontology/com.atproto.server.defs#inviteCode/available>
        a            owl:DatatypeProperty;
        rdfs:domain  <https://atproto.social/ontology/com.atproto.server.defs#inviteCode>;
        rdfs:range   <xsd:integer> .

<https://atproto.social/ontology/com.atproto.server.defs#inviteCode/disabled>
        a            owl:DatatypeProperty;
        rdfs:domain  <https://atproto.social/ontology/com.atproto.server.defs#inviteCode>;
        rdfs:range   <xsd:boolean> .

<https://atproto.social/ontology/com.atproto.server.defs#inviteCode/forAccount>
        a            owl:DatatypeProperty;
        rdfs:domain  <https://atproto.social/ontology/com.atproto.server.defs#inviteCode>;
        rdfs:range   <xsd:string> .

<https://atproto.social/ontology/com.atproto.server.defs#inviteCode/createdBy>
        a            owl:DatatypeProperty;
        rdfs:domain  <https://atproto.social/ontology/com.atproto.server.defs#inviteCode>;
        rdfs:range   <xsd:string> .

<https://atproto.social/ontology/com.atproto.server.defs#inviteCode/createdAt>
        a            owl:DatatypeProperty;
        rdfs:domain  <https://atproto.social/ontology/com.atproto.server.defs#inviteCode>;
        rdfs:range   <xsd:string> .

<https://atproto.social/ontology/com.atproto.server.defs#inviteCode/uses>
        a            owl:ObjectProperty;
        rdfs:domain  <https://atproto.social/ontology/com.atproto.server.defs#inviteCode>;
        rdfs:range   <https://atproto.social/ontology/com.atproto.server.defs#inviteCodeUse> .

<https://atproto.social/ontology/com.atproto.server.defs#inviteCodeUse>
        a       owl:Class .

<https://atproto.social/ontology/com.atproto.server.defs#inviteCodeUse/usedBy>
        a            owl:DatatypeProperty;
        rdfs:domain  <https://atproto.social/ontology/com.atproto.server.defs#inviteCodeUse>;
        rdfs:range   <xsd:string> .

<https://atproto.social/ontology/com.atproto.server.defs#inviteCodeUse/usedAt>
        a            owl:DatatypeProperty;
        rdfs:domain  <https://atproto.social/ontology/com.atproto.server.defs#inviteCodeUse>;
        rdfs:range   <xsd:string> .

<https://atproto.social/ontology/com.atproto.server.deleteAccount#main>
        a             owl:Class;
        rdfs:comment  "Delete an actor's account with a token and password. Can only be called after requesting a deletion token. Requires auth." .

<https://atproto.social/ontology/com.atproto.server.deleteSession#main>
        a             owl:Class;
        rdfs:comment  "Delete the current session. Requires auth." .

<https://atproto.social/ontology/com.atproto.server.describeServer#contact>
        a       owl:Class .

<https://atproto.social/ontology/com.atproto.server.describeServer#contact/email>
        a            owl:DatatypeProperty;
        rdfs:domain  <https://atproto.social/ontology/com.atproto.server.describeServer#contact>;
        rdfs:range   <xsd:string> .

<https://atproto.social/ontology/com.atproto.server.describeServer#main>
        a             owl:Class;
        rdfs:comment  "Describes the server's account creation requirements and capabilities. Implemented by PDS." .

<https://atproto.social/ontology/com.atproto.server.describeServer#links>
        a       owl:Class .

<https://atproto.social/ontology/com.atproto.server.describeServer#links/privacyPolicy>
        a            owl:DatatypeProperty;
        rdfs:domain  <https://atproto.social/ontology/com.atproto.server.describeServer#links>;
        rdfs:range   <xsd:string> .

<https://atproto.social/ontology/com.atproto.server.describeServer#links/termsOfService>
        a            owl:DatatypeProperty;
        rdfs:domain  <https://atproto.social/ontology/com.atproto.server.describeServer#links>;
        rdfs:range   <xsd:string> .

<https://atproto.social/ontology/com.atproto.server.getAccountInviteCodes#main>
        a             owl:Class;
        rdfs:comment  "Get all invite codes for the current account. Requires auth." .

<https://atproto.social/ontology/com.atproto.server.getServiceAuth#main>
        a             owl:Class;
        rdfs:comment  "Get a signed token on behalf of the requesting DID for the requested service." .

<https://atproto.social/ontology/com.atproto.server.getSession#main>
        a             owl:Class;
        rdfs:comment  "Get information about the current auth session. Requires auth." .

<https://atproto.social/ontology/com.atproto.server.listAppPasswords#main>
        a             owl:Class;
        rdfs:comment  "List all App Passwords." .

<https://atproto.social/ontology/com.atproto.server.listAppPasswords#appPassword>
        a       owl:Class .

<https://atproto.social/ontology/com.atproto.server.listAppPasswords#appPassword/name>
        a            owl:DatatypeProperty;
        rdfs:domain  <https://atproto.social/ontology/com.atproto.server.listAppPasswords#appPassword>;
        rdfs:range   <xsd:string> .

<https://atproto.social/ontology/com.atproto.server.listAppPasswords#appPassword/createdAt>
        a            owl:DatatypeProperty;
        rdfs:domain  <https://atproto.social/ontology/com.atproto.server.listAppPasswords#appPassword>;
        rdfs:range   <xsd:string> .

<https://atproto.social/ontology/com.atproto.server.listAppPasswords#appPassword/privileged>
        a            owl:DatatypeProperty;
        rdfs:domain  <https://atproto.social/ontology/com.atproto.server.listAppPasswords#appPassword>;
        rdfs:range   <xsd:boolean> .

<https://atproto.social/ontology/com.atproto.server.refreshSession#main>
        a             owl:Class;
        rdfs:comment  "Refresh an authentication session. Requires auth using the 'refreshJwt' (not the 'accessJwt')." .

<https://atproto.social/ontology/com.atproto.server.requestAccountDelete#main>
        a             owl:Class;
        rdfs:comment  "Initiate a user account deletion via email." .

<https://atproto.social/ontology/com.atproto.server.requestEmailConfirmation#main>
        a             owl:Class;
        rdfs:comment  "Request an email with a code to confirm ownership of email." .

<https://atproto.social/ontology/com.atproto.server.requestEmailUpdate#main>
        a             owl:Class;
        rdfs:comment  "Request a token in order to update email." .

<https://atproto.social/ontology/com.atproto.server.requestPasswordReset#main>
        a             owl:Class;
        rdfs:comment  "Initiate a user account password reset via email." .

<https://atproto.social/ontology/com.atproto.server.reserveSigningKey#main>
        a             owl:Class;
        rdfs:comment  "Reserve a repo signing key, for use with account creation. Necessary so that a DID PLC update operation can be constructed during an account migraiton. Public and does not require auth; implemented by PDS. NOTE: this endpoint may change when full account migration is implemented." .

<https://atproto.social/ontology/com.atproto.server.resetPassword#main>
        a             owl:Class;
        rdfs:comment  "Reset a user account password using a token." .

<https://atproto.social/ontology/com.atproto.server.revokeAppPassword#main>
        a             owl:Class;
        rdfs:comment  "Revoke an App Password by name." .

<https://atproto.social/ontology/com.atproto.server.updateEmail#main>
        a             owl:Class;
        rdfs:comment  "Update an account's email." .

<https://atproto.social/ontology/com.atproto.sync.defs#hostStatus>
        a       owl:Class .

<https://atproto.social/ontology/com.atproto.sync.getBlob#main>
        a             owl:Class;
        rdfs:comment  "Get a blob associated with a given account. Returns the full blob as originally uploaded. Does not require auth; implemented by PDS." .

<https://atproto.social/ontology/com.atproto.sync.getBlocks#main>
        a             owl:Class;
        rdfs:comment  "Get data blocks from a given repo, by CID. For example, intermediate MST nodes, or records. Does not require auth; implemented by PDS." .

<https://atproto.social/ontology/com.atproto.sync.getCheckout#main>
        a             owl:Class;
        rdfs:comment  "DEPRECATED - please use com.atproto.sync.getRepo instead" .

<https://atproto.social/ontology/com.atproto.sync.getHead#main>
        a             owl:Class;
        rdfs:comment  "DEPRECATED - please use com.atproto.sync.getLatestCommit instead" .

<https://atproto.social/ontology/com.atproto.sync.getHostStatus#main>
        a             owl:Class;
        rdfs:comment  "Returns information about a specified upstream host, as consumed by the server. Implemented by relays." .

<https://atproto.social/ontology/com.atproto.sync.getLatestCommit#main>
        a             owl:Class;
        rdfs:comment  "Get the current commit CID & revision of the specified repo. Does not require auth." .

<https://atproto.social/ontology/com.atproto.sync.getRecord#main>
        a             owl:Class;
        rdfs:comment  "Get data blocks needed to prove the existence or non-existence of record in the current version of repo. Does not require auth." .

<https://atproto.social/ontology/com.atproto.sync.getRepo#main>
        a             owl:Class;
        rdfs:comment  "Download a repository export as CAR file. Optionally only a 'diff' since a previous revision. Does not require auth; implemented by PDS." .

<https://atproto.social/ontology/com.atproto.sync.getRepoStatus#main>
        a             owl:Class;
        rdfs:comment  "Get the hosting status for a repository, on this server. Expected to be implemented by PDS and Relay." .

<https://atproto.social/ontology/com.atproto.sync.listBlobs#main>
        a             owl:Class;
        rdfs:comment  "List blob CIDs for an account, since some repo revision. Does not require auth; implemented by PDS." .

<https://atproto.social/ontology/com.atproto.sync.listHosts#main>
        a             owl:Class;
        rdfs:comment  "Enumerates upstream hosts (eg, PDS or relay instances) that this service consumes from. Implemented by relays." .

<https://atproto.social/ontology/com.atproto.sync.listHosts#host>
        a       owl:Class .

<https://atproto.social/ontology/com.atproto.sync.listHosts#host/hostname>
        a             owl:DatatypeProperty;
        rdfs:domain   <https://atproto.social/ontology/com.atproto.sync.listHosts#host>;
        rdfs:range    <xsd:string>;
        rdfs:comment  "hostname of server; not a URL (no scheme)" .

<https://atproto.social/ontology/com.atproto.sync.listHosts#host/seq>
        a             owl:DatatypeProperty;
        rdfs:domain   <https://atproto.social/ontology/com.atproto.sync.listHosts#host>;
        rdfs:range    <xsd:integer>;
        rdfs:comment  "Recent repo stream event sequence number. May be delayed from actual stream processing (eg, persisted cursor not in-memory cursor)." .

<https://atproto.social/ontology/com.atproto.sync.listHosts#host/accountCount>
        a            owl:DatatypeProperty;
        rdfs:domain  <https://atproto.social/ontology/com.atproto.sync.listHosts#host>;
        rdfs:range   <xsd:integer> .

<https://atproto.social/ontology/com.atproto.sync.listHosts#host/status>
        a            owl:ObjectProperty;
        rdfs:domain  <https://atproto.social/ontology/com.atproto.sync.listHosts#host>;
        rdfs:range   <https://atproto.social/ontology/com.atproto.sync.defs#hostStatus> .

<https://atproto.social/ontology/com.atproto.sync.listRepos#repo>
        a       owl:Class .

<https://atproto.social/ontology/com.atproto.sync.listRepos#repo/did>
        a            owl:DatatypeProperty;
        rdfs:domain  <https://atproto.social/ontology/com.atproto.sync.listRepos#repo>;
        rdfs:range   <xsd:string> .

<https://atproto.social/ontology/com.atproto.sync.listRepos#repo/head>
        a             owl:DatatypeProperty;
        rdfs:domain   <https://atproto.social/ontology/com.atproto.sync.listRepos#repo>;
        rdfs:range    <xsd:string>;
        rdfs:comment  "Current repo commit CID" .

<https://atproto.social/ontology/com.atproto.sync.listRepos#repo/rev>
        a            owl:DatatypeProperty;
        rdfs:domain  <https://atproto.social/ontology/com.atproto.sync.listRepos#repo>;
        rdfs:range   <xsd:string> .

<https://atproto.social/ontology/com.atproto.sync.listRepos#repo/active>
        a            owl:DatatypeProperty;
        rdfs:domain  <https://atproto.social/ontology/com.atproto.sync.listRepos#repo>;
        rdfs:range   <xsd:boolean> .

<https://atproto.social/ontology/com.atproto.sync.listRepos#repo/status>
        a             owl:DatatypeProperty;
        rdfs:domain   <https://atproto.social/ontology/com.atproto.sync.listRepos#repo>;
        rdfs:range    <xsd:string>;
        rdfs:comment  "If active=false, this optional field indicates a possible reason for why the account is not active. If active=false and no status is supplied, then the host makes no claim for why the repository is no longer being hosted." .

<https://atproto.social/ontology/com.atproto.sync.listRepos#main>
        a             owl:Class;
        rdfs:comment  "Enumerates all the DID, rev, and commit CID for all repos hosted by this service. Does not require auth; implemented by PDS and Relay." .

<https://atproto.social/ontology/com.atproto.sync.listReposByCollection#main>
        a             owl:Class;
        rdfs:comment  "Enumerates all the DIDs which have records with the given collection NSID." .

<https://atproto.social/ontology/com.atproto.sync.listReposByCollection#repo>
        a       owl:Class .

<https://atproto.social/ontology/com.atproto.sync.listReposByCollection#repo/did>
        a            owl:DatatypeProperty;
        rdfs:domain  <https://atproto.social/ontology/com.atproto.sync.listReposByCollection#repo>;
        rdfs:range   <xsd:string> .

<https://atproto.social/ontology/com.atproto.sync.notifyOfUpdate#main>
        a             owl:Class;
        rdfs:comment  "Notify a crawling service of a recent update, and that crawling should resume. Intended use is after a gap between repo stream events caused the crawling service to disconnect. Does not require auth; implemented by Relay. DEPRECATED: just use com.atproto.sync.requestCrawl" .

<https://atproto.social/ontology/com.atproto.sync.requestCrawl#main>
        a             owl:Class;
        rdfs:comment  "Request a service to persistently crawl hosted repos. Expected use is new PDS instances declaring their existence to Relays. Does not require auth." .

<https://atproto.social/ontology/com.atproto.sync.subscribeRepos#account>
        a             owl:Class;
        rdfs:comment  "Represents a change to an account's status on a host (eg, PDS or Relay). The semantics of this event are that the status is at the host which emitted the event, not necessarily that at the currently active PDS. Eg, a Relay takedown would emit a takedown with active=false, even if the PDS is still active." .

<https://atproto.social/ontology/com.atproto.sync.subscribeRepos#account/status>
        a             owl:DatatypeProperty;
        rdfs:domain   <https://atproto.social/ontology/com.atproto.sync.subscribeRepos#account>;
        rdfs:range    <xsd:string>;
        rdfs:comment  "If active=false, this optional field indicates a reason for why the account is not active." .

<https://atproto.social/ontology/com.atproto.sync.subscribeRepos#account/seq>
        a            owl:DatatypeProperty;
        rdfs:domain  <https://atproto.social/ontology/com.atproto.sync.subscribeRepos#account>;
        rdfs:range   <xsd:integer> .

<https://atproto.social/ontology/com.atproto.sync.subscribeRepos#account/did>
        a            owl:DatatypeProperty;
        rdfs:domain  <https://atproto.social/ontology/com.atproto.sync.subscribeRepos#account>;
        rdfs:range   <xsd:string> .

<https://atproto.social/ontology/com.atproto.sync.subscribeRepos#account/time>
        a            owl:DatatypeProperty;
        rdfs:domain  <https://atproto.social/ontology/com.atproto.sync.subscribeRepos#account>;
        rdfs:range   <xsd:string> .

<https://atproto.social/ontology/com.atproto.sync.subscribeRepos#account/active>
        a             owl:DatatypeProperty;
        rdfs:domain   <https://atproto.social/ontology/com.atproto.sync.subscribeRepos#account>;
        rdfs:range    <xsd:boolean>;
        rdfs:comment  "Indicates that the account has a repository which can be fetched from the host that emitted this event." .

<https://atproto.social/ontology/com.atproto.sync.subscribeRepos#info>
        a       owl:Class .

<https://atproto.social/ontology/com.atproto.sync.subscribeRepos#info/name>
        a            owl:DatatypeProperty;
        rdfs:domain  <https://atproto.social/ontology/com.atproto.sync.subscribeRepos#info>;
        rdfs:range   <xsd:string> .

<https://atproto.social/ontology/com.atproto.sync.subscribeRepos#info/message>
        a            owl:DatatypeProperty;
        rdfs:domain  <https://atproto.social/ontology/com.atproto.sync.subscribeRepos#info>;
        rdfs:range   <xsd:string> .

<https://atproto.social/ontology/com.atproto.sync.subscribeRepos#repoOp>
        a             owl:Class;
        rdfs:comment  "A repo operation, ie a mutation of a single record." .

<https://atproto.social/ontology/com.atproto.sync.subscribeRepos#repoOp/cid>
        a             owl:ObjectProperty;
        rdfs:domain   <https://atproto.social/ontology/com.atproto.sync.subscribeRepos#repoOp>;
        rdfs:comment  "For creates and updates, the new record CID. For deletions, null." .

<https://atproto.social/ontology/com.atproto.sync.subscribeRepos#repoOp/prev>
        a             owl:ObjectProperty;
        rdfs:domain   <https://atproto.social/ontology/com.atproto.sync.subscribeRepos#repoOp>;
        rdfs:comment  "For updates and deletes, the previous record CID (required for inductive firehose). For creations, field should not be defined." .

<https://atproto.social/ontology/com.atproto.sync.subscribeRepos#repoOp/action>
        a            owl:DatatypeProperty;
        rdfs:domain  <https://atproto.social/ontology/com.atproto.sync.subscribeRepos#repoOp>;
        rdfs:range   <xsd:string> .

<https://atproto.social/ontology/com.atproto.sync.subscribeRepos#repoOp/path>
        a            owl:DatatypeProperty;
        rdfs:domain  <https://atproto.social/ontology/com.atproto.sync.subscribeRepos#repoOp>;
        rdfs:range   <xsd:string> .

<https://atproto.social/ontology/com.atproto.sync.subscribeRepos#main>
        a             owl:Class;
        rdfs:comment  "Repository event stream, aka Firehose endpoint. Outputs repo commits with diff data, and identity update events, for all repositories on the current server. See the atproto specifications for details around stream sequencing, repo versioning, CAR diff format, and more. Public and does not require auth; implemented by PDS and Relay." .

<https://atproto.social/ontology/com.atproto.sync.subscribeRepos#commit>
        a             owl:Class;
        rdfs:comment  "Represents an update of repository state. Note that empty commits are allowed, which include no repo data changes, but an update to rev and signature." .

<https://atproto.social/ontology/com.atproto.sync.subscribeRepos#commit/blobs>
        a            owl:ObjectProperty;
        rdfs:domain  <https://atproto.social/ontology/com.atproto.sync.subscribeRepos#commit> .

<https://atproto.social/ontology/com.atproto.sync.subscribeRepos#commit/prevData>
        a             owl:ObjectProperty;
        rdfs:domain   <https://atproto.social/ontology/com.atproto.sync.subscribeRepos#commit>;
        rdfs:comment  "The root CID of the MST tree for the previous commit from this repo (indicated by the 'since' revision field in this message). Corresponds to the 'data' field in the repo commit object. NOTE: this field is effectively required for the 'inductive' version of firehose." .

<https://atproto.social/ontology/com.atproto.sync.subscribeRepos#commit/seq>
        a             owl:DatatypeProperty;
        rdfs:domain   <https://atproto.social/ontology/com.atproto.sync.subscribeRepos#commit>;
        rdfs:range    <xsd:integer>;
        rdfs:comment  "The stream sequence number of this message." .

<https://atproto.social/ontology/com.atproto.sync.subscribeRepos#commit/rebase>
        a             owl:DatatypeProperty;
        rdfs:domain   <https://atproto.social/ontology/com.atproto.sync.subscribeRepos#commit>;
        rdfs:range    <xsd:boolean>;
        rdfs:comment  "DEPRECATED -- unused" .

<https://atproto.social/ontology/com.atproto.sync.subscribeRepos#commit/repo>
        a             owl:DatatypeProperty;
        rdfs:domain   <https://atproto.social/ontology/com.atproto.sync.subscribeRepos#commit>;
        rdfs:range    <xsd:string>;
        rdfs:comment  "The repo this event comes from. Note that all other message types name this field 'did'." .

<https://atproto.social/ontology/com.atproto.sync.subscribeRepos#commit/commit>
        a             owl:ObjectProperty;
        rdfs:domain   <https://atproto.social/ontology/com.atproto.sync.subscribeRepos#commit>;
        rdfs:comment  "Repo commit object CID." .

<https://atproto.social/ontology/com.atproto.sync.subscribeRepos#commit/since>
        a             owl:DatatypeProperty;
        rdfs:domain   <https://atproto.social/ontology/com.atproto.sync.subscribeRepos#commit>;
        rdfs:range    <xsd:string>;
        rdfs:comment  "The rev of the last emitted commit from this repo (if any)." .

<https://atproto.social/ontology/com.atproto.sync.subscribeRepos#commit/ops>
        a            owl:ObjectProperty;
        rdfs:domain  <https://atproto.social/ontology/com.atproto.sync.subscribeRepos#commit>;
        rdfs:range   <https://atproto.social/ontology/com.atproto.sync.subscribeRepos#repoOp> .

<https://atproto.social/ontology/com.atproto.sync.subscribeRepos#commit/time>
        a             owl:DatatypeProperty;
        rdfs:domain   <https://atproto.social/ontology/com.atproto.sync.subscribeRepos#commit>;
        rdfs:range    <xsd:string>;
        rdfs:comment  "Timestamp of when this message was originally broadcast." .

<https://atproto.social/ontology/com.atproto.sync.subscribeRepos#commit/tooBig>
        a             owl:DatatypeProperty;
        rdfs:domain   <https://atproto.social/ontology/com.atproto.sync.subscribeRepos#commit>;
        rdfs:range    <xsd:boolean>;
        rdfs:comment  "DEPRECATED -- replaced by #sync event and data limits. Indicates that this commit contained too many ops, or data size was too large. Consumers will need to make a separate request to get missing data." .

<https://atproto.social/ontology/com.atproto.sync.subscribeRepos#commit/rev>
        a             owl:DatatypeProperty;
        rdfs:domain   <https://atproto.social/ontology/com.atproto.sync.subscribeRepos#commit>;
        rdfs:range    <xsd:string>;
        rdfs:comment  "The rev of the emitted commit. Note that this information is also in the commit object included in blocks, unless this is a tooBig event." .

<https://atproto.social/ontology/com.atproto.sync.subscribeRepos#commit/blocks>
        a             owl:ObjectProperty;
        rdfs:domain   <https://atproto.social/ontology/com.atproto.sync.subscribeRepos#commit>;
        rdfs:comment  "CAR file containing relevant blocks, as a diff since the previous repo state. The commit must be included as a block, and the commit block CID must be the first entry in the CAR header 'roots' list." .

<https://atproto.social/ontology/com.atproto.sync.subscribeRepos#sync>
        a             owl:Class;
        rdfs:comment  "Updates the repo to a new state, without necessarily including that state on the firehose. Used to recover from broken commit streams, data loss incidents, or in situations where upstream host does not know recent state of the repository." .

<https://atproto.social/ontology/com.atproto.sync.subscribeRepos#sync/seq>
        a             owl:DatatypeProperty;
        rdfs:domain   <https://atproto.social/ontology/com.atproto.sync.subscribeRepos#sync>;
        rdfs:range    <xsd:integer>;
        rdfs:comment  "The stream sequence number of this message." .

<https://atproto.social/ontology/com.atproto.sync.subscribeRepos#sync/did>
        a             owl:DatatypeProperty;
        rdfs:domain   <https://atproto.social/ontology/com.atproto.sync.subscribeRepos#sync>;
        rdfs:range    <xsd:string>;
        rdfs:comment  "The account this repo event corresponds to. Must match that in the commit object." .

<https://atproto.social/ontology/com.atproto.sync.subscribeRepos#sync/blocks>
        a             owl:ObjectProperty;
        rdfs:domain   <https://atproto.social/ontology/com.atproto.sync.subscribeRepos#sync>;
        rdfs:comment  "CAR file containing the commit, as a block. The CAR header must include the commit block CID as the first 'root'." .

<https://atproto.social/ontology/com.atproto.sync.subscribeRepos#sync/rev>
        a             owl:DatatypeProperty;
        rdfs:domain   <https://atproto.social/ontology/com.atproto.sync.subscribeRepos#sync>;
        rdfs:range    <xsd:string>;
        rdfs:comment  "The rev of the commit. This value must match that in the commit object." .

<https://atproto.social/ontology/com.atproto.sync.subscribeRepos#sync/time>
        a             owl:DatatypeProperty;
        rdfs:domain   <https://atproto.social/ontology/com.atproto.sync.subscribeRepos#sync>;
        rdfs:range    <xsd:string>;
        rdfs:comment  "Timestamp of when this message was originally broadcast." .

<https://atproto.social/ontology/com.atproto.sync.subscribeRepos#identity>
        a             owl:Class;
        rdfs:comment  "Represents a change to an account's identity. Could be an updated handle, signing key, or pds hosting endpoint. Serves as a prod to all downstream services to refresh their identity cache." .

<https://atproto.social/ontology/com.atproto.sync.subscribeRepos#identity/seq>
        a            owl:DatatypeProperty;
        rdfs:domain  <https://atproto.social/ontology/com.atproto.sync.subscribeRepos#identity>;
        rdfs:range   <xsd:integer> .

<https://atproto.social/ontology/com.atproto.sync.subscribeRepos#identity/did>
        a            owl:DatatypeProperty;
        rdfs:domain  <https://atproto.social/ontology/com.atproto.sync.subscribeRepos#identity>;
        rdfs:range   <xsd:string> .

<https://atproto.social/ontology/com.atproto.sync.subscribeRepos#identity/time>
        a            owl:DatatypeProperty;
        rdfs:domain  <https://atproto.social/ontology/com.atproto.sync.subscribeRepos#identity>;
        rdfs:range   <xsd:string> .

<https://atproto.social/ontology/com.atproto.sync.subscribeRepos#identity/handle>
        a             owl:DatatypeProperty;
        rdfs:domain   <https://atproto.social/ontology/com.atproto.sync.subscribeRepos#identity>;
        rdfs:range    <xsd:string>;
        rdfs:comment  "The current handle for the account, or 'handle.invalid' if validation fails. This field is optional, might have been validated or passed-through from an upstream source. Semantics and behaviors for PDS vs Relay may evolve in the future; see atproto specs for more details." .

<https://atproto.social/ontology/com.atproto.temp.addReservedHandle#main>
        a             owl:Class;
        rdfs:comment  "Add a handle to the set of reserved handles." .

<https://atproto.social/ontology/com.atproto.temp.checkSignupQueue#main>
        a             owl:Class;
        rdfs:comment  "Check accounts location in signup queue." .

<https://atproto.social/ontology/com.atproto.temp.fetchLabels#main>
        a             owl:Class;
        rdfs:comment  "DEPRECATED: use queryLabels or subscribeLabels instead -- Fetch all labels from a labeler created after a certain date." .

<https://atproto.social/ontology/com.atproto.temp.requestPhoneVerification#main>
        a             owl:Class;
        rdfs:comment  "Request a verification code to be sent to the supplied phone number" .

<https://atproto.social/ontology/tools.ozone.communication.createTemplate#main>
        a             owl:Class;
        rdfs:comment  "Administrative action to create a new, re-usable communication (email for now) template." .

<https://atproto.social/ontology/tools.ozone.communication.defs#templateView>
        a       owl:Class .

<https://atproto.social/ontology/tools.ozone.communication.defs#templateView/createdAt>
        a            owl:DatatypeProperty;
        rdfs:domain  <https://atproto.social/ontology/tools.ozone.communication.defs#templateView>;
        rdfs:range   <xsd:string> .

<https://atproto.social/ontology/tools.ozone.communication.defs#templateView/updatedAt>
        a            owl:DatatypeProperty;
        rdfs:domain  <https://atproto.social/ontology/tools.ozone.communication.defs#templateView>;
        rdfs:range   <xsd:string> .

<https://atproto.social/ontology/tools.ozone.communication.defs#templateView/lastUpdatedBy>
        a             owl:DatatypeProperty;
        rdfs:domain   <https://atproto.social/ontology/tools.ozone.communication.defs#templateView>;
        rdfs:range    <xsd:string>;
        rdfs:comment  "DID of the user who last updated the template." .

<https://atproto.social/ontology/tools.ozone.communication.defs#templateView/id>
        a            owl:DatatypeProperty;
        rdfs:domain  <https://atproto.social/ontology/tools.ozone.communication.defs#templateView>;
        rdfs:range   <xsd:string> .

<https://atproto.social/ontology/tools.ozone.communication.defs#templateView/name>
        a             owl:DatatypeProperty;
        rdfs:domain   <https://atproto.social/ontology/tools.ozone.communication.defs#templateView>;
        rdfs:range    <xsd:string>;
        rdfs:comment  "Name of the template." .

<https://atproto.social/ontology/tools.ozone.communication.defs#templateView/subject>
        a             owl:DatatypeProperty;
        rdfs:domain   <https://atproto.social/ontology/tools.ozone.communication.defs#templateView>;
        rdfs:range    <xsd:string>;
        rdfs:comment  "Content of the template, can contain markdown and variable placeholders." .

<https://atproto.social/ontology/tools.ozone.communication.defs#templateView/contentMarkdown>
        a             owl:DatatypeProperty;
        rdfs:domain   <https://atproto.social/ontology/tools.ozone.communication.defs#templateView>;
        rdfs:range    <xsd:string>;
        rdfs:comment  "Subject of the message, used in emails." .

<https://atproto.social/ontology/tools.ozone.communication.defs#templateView/disabled>
        a            owl:DatatypeProperty;
        rdfs:domain  <https://atproto.social/ontology/tools.ozone.communication.defs#templateView>;
        rdfs:range   <xsd:boolean> .

<https://atproto.social/ontology/tools.ozone.communication.defs#templateView/lang>
        a             owl:DatatypeProperty;
        rdfs:domain   <https://atproto.social/ontology/tools.ozone.communication.defs#templateView>;
        rdfs:range    <xsd:string>;
        rdfs:comment  "Message language." .

<https://atproto.social/ontology/tools.ozone.communication.deleteTemplate#main>
        a             owl:Class;
        rdfs:comment  "Delete a communication template." .

<https://atproto.social/ontology/tools.ozone.communication.listTemplates#main>
        a             owl:Class;
        rdfs:comment  "Get list of all communication templates." .

<https://atproto.social/ontology/tools.ozone.communication.updateTemplate#main>
        a             owl:Class;
        rdfs:comment  "Administrative action to update an existing communication template. Allows passing partial fields to patch specific fields only." .

<https://atproto.social/ontology/tools.ozone.hosting.getAccountHistory#main>
        a             owl:Class;
        rdfs:comment  "Get account history, e.g. log of updated email addresses or other identity information." .

<https://atproto.social/ontology/tools.ozone.hosting.getAccountHistory#event>
        a       owl:Class .

<https://atproto.social/ontology/tools.ozone.hosting.getAccountHistory#event/details>
        a            owl:ObjectProperty;
        rdfs:domain  <https://atproto.social/ontology/tools.ozone.hosting.getAccountHistory#event> .

<https://atproto.social/ontology/tools.ozone.hosting.getAccountHistory#event/createdBy>
        a            owl:DatatypeProperty;
        rdfs:domain  <https://atproto.social/ontology/tools.ozone.hosting.getAccountHistory#event>;
        rdfs:range   <xsd:string> .

<https://atproto.social/ontology/tools.ozone.hosting.getAccountHistory#event/createdAt>
        a            owl:DatatypeProperty;
        rdfs:domain  <https://atproto.social/ontology/tools.ozone.hosting.getAccountHistory#event>;
        rdfs:range   <xsd:string> .

<https://atproto.social/ontology/tools.ozone.hosting.getAccountHistory#accountCreated>
        a       owl:Class .

<https://atproto.social/ontology/tools.ozone.hosting.getAccountHistory#accountCreated/email>
        a            owl:DatatypeProperty;
        rdfs:domain  <https://atproto.social/ontology/tools.ozone.hosting.getAccountHistory#accountCreated>;
        rdfs:range   <xsd:string> .

<https://atproto.social/ontology/tools.ozone.hosting.getAccountHistory#accountCreated/handle>
        a            owl:DatatypeProperty;
        rdfs:domain  <https://atproto.social/ontology/tools.ozone.hosting.getAccountHistory#accountCreated>;
        rdfs:range   <xsd:string> .

<https://atproto.social/ontology/tools.ozone.hosting.getAccountHistory#emailUpdated>
        a       owl:Class .

<https://atproto.social/ontology/tools.ozone.hosting.getAccountHistory#emailUpdated/email>
        a            owl:DatatypeProperty;
        rdfs:domain  <https://atproto.social/ontology/tools.ozone.hosting.getAccountHistory#emailUpdated>;
        rdfs:range   <xsd:string> .

<https://atproto.social/ontology/tools.ozone.hosting.getAccountHistory#emailConfirmed>
        a       owl:Class .

<https://atproto.social/ontology/tools.ozone.hosting.getAccountHistory#emailConfirmed/email>
        a            owl:DatatypeProperty;
        rdfs:domain  <https://atproto.social/ontology/tools.ozone.hosting.getAccountHistory#emailConfirmed>;
        rdfs:range   <xsd:string> .

<https://atproto.social/ontology/tools.ozone.hosting.getAccountHistory#passwordUpdated>
        a       owl:Class .

<https://atproto.social/ontology/tools.ozone.hosting.getAccountHistory#handleUpdated>
        a       owl:Class .

<https://atproto.social/ontology/tools.ozone.hosting.getAccountHistory#handleUpdated/handle>
        a            owl:DatatypeProperty;
        rdfs:domain  <https://atproto.social/ontology/tools.ozone.hosting.getAccountHistory#handleUpdated>;
        rdfs:range   <xsd:string> .

<https://atproto.social/ontology/tools.ozone.moderation.defs#recordHosting>
        a       owl:Class .

<https://atproto.social/ontology/tools.ozone.moderation.defs#recordHosting/status>
        a            owl:DatatypeProperty;
        rdfs:domain  <https://atproto.social/ontology/tools.ozone.moderation.defs#recordHosting>;
        rdfs:range   <xsd:string> .

<https://atproto.social/ontology/tools.ozone.moderation.defs#recordHosting/updatedAt>
        a            owl:DatatypeProperty;
        rdfs:domain  <https://atproto.social/ontology/tools.ozone.moderation.defs#recordHosting>;
        rdfs:range   <xsd:string> .

<https://atproto.social/ontology/tools.ozone.moderation.defs#recordHosting/createdAt>
        a            owl:DatatypeProperty;
        rdfs:domain  <https://atproto.social/ontology/tools.ozone.moderation.defs#recordHosting>;
        rdfs:range   <xsd:string> .

<https://atproto.social/ontology/tools.ozone.moderation.defs#recordHosting/deletedAt>
        a            owl:DatatypeProperty;
        rdfs:domain  <https://atproto.social/ontology/tools.ozone.moderation.defs#recordHosting>;
        rdfs:range   <xsd:string> .

<https://atproto.social/ontology/tools.ozone.moderation.defs#modEventReverseTakedown>
        a             owl:Class;
        rdfs:comment  "Revert take down action on a subject" .

<https://atproto.social/ontology/tools.ozone.moderation.defs#modEventReverseTakedown/comment>
        a             owl:DatatypeProperty;
        rdfs:domain   <https://atproto.social/ontology/tools.ozone.moderation.defs#modEventReverseTakedown>;
        rdfs:range    <xsd:string>;
        rdfs:comment  "Describe reasoning behind the reversal." .

<https://atproto.social/ontology/tools.ozone.moderation.defs#modEventLabel>
        a             owl:Class;
        rdfs:comment  "Apply/Negate labels on a subject" .

<https://atproto.social/ontology/tools.ozone.moderation.defs#modEventLabel/comment>
        a            owl:DatatypeProperty;
        rdfs:domain  <https://atproto.social/ontology/tools.ozone.moderation.defs#modEventLabel>;
        rdfs:range   <xsd:string> .

<https://atproto.social/ontology/tools.ozone.moderation.defs#modEventLabel/createLabelVals>
        a            owl:DatatypeProperty;
        rdfs:domain  <https://atproto.social/ontology/tools.ozone.moderation.defs#modEventLabel>;
        rdfs:range   <xsd:string> .

<https://atproto.social/ontology/tools.ozone.moderation.defs#modEventLabel/negateLabelVals>
        a            owl:DatatypeProperty;
        rdfs:domain  <https://atproto.social/ontology/tools.ozone.moderation.defs#modEventLabel>;
        rdfs:range   <xsd:string> .

<https://atproto.social/ontology/tools.ozone.moderation.defs#modEventLabel/durationInHours>
        a             owl:DatatypeProperty;
        rdfs:domain   <https://atproto.social/ontology/tools.ozone.moderation.defs#modEventLabel>;
        rdfs:range    <xsd:integer>;
        rdfs:comment  "Indicates how long the label will remain on the subject. Only applies on labels that are being added." .

<https://atproto.social/ontology/tools.ozone.moderation.defs#modEventAcknowledge>
        a       owl:Class .

<https://atproto.social/ontology/tools.ozone.moderation.defs#modEventAcknowledge/acknowledgeAccountSubjects>
        a             owl:DatatypeProperty;
        rdfs:domain   <https://atproto.social/ontology/tools.ozone.moderation.defs#modEventAcknowledge>;
        rdfs:range    <xsd:boolean>;
        rdfs:comment  "If true, all other reports on content authored by this account will be resolved (acknowledged)." .

<https://atproto.social/ontology/tools.ozone.moderation.defs#modEventAcknowledge/comment>
        a            owl:DatatypeProperty;
        rdfs:domain  <https://atproto.social/ontology/tools.ozone.moderation.defs#modEventAcknowledge>;
        rdfs:range   <xsd:string> .

<https://atproto.social/ontology/tools.ozone.moderation.defs#modEventUnmute>
        a             owl:Class;
        rdfs:comment  "Unmute action on a subject" .

<https://atproto.social/ontology/tools.ozone.moderation.defs#modEventUnmute/comment>
        a             owl:DatatypeProperty;
        rdfs:domain   <https://atproto.social/ontology/tools.ozone.moderation.defs#modEventUnmute>;
        rdfs:range    <xsd:string>;
        rdfs:comment  "Describe reasoning behind the reversal." .

<https://atproto.social/ontology/tools.ozone.moderation.defs#modEventUnmuteReporter>
        a             owl:Class;
        rdfs:comment  "Unmute incoming reports from an account" .

<https://atproto.social/ontology/tools.ozone.moderation.defs#modEventUnmuteReporter/comment>
        a             owl:DatatypeProperty;
        rdfs:domain   <https://atproto.social/ontology/tools.ozone.moderation.defs#modEventUnmuteReporter>;
        rdfs:range    <xsd:string>;
        rdfs:comment  "Describe reasoning behind the reversal." .

<https://atproto.social/ontology/tools.ozone.moderation.defs#identityEvent>
        a             owl:Class;
        rdfs:comment  "Logs identity related events on a repo subject. Normally captured by automod from the firehose and emitted to ozone for historical tracking." .

<https://atproto.social/ontology/tools.ozone.moderation.defs#identityEvent/comment>
        a            owl:DatatypeProperty;
        rdfs:domain  <https://atproto.social/ontology/tools.ozone.moderation.defs#identityEvent>;
        rdfs:range   <xsd:string> .

<https://atproto.social/ontology/tools.ozone.moderation.defs#identityEvent/handle>
        a            owl:DatatypeProperty;
        rdfs:domain  <https://atproto.social/ontology/tools.ozone.moderation.defs#identityEvent>;
        rdfs:range   <xsd:string> .

<https://atproto.social/ontology/tools.ozone.moderation.defs#identityEvent/pdsHost>
        a            owl:DatatypeProperty;
        rdfs:domain  <https://atproto.social/ontology/tools.ozone.moderation.defs#identityEvent>;
        rdfs:range   <xsd:string> .

<https://atproto.social/ontology/tools.ozone.moderation.defs#identityEvent/tombstone>
        a            owl:DatatypeProperty;
        rdfs:domain  <https://atproto.social/ontology/tools.ozone.moderation.defs#identityEvent>;
        rdfs:range   <xsd:boolean> .

<https://atproto.social/ontology/tools.ozone.moderation.defs#identityEvent/timestamp>
        a            owl:DatatypeProperty;
        rdfs:domain  <https://atproto.social/ontology/tools.ozone.moderation.defs#identityEvent>;
        rdfs:range   <xsd:string> .

<https://atproto.social/ontology/tools.ozone.moderation.defs#modEventViewDetail>
        a       owl:Class .

<https://atproto.social/ontology/tools.ozone.moderation.defs#modEventViewDetail/createdAt>
        a            owl:DatatypeProperty;
        rdfs:domain  <https://atproto.social/ontology/tools.ozone.moderation.defs#modEventViewDetail>;
        rdfs:range   <xsd:string> .

<https://atproto.social/ontology/tools.ozone.moderation.defs#modEventViewDetail/id>
        a            owl:DatatypeProperty;
        rdfs:domain  <https://atproto.social/ontology/tools.ozone.moderation.defs#modEventViewDetail>;
        rdfs:range   <xsd:integer> .

<https://atproto.social/ontology/tools.ozone.moderation.defs#modEventViewDetail/event>
        a            owl:ObjectProperty;
        rdfs:domain  <https://atproto.social/ontology/tools.ozone.moderation.defs#modEventViewDetail> .

<https://atproto.social/ontology/tools.ozone.moderation.defs#modEventViewDetail/subject>
        a            owl:ObjectProperty;
        rdfs:domain  <https://atproto.social/ontology/tools.ozone.moderation.defs#modEventViewDetail> .

<https://atproto.social/ontology/tools.ozone.moderation.defs#modEventViewDetail/subjectBlobs>
        a            owl:ObjectProperty;
        rdfs:domain  <https://atproto.social/ontology/tools.ozone.moderation.defs#modEventViewDetail>;
        rdfs:range   <https://atproto.social/ontology/tools.ozone.moderation.defs#blobView> .

<https://atproto.social/ontology/tools.ozone.moderation.defs#modEventViewDetail/createdBy>
        a            owl:DatatypeProperty;
        rdfs:domain  <https://atproto.social/ontology/tools.ozone.moderation.defs#modEventViewDetail>;
        rdfs:range   <xsd:string> .

<https://atproto.social/ontology/tools.ozone.moderation.defs#reviewOpen>
        a             owl:Class;
        rdfs:comment  "Moderator review status of a subject: Open. Indicates that the subject needs to be reviewed by a moderator" .

<https://atproto.social/ontology/tools.ozone.moderation.defs#modEventResolveAppeal>
        a             owl:Class;
        rdfs:comment  "Resolve appeal on a subject" .

<https://atproto.social/ontology/tools.ozone.moderation.defs#modEventResolveAppeal/comment>
        a             owl:DatatypeProperty;
        rdfs:domain   <https://atproto.social/ontology/tools.ozone.moderation.defs#modEventResolveAppeal>;
        rdfs:range    <xsd:string>;
        rdfs:comment  "Describe resolution." .

<https://atproto.social/ontology/tools.ozone.moderation.defs#reporterStats>
        a       owl:Class .

<https://atproto.social/ontology/tools.ozone.moderation.defs#reporterStats/takendownAccountCount>
        a             owl:DatatypeProperty;
        rdfs:domain   <https://atproto.social/ontology/tools.ozone.moderation.defs#reporterStats>;
        rdfs:range    <xsd:integer>;
        rdfs:comment  "The total number of accounts taken down as a result of the user's reports." .

<https://atproto.social/ontology/tools.ozone.moderation.defs#reporterStats/labeledAccountCount>
        a             owl:DatatypeProperty;
        rdfs:domain   <https://atproto.social/ontology/tools.ozone.moderation.defs#reporterStats>;
        rdfs:range    <xsd:integer>;
        rdfs:comment  "The total number of accounts labeled as a result of the user's reports." .

<https://atproto.social/ontology/tools.ozone.moderation.defs#reporterStats/labeledRecordCount>
        a             owl:DatatypeProperty;
        rdfs:domain   <https://atproto.social/ontology/tools.ozone.moderation.defs#reporterStats>;
        rdfs:range    <xsd:integer>;
        rdfs:comment  "The total number of records labeled as a result of the user's reports." .

<https://atproto.social/ontology/tools.ozone.moderation.defs#reporterStats/accountReportCount>
        a             owl:DatatypeProperty;
        rdfs:domain   <https://atproto.social/ontology/tools.ozone.moderation.defs#reporterStats>;
        rdfs:range    <xsd:integer>;
        rdfs:comment  "The total number of reports made by the user on accounts." .

<https://atproto.social/ontology/tools.ozone.moderation.defs#reporterStats/recordReportCount>
        a             owl:DatatypeProperty;
        rdfs:domain   <https://atproto.social/ontology/tools.ozone.moderation.defs#reporterStats>;
        rdfs:range    <xsd:integer>;
        rdfs:comment  "The total number of reports made by the user on records." .

<https://atproto.social/ontology/tools.ozone.moderation.defs#reporterStats/reportedAccountCount>
        a             owl:DatatypeProperty;
        rdfs:domain   <https://atproto.social/ontology/tools.ozone.moderation.defs#reporterStats>;
        rdfs:range    <xsd:integer>;
        rdfs:comment  "The total number of accounts reported by the user." .

<https://atproto.social/ontology/tools.ozone.moderation.defs#reporterStats/reportedRecordCount>
        a             owl:DatatypeProperty;
        rdfs:domain   <https://atproto.social/ontology/tools.ozone.moderation.defs#reporterStats>;
        rdfs:range    <xsd:integer>;
        rdfs:comment  "The total number of records reported by the user." .

<https://atproto.social/ontology/tools.ozone.moderation.defs#reporterStats/takendownRecordCount>
        a             owl:DatatypeProperty;
        rdfs:domain   <https://atproto.social/ontology/tools.ozone.moderation.defs#reporterStats>;
        rdfs:range    <xsd:integer>;
        rdfs:comment  "The total number of records taken down as a result of the user's reports." .

<https://atproto.social/ontology/tools.ozone.moderation.defs#reporterStats/did>
        a            owl:DatatypeProperty;
        rdfs:domain  <https://atproto.social/ontology/tools.ozone.moderation.defs#reporterStats>;
        rdfs:range   <xsd:string> .

<https://atproto.social/ontology/tools.ozone.moderation.defs#subjectView>
        a             owl:Class;
        rdfs:comment  "Detailed view of a subject. For record subjects, the author's repo and profile will be returned." .

<https://atproto.social/ontology/tools.ozone.moderation.defs#subjectView/record>
        a            owl:ObjectProperty;
        rdfs:domain  <https://atproto.social/ontology/tools.ozone.moderation.defs#subjectView>;
        rdfs:range   <https://atproto.social/ontology/tools.ozone.moderation.defs#recordViewDetail> .

<https://atproto.social/ontology/tools.ozone.moderation.defs#subjectView/type>
        a            owl:ObjectProperty;
        rdfs:domain  <https://atproto.social/ontology/tools.ozone.moderation.defs#subjectView>;
        rdfs:range   <https://atproto.social/ontology/com.atproto.moderation.defs#subjectType> .

<https://atproto.social/ontology/tools.ozone.moderation.defs#subjectView/subject>
        a            owl:DatatypeProperty;
        rdfs:domain  <https://atproto.social/ontology/tools.ozone.moderation.defs#subjectView>;
        rdfs:range   <xsd:string> .

<https://atproto.social/ontology/tools.ozone.moderation.defs#subjectView/status>
        a            owl:ObjectProperty;
        rdfs:domain  <https://atproto.social/ontology/tools.ozone.moderation.defs#subjectView>;
        rdfs:range   <https://atproto.social/ontology/tools.ozone.moderation.defs#subjectStatusView> .

<https://atproto.social/ontology/tools.ozone.moderation.defs#subjectView/repo>
        a            owl:ObjectProperty;
        rdfs:domain  <https://atproto.social/ontology/tools.ozone.moderation.defs#subjectView>;
        rdfs:range   <https://atproto.social/ontology/tools.ozone.moderation.defs#repoViewDetail> .

<https://atproto.social/ontology/tools.ozone.moderation.defs#subjectView/profile>
        a            owl:ObjectProperty;
        rdfs:domain  <https://atproto.social/ontology/tools.ozone.moderation.defs#subjectView> .

<https://atproto.social/ontology/tools.ozone.moderation.defs#modEventTakedown>
        a             owl:Class;
        rdfs:comment  "Take down a subject permanently or temporarily" .

<https://atproto.social/ontology/tools.ozone.moderation.defs#modEventTakedown/comment>
        a            owl:DatatypeProperty;
        rdfs:domain  <https://atproto.social/ontology/tools.ozone.moderation.defs#modEventTakedown>;
        rdfs:range   <xsd:string> .

<https://atproto.social/ontology/tools.ozone.moderation.defs#modEventTakedown/durationInHours>
        a             owl:DatatypeProperty;
        rdfs:domain   <https://atproto.social/ontology/tools.ozone.moderation.defs#modEventTakedown>;
        rdfs:range    <xsd:integer>;
        rdfs:comment  "Indicates how long the takedown should be in effect before automatically expiring." .

<https://atproto.social/ontology/tools.ozone.moderation.defs#modEventTakedown/acknowledgeAccountSubjects>
        a             owl:DatatypeProperty;
        rdfs:domain   <https://atproto.social/ontology/tools.ozone.moderation.defs#modEventTakedown>;
        rdfs:range    <xsd:boolean>;
        rdfs:comment  "If true, all other reports on content authored by this account will be resolved (acknowledged)." .

<https://atproto.social/ontology/tools.ozone.moderation.defs#modEventTakedown/policies>
        a             owl:DatatypeProperty;
        rdfs:domain   <https://atproto.social/ontology/tools.ozone.moderation.defs#modEventTakedown>;
        rdfs:range    <xsd:string>;
        rdfs:comment  "Names/Keywords of the policies that drove the decision." .

<https://atproto.social/ontology/tools.ozone.moderation.defs#modEventEscalate>
        a       owl:Class .

<https://atproto.social/ontology/tools.ozone.moderation.defs#modEventEscalate/comment>
        a            owl:DatatypeProperty;
        rdfs:domain  <https://atproto.social/ontology/tools.ozone.moderation.defs#modEventEscalate>;
        rdfs:range   <xsd:string> .

<https://atproto.social/ontology/tools.ozone.moderation.defs#accountEvent>
        a             owl:Class;
        rdfs:comment  "Logs account status related events on a repo subject. Normally captured by automod from the firehose and emitted to ozone for historical tracking." .

<https://atproto.social/ontology/tools.ozone.moderation.defs#accountEvent/timestamp>
        a            owl:DatatypeProperty;
        rdfs:domain  <https://atproto.social/ontology/tools.ozone.moderation.defs#accountEvent>;
        rdfs:range   <xsd:string> .

<https://atproto.social/ontology/tools.ozone.moderation.defs#accountEvent/comment>
        a            owl:DatatypeProperty;
        rdfs:domain  <https://atproto.social/ontology/tools.ozone.moderation.defs#accountEvent>;
        rdfs:range   <xsd:string> .

<https://atproto.social/ontology/tools.ozone.moderation.defs#accountEvent/active>
        a             owl:DatatypeProperty;
        rdfs:domain   <https://atproto.social/ontology/tools.ozone.moderation.defs#accountEvent>;
        rdfs:range    <xsd:boolean>;
        rdfs:comment  "Indicates that the account has a repository which can be fetched from the host that emitted this event." .

<https://atproto.social/ontology/tools.ozone.moderation.defs#accountEvent/status>
        a            owl:DatatypeProperty;
        rdfs:domain  <https://atproto.social/ontology/tools.ozone.moderation.defs#accountEvent>;
        rdfs:range   <xsd:string> .

<https://atproto.social/ontology/tools.ozone.moderation.defs#recordView>
        a       owl:Class .

<https://atproto.social/ontology/tools.ozone.moderation.defs#recordView/indexedAt>
        a            owl:DatatypeProperty;
        rdfs:domain  <https://atproto.social/ontology/tools.ozone.moderation.defs#recordView>;
        rdfs:range   <xsd:string> .

<https://atproto.social/ontology/tools.ozone.moderation.defs#recordView/moderation>
        a            owl:ObjectProperty;
        rdfs:domain  <https://atproto.social/ontology/tools.ozone.moderation.defs#recordView>;
        rdfs:range   <https://atproto.social/ontology/tools.ozone.moderation.defs#moderation> .

<https://atproto.social/ontology/tools.ozone.moderation.defs#recordView/repo>
        a            owl:ObjectProperty;
        rdfs:domain  <https://atproto.social/ontology/tools.ozone.moderation.defs#recordView>;
        rdfs:range   <https://atproto.social/ontology/tools.ozone.moderation.defs#repoView> .

<https://atproto.social/ontology/tools.ozone.moderation.defs#recordView/uri>
        a            owl:DatatypeProperty;
        rdfs:domain  <https://atproto.social/ontology/tools.ozone.moderation.defs#recordView>;
        rdfs:range   <xsd:string> .

<https://atproto.social/ontology/tools.ozone.moderation.defs#recordView/cid>
        a            owl:DatatypeProperty;
        rdfs:domain  <https://atproto.social/ontology/tools.ozone.moderation.defs#recordView>;
        rdfs:range   <xsd:string> .

<https://atproto.social/ontology/tools.ozone.moderation.defs#recordView/value>
        a            owl:ObjectProperty;
        rdfs:domain  <https://atproto.social/ontology/tools.ozone.moderation.defs#recordView> .

<https://atproto.social/ontology/tools.ozone.moderation.defs#recordView/blobCids>
        a            owl:DatatypeProperty;
        rdfs:domain  <https://atproto.social/ontology/tools.ozone.moderation.defs#recordView>;
        rdfs:range   <xsd:string> .

<https://atproto.social/ontology/tools.ozone.moderation.defs#accountHosting>
        a       owl:Class .

<https://atproto.social/ontology/tools.ozone.moderation.defs#accountHosting/deletedAt>
        a            owl:DatatypeProperty;
        rdfs:domain  <https://atproto.social/ontology/tools.ozone.moderation.defs#accountHosting>;
        rdfs:range   <xsd:string> .

<https://atproto.social/ontology/tools.ozone.moderation.defs#accountHosting/deactivatedAt>
        a            owl:DatatypeProperty;
        rdfs:domain  <https://atproto.social/ontology/tools.ozone.moderation.defs#accountHosting>;
        rdfs:range   <xsd:string> .

<https://atproto.social/ontology/tools.ozone.moderation.defs#accountHosting/reactivatedAt>
        a            owl:DatatypeProperty;
        rdfs:domain  <https://atproto.social/ontology/tools.ozone.moderation.defs#accountHosting>;
        rdfs:range   <xsd:string> .

<https://atproto.social/ontology/tools.ozone.moderation.defs#accountHosting/status>
        a            owl:DatatypeProperty;
        rdfs:domain  <https://atproto.social/ontology/tools.ozone.moderation.defs#accountHosting>;
        rdfs:range   <xsd:string> .

<https://atproto.social/ontology/tools.ozone.moderation.defs#accountHosting/updatedAt>
        a            owl:DatatypeProperty;
        rdfs:domain  <https://atproto.social/ontology/tools.ozone.moderation.defs#accountHosting>;
        rdfs:range   <xsd:string> .

<https://atproto.social/ontology/tools.ozone.moderation.defs#accountHosting/createdAt>
        a            owl:DatatypeProperty;
        rdfs:domain  <https://atproto.social/ontology/tools.ozone.moderation.defs#accountHosting>;
        rdfs:range   <xsd:string> .

<https://atproto.social/ontology/tools.ozone.moderation.defs#reviewEscalated>
        a             owl:Class;
        rdfs:comment  "Moderator review status of a subject: Escalated. Indicates that the subject was escalated for review by a moderator" .

<https://atproto.social/ontology/tools.ozone.moderation.defs#modEventComment>
        a             owl:Class;
        rdfs:comment  "Add a comment to a subject. An empty comment will clear any previously set sticky comment." .

<https://atproto.social/ontology/tools.ozone.moderation.defs#modEventComment/comment>
        a            owl:DatatypeProperty;
        rdfs:domain  <https://atproto.social/ontology/tools.ozone.moderation.defs#modEventComment>;
        rdfs:range   <xsd:string> .

<https://atproto.social/ontology/tools.ozone.moderation.defs#modEventComment/sticky>
        a             owl:DatatypeProperty;
        rdfs:domain   <https://atproto.social/ontology/tools.ozone.moderation.defs#modEventComment>;
        rdfs:range    <xsd:boolean>;
        rdfs:comment  "Make the comment persistent on the subject" .

<https://atproto.social/ontology/tools.ozone.moderation.defs#modEventPriorityScore>
        a             owl:Class;
        rdfs:comment  "Set priority score of the subject. Higher score means higher priority." .

<https://atproto.social/ontology/tools.ozone.moderation.defs#modEventPriorityScore/comment>
        a            owl:DatatypeProperty;
        rdfs:domain  <https://atproto.social/ontology/tools.ozone.moderation.defs#modEventPriorityScore>;
        rdfs:range   <xsd:string> .

<https://atproto.social/ontology/tools.ozone.moderation.defs#modEventPriorityScore/score>
        a            owl:DatatypeProperty;
        rdfs:domain  <https://atproto.social/ontology/tools.ozone.moderation.defs#modEventPriorityScore>;
        rdfs:range   <xsd:integer> .

<https://atproto.social/ontology/tools.ozone.moderation.defs#modEventMute>
        a             owl:Class;
        rdfs:comment  "Mute incoming reports on a subject" .

<https://atproto.social/ontology/tools.ozone.moderation.defs#modEventMute/comment>
        a            owl:DatatypeProperty;
        rdfs:domain  <https://atproto.social/ontology/tools.ozone.moderation.defs#modEventMute>;
        rdfs:range   <xsd:string> .

<https://atproto.social/ontology/tools.ozone.moderation.defs#modEventMute/durationInHours>
        a             owl:DatatypeProperty;
        rdfs:domain   <https://atproto.social/ontology/tools.ozone.moderation.defs#modEventMute>;
        rdfs:range    <xsd:integer>;
        rdfs:comment  "Indicates how long the subject should remain muted." .

<https://atproto.social/ontology/tools.ozone.moderation.defs#recordEvent>
        a             owl:Class;
        rdfs:comment  "Logs lifecycle event on a record subject. Normally captured by automod from the firehose and emitted to ozone for historical tracking." .

<https://atproto.social/ontology/tools.ozone.moderation.defs#recordEvent/comment>
        a            owl:DatatypeProperty;
        rdfs:domain  <https://atproto.social/ontology/tools.ozone.moderation.defs#recordEvent>;
        rdfs:range   <xsd:string> .

<https://atproto.social/ontology/tools.ozone.moderation.defs#recordEvent/op>
        a            owl:DatatypeProperty;
        rdfs:domain  <https://atproto.social/ontology/tools.ozone.moderation.defs#recordEvent>;
        rdfs:range   <xsd:string> .

<https://atproto.social/ontology/tools.ozone.moderation.defs#recordEvent/cid>
        a            owl:DatatypeProperty;
        rdfs:domain  <https://atproto.social/ontology/tools.ozone.moderation.defs#recordEvent>;
        rdfs:range   <xsd:string> .

<https://atproto.social/ontology/tools.ozone.moderation.defs#recordEvent/timestamp>
        a            owl:DatatypeProperty;
        rdfs:domain  <https://atproto.social/ontology/tools.ozone.moderation.defs#recordEvent>;
        rdfs:range   <xsd:string> .

<https://atproto.social/ontology/tools.ozone.moderation.defs#moderationDetail>
        a       owl:Class .

<https://atproto.social/ontology/tools.ozone.moderation.defs#moderationDetail/subjectStatus>
        a            owl:ObjectProperty;
        rdfs:domain  <https://atproto.social/ontology/tools.ozone.moderation.defs#moderationDetail>;
        rdfs:range   <https://atproto.social/ontology/tools.ozone.moderation.defs#subjectStatusView> .

<https://atproto.social/ontology/tools.ozone.moderation.defs#modEventReport>
        a             owl:Class;
        rdfs:comment  "Report a subject" .

<https://atproto.social/ontology/tools.ozone.moderation.defs#modEventReport/isReporterMuted>
        a             owl:DatatypeProperty;
        rdfs:domain   <https://atproto.social/ontology/tools.ozone.moderation.defs#modEventReport>;
        rdfs:range    <xsd:boolean>;
        rdfs:comment  "Set to true if the reporter was muted from reporting at the time of the event. These reports won't impact the reviewState of the subject." .

<https://atproto.social/ontology/tools.ozone.moderation.defs#modEventReport/reportType>
        a            owl:ObjectProperty;
        rdfs:domain  <https://atproto.social/ontology/tools.ozone.moderation.defs#modEventReport>;
        rdfs:range   <https://atproto.social/ontology/com.atproto.moderation.defs#reasonType> .

<https://atproto.social/ontology/tools.ozone.moderation.defs#modEventReport/comment>
        a            owl:DatatypeProperty;
        rdfs:domain  <https://atproto.social/ontology/tools.ozone.moderation.defs#modEventReport>;
        rdfs:range   <xsd:string> .

<https://atproto.social/ontology/tools.ozone.moderation.defs#repoView>
        a       owl:Class .

<https://atproto.social/ontology/tools.ozone.moderation.defs#repoView/email>
        a            owl:DatatypeProperty;
        rdfs:domain  <https://atproto.social/ontology/tools.ozone.moderation.defs#repoView>;
        rdfs:range   <xsd:string> .

<https://atproto.social/ontology/tools.ozone.moderation.defs#repoView/relatedRecords>
        a            owl:ObjectProperty;
        rdfs:domain  <https://atproto.social/ontology/tools.ozone.moderation.defs#repoView> .

<https://atproto.social/ontology/tools.ozone.moderation.defs#repoView/indexedAt>
        a            owl:DatatypeProperty;
        rdfs:domain  <https://atproto.social/ontology/tools.ozone.moderation.defs#repoView>;
        rdfs:range   <xsd:string> .

<https://atproto.social/ontology/tools.ozone.moderation.defs#repoView/invitesDisabled>
        a            owl:DatatypeProperty;
        rdfs:domain  <https://atproto.social/ontology/tools.ozone.moderation.defs#repoView>;
        rdfs:range   <xsd:boolean> .

<https://atproto.social/ontology/tools.ozone.moderation.defs#repoView/did>
        a            owl:DatatypeProperty;
        rdfs:domain  <https://atproto.social/ontology/tools.ozone.moderation.defs#repoView>;
        rdfs:range   <xsd:string> .

<https://atproto.social/ontology/tools.ozone.moderation.defs#repoView/handle>
        a            owl:DatatypeProperty;
        rdfs:domain  <https://atproto.social/ontology/tools.ozone.moderation.defs#repoView>;
        rdfs:range   <xsd:string> .

<https://atproto.social/ontology/tools.ozone.moderation.defs#repoView/moderation>
        a            owl:ObjectProperty;
        rdfs:domain  <https://atproto.social/ontology/tools.ozone.moderation.defs#repoView>;
        rdfs:range   <https://atproto.social/ontology/tools.ozone.moderation.defs#moderation> .

<https://atproto.social/ontology/tools.ozone.moderation.defs#repoView/invitedBy>
        a            owl:ObjectProperty;
        rdfs:domain  <https://atproto.social/ontology/tools.ozone.moderation.defs#repoView>;
        rdfs:range   <https://atproto.social/ontology/com.atproto.server.defs#inviteCode> .

<https://atproto.social/ontology/tools.ozone.moderation.defs#repoView/inviteNote>
        a            owl:DatatypeProperty;
        rdfs:domain  <https://atproto.social/ontology/tools.ozone.moderation.defs#repoView>;
        rdfs:range   <xsd:string> .

<https://atproto.social/ontology/tools.ozone.moderation.defs#repoView/deactivatedAt>
        a            owl:DatatypeProperty;
        rdfs:domain  <https://atproto.social/ontology/tools.ozone.moderation.defs#repoView>;
        rdfs:range   <xsd:string> .

<https://atproto.social/ontology/tools.ozone.moderation.defs#repoView/threatSignatures>
        a            owl:ObjectProperty;
        rdfs:domain  <https://atproto.social/ontology/tools.ozone.moderation.defs#repoView>;
        rdfs:range   <https://atproto.social/ontology/com.atproto.admin.defs#threatSignature> .

<https://atproto.social/ontology/tools.ozone.moderation.defs#repoViewNotFound>
        a       owl:Class .

<https://atproto.social/ontology/tools.ozone.moderation.defs#repoViewNotFound/did>
        a            owl:DatatypeProperty;
        rdfs:domain  <https://atproto.social/ontology/tools.ozone.moderation.defs#repoViewNotFound>;
        rdfs:range   <xsd:string> .

<https://atproto.social/ontology/tools.ozone.moderation.defs#blobView>
        a       owl:Class .

<https://atproto.social/ontology/tools.ozone.moderation.defs#blobView/mimeType>
        a            owl:DatatypeProperty;
        rdfs:domain  <https://atproto.social/ontology/tools.ozone.moderation.defs#blobView>;
        rdfs:range   <xsd:string> .

<https://atproto.social/ontology/tools.ozone.moderation.defs#blobView/size>
        a            owl:DatatypeProperty;
        rdfs:domain  <https://atproto.social/ontology/tools.ozone.moderation.defs#blobView>;
        rdfs:range   <xsd:integer> .

<https://atproto.social/ontology/tools.ozone.moderation.defs#blobView/createdAt>
        a            owl:DatatypeProperty;
        rdfs:domain  <https://atproto.social/ontology/tools.ozone.moderation.defs#blobView>;
        rdfs:range   <xsd:string> .

<https://atproto.social/ontology/tools.ozone.moderation.defs#blobView/details>
        a            owl:ObjectProperty;
        rdfs:domain  <https://atproto.social/ontology/tools.ozone.moderation.defs#blobView> .

<https://atproto.social/ontology/tools.ozone.moderation.defs#blobView/moderation>
        a            owl:ObjectProperty;
        rdfs:domain  <https://atproto.social/ontology/tools.ozone.moderation.defs#blobView>;
        rdfs:range   <https://atproto.social/ontology/tools.ozone.moderation.defs#moderation> .

<https://atproto.social/ontology/tools.ozone.moderation.defs#blobView/cid>
        a            owl:DatatypeProperty;
        rdfs:domain  <https://atproto.social/ontology/tools.ozone.moderation.defs#blobView>;
        rdfs:range   <xsd:string> .

<https://atproto.social/ontology/tools.ozone.moderation.defs#imageDetails>
        a       owl:Class .

<https://atproto.social/ontology/tools.ozone.moderation.defs#imageDetails/width>
        a            owl:DatatypeProperty;
        rdfs:domain  <https://atproto.social/ontology/tools.ozone.moderation.defs#imageDetails>;
        rdfs:range   <xsd:integer> .

<https://atproto.social/ontology/tools.ozone.moderation.defs#imageDetails/height>
        a            owl:DatatypeProperty;
        rdfs:domain  <https://atproto.social/ontology/tools.ozone.moderation.defs#imageDetails>;
        rdfs:range   <xsd:integer> .

<https://atproto.social/ontology/tools.ozone.moderation.defs#recordsStats>
        a             owl:Class;
        rdfs:comment  "Statistics about a set of record subject items" .

<https://atproto.social/ontology/tools.ozone.moderation.defs#recordsStats/takendownCount>
        a             owl:DatatypeProperty;
        rdfs:domain   <https://atproto.social/ontology/tools.ozone.moderation.defs#recordsStats>;
        rdfs:range    <xsd:integer>;
        rdfs:comment  "Number of item currently taken down" .

<https://atproto.social/ontology/tools.ozone.moderation.defs#recordsStats/totalReports>
        a             owl:DatatypeProperty;
        rdfs:domain   <https://atproto.social/ontology/tools.ozone.moderation.defs#recordsStats>;
        rdfs:range    <xsd:integer>;
        rdfs:comment  "Cumulative sum of the number of reports on the items in the set" .

<https://atproto.social/ontology/tools.ozone.moderation.defs#recordsStats/reportedCount>
        a             owl:DatatypeProperty;
        rdfs:domain   <https://atproto.social/ontology/tools.ozone.moderation.defs#recordsStats>;
        rdfs:range    <xsd:integer>;
        rdfs:comment  "Number of items that were reported at least once" .

<https://atproto.social/ontology/tools.ozone.moderation.defs#recordsStats/escalatedCount>
        a             owl:DatatypeProperty;
        rdfs:domain   <https://atproto.social/ontology/tools.ozone.moderation.defs#recordsStats>;
        rdfs:range    <xsd:integer>;
        rdfs:comment  "Number of items that were escalated at least once" .

<https://atproto.social/ontology/tools.ozone.moderation.defs#recordsStats/appealedCount>
        a             owl:DatatypeProperty;
        rdfs:domain   <https://atproto.social/ontology/tools.ozone.moderation.defs#recordsStats>;
        rdfs:range    <xsd:integer>;
        rdfs:comment  "Number of items that were appealed at least once" .

<https://atproto.social/ontology/tools.ozone.moderation.defs#recordsStats/subjectCount>
        a             owl:DatatypeProperty;
        rdfs:domain   <https://atproto.social/ontology/tools.ozone.moderation.defs#recordsStats>;
        rdfs:range    <xsd:integer>;
        rdfs:comment  "Total number of item in the set" .

<https://atproto.social/ontology/tools.ozone.moderation.defs#recordsStats/pendingCount>
        a             owl:DatatypeProperty;
        rdfs:domain   <https://atproto.social/ontology/tools.ozone.moderation.defs#recordsStats>;
        rdfs:range    <xsd:integer>;
        rdfs:comment  "Number of item currently in \"reviewOpen\" or \"reviewEscalated\" state" .

<https://atproto.social/ontology/tools.ozone.moderation.defs#recordsStats/processedCount>
        a             owl:DatatypeProperty;
        rdfs:domain   <https://atproto.social/ontology/tools.ozone.moderation.defs#recordsStats>;
        rdfs:range    <xsd:integer>;
        rdfs:comment  "Number of item currently in \"reviewNone\" or \"reviewClosed\" state" .

<https://atproto.social/ontology/tools.ozone.moderation.defs#subjectReviewState>
        a       owl:Class .

<https://atproto.social/ontology/tools.ozone.moderation.defs#reviewClosed>
        a             owl:Class;
        rdfs:comment  "Moderator review status of a subject: Closed. Indicates that the subject was already reviewed and resolved by a moderator" .

<https://atproto.social/ontology/tools.ozone.moderation.defs#modEventDivert>
        a             owl:Class;
        rdfs:comment  "Divert a record's blobs to a 3rd party service for further scanning/tagging" .

<https://atproto.social/ontology/tools.ozone.moderation.defs#modEventDivert/comment>
        a            owl:DatatypeProperty;
        rdfs:domain  <https://atproto.social/ontology/tools.ozone.moderation.defs#modEventDivert>;
        rdfs:range   <xsd:string> .

<https://atproto.social/ontology/tools.ozone.moderation.defs#repoViewDetail>
        a       owl:Class .

<https://atproto.social/ontology/tools.ozone.moderation.defs#repoViewDetail/deactivatedAt>
        a            owl:DatatypeProperty;
        rdfs:domain  <https://atproto.social/ontology/tools.ozone.moderation.defs#repoViewDetail>;
        rdfs:range   <xsd:string> .

<https://atproto.social/ontology/tools.ozone.moderation.defs#repoViewDetail/did>
        a            owl:DatatypeProperty;
        rdfs:domain  <https://atproto.social/ontology/tools.ozone.moderation.defs#repoViewDetail>;
        rdfs:range   <xsd:string> .

<https://atproto.social/ontology/tools.ozone.moderation.defs#repoViewDetail/handle>
        a            owl:DatatypeProperty;
        rdfs:domain  <https://atproto.social/ontology/tools.ozone.moderation.defs#repoViewDetail>;
        rdfs:range   <xsd:string> .

<https://atproto.social/ontology/tools.ozone.moderation.defs#repoViewDetail/relatedRecords>
        a            owl:ObjectProperty;
        rdfs:domain  <https://atproto.social/ontology/tools.ozone.moderation.defs#repoViewDetail> .

<https://atproto.social/ontology/tools.ozone.moderation.defs#repoViewDetail/labels>
        a            owl:ObjectProperty;
        rdfs:domain  <https://atproto.social/ontology/tools.ozone.moderation.defs#repoViewDetail>;
        rdfs:range   <https://atproto.social/ontology/com.atproto.label.defs#label> .

<https://atproto.social/ontology/tools.ozone.moderation.defs#repoViewDetail/invites>
        a            owl:ObjectProperty;
        rdfs:domain  <https://atproto.social/ontology/tools.ozone.moderation.defs#repoViewDetail>;
        rdfs:range   <https://atproto.social/ontology/com.atproto.server.defs#inviteCode> .

<https://atproto.social/ontology/tools.ozone.moderation.defs#repoViewDetail/threatSignatures>
        a            owl:ObjectProperty;
        rdfs:domain  <https://atproto.social/ontology/tools.ozone.moderation.defs#repoViewDetail>;
        rdfs:range   <https://atproto.social/ontology/com.atproto.admin.defs#threatSignature> .

<https://atproto.social/ontology/tools.ozone.moderation.defs#repoViewDetail/email>
        a            owl:DatatypeProperty;
        rdfs:domain  <https://atproto.social/ontology/tools.ozone.moderation.defs#repoViewDetail>;
        rdfs:range   <xsd:string> .

<https://atproto.social/ontology/tools.ozone.moderation.defs#repoViewDetail/indexedAt>
        a            owl:DatatypeProperty;
        rdfs:domain  <https://atproto.social/ontology/tools.ozone.moderation.defs#repoViewDetail>;
        rdfs:range   <xsd:string> .

<https://atproto.social/ontology/tools.ozone.moderation.defs#repoViewDetail/moderation>
        a            owl:ObjectProperty;
        rdfs:domain  <https://atproto.social/ontology/tools.ozone.moderation.defs#repoViewDetail>;
        rdfs:range   <https://atproto.social/ontology/tools.ozone.moderation.defs#moderationDetail> .

<https://atproto.social/ontology/tools.ozone.moderation.defs#repoViewDetail/invitedBy>
        a            owl:ObjectProperty;
        rdfs:domain  <https://atproto.social/ontology/tools.ozone.moderation.defs#repoViewDetail>;
        rdfs:range   <https://atproto.social/ontology/com.atproto.server.defs#inviteCode> .

<https://atproto.social/ontology/tools.ozone.moderation.defs#repoViewDetail/invitesDisabled>
        a            owl:DatatypeProperty;
        rdfs:domain  <https://atproto.social/ontology/tools.ozone.moderation.defs#repoViewDetail>;
        rdfs:range   <xsd:boolean> .

<https://atproto.social/ontology/tools.ozone.moderation.defs#repoViewDetail/inviteNote>
        a            owl:DatatypeProperty;
        rdfs:domain  <https://atproto.social/ontology/tools.ozone.moderation.defs#repoViewDetail>;
        rdfs:range   <xsd:string> .

<https://atproto.social/ontology/tools.ozone.moderation.defs#repoViewDetail/emailConfirmedAt>
        a            owl:DatatypeProperty;
        rdfs:domain  <https://atproto.social/ontology/tools.ozone.moderation.defs#repoViewDetail>;
        rdfs:range   <xsd:string> .

<https://atproto.social/ontology/tools.ozone.moderation.defs#videoDetails>
        a       owl:Class .

<https://atproto.social/ontology/tools.ozone.moderation.defs#videoDetails/width>
        a            owl:DatatypeProperty;
        rdfs:domain  <https://atproto.social/ontology/tools.ozone.moderation.defs#videoDetails>;
        rdfs:range   <xsd:integer> .

<https://atproto.social/ontology/tools.ozone.moderation.defs#videoDetails/height>
        a            owl:DatatypeProperty;
        rdfs:domain  <https://atproto.social/ontology/tools.ozone.moderation.defs#videoDetails>;
        rdfs:range   <xsd:integer> .

<https://atproto.social/ontology/tools.ozone.moderation.defs#videoDetails/length>
        a            owl:DatatypeProperty;
        rdfs:domain  <https://atproto.social/ontology/tools.ozone.moderation.defs#videoDetails>;
        rdfs:range   <xsd:integer> .

<https://atproto.social/ontology/tools.ozone.moderation.defs#modEventEmail>
        a             owl:Class;
        rdfs:comment  "Keep a log of outgoing email to a user" .

<https://atproto.social/ontology/tools.ozone.moderation.defs#modEventEmail/content>
        a             owl:DatatypeProperty;
        rdfs:domain   <https://atproto.social/ontology/tools.ozone.moderation.defs#modEventEmail>;
        rdfs:range    <xsd:string>;
        rdfs:comment  "The content of the email sent to the user." .

<https://atproto.social/ontology/tools.ozone.moderation.defs#modEventEmail/comment>
        a             owl:DatatypeProperty;
        rdfs:domain   <https://atproto.social/ontology/tools.ozone.moderation.defs#modEventEmail>;
        rdfs:range    <xsd:string>;
        rdfs:comment  "Additional comment about the outgoing comm." .

<https://atproto.social/ontology/tools.ozone.moderation.defs#modEventEmail/subjectLine>
        a             owl:DatatypeProperty;
        rdfs:domain   <https://atproto.social/ontology/tools.ozone.moderation.defs#modEventEmail>;
        rdfs:range    <xsd:string>;
        rdfs:comment  "The subject line of the email sent to the user." .

<https://atproto.social/ontology/tools.ozone.moderation.defs#recordViewDetail>
        a       owl:Class .

<https://atproto.social/ontology/tools.ozone.moderation.defs#recordViewDetail/moderation>
        a            owl:ObjectProperty;
        rdfs:domain  <https://atproto.social/ontology/tools.ozone.moderation.defs#recordViewDetail>;
        rdfs:range   <https://atproto.social/ontology/tools.ozone.moderation.defs#moderationDetail> .

<https://atproto.social/ontology/tools.ozone.moderation.defs#recordViewDetail/repo>
        a            owl:ObjectProperty;
        rdfs:domain  <https://atproto.social/ontology/tools.ozone.moderation.defs#recordViewDetail>;
        rdfs:range   <https://atproto.social/ontology/tools.ozone.moderation.defs#repoView> .

<https://atproto.social/ontology/tools.ozone.moderation.defs#recordViewDetail/uri>
        a            owl:DatatypeProperty;
        rdfs:domain  <https://atproto.social/ontology/tools.ozone.moderation.defs#recordViewDetail>;
        rdfs:range   <xsd:string> .

<https://atproto.social/ontology/tools.ozone.moderation.defs#recordViewDetail/cid>
        a            owl:DatatypeProperty;
        rdfs:domain  <https://atproto.social/ontology/tools.ozone.moderation.defs#recordViewDetail>;
        rdfs:range   <xsd:string> .

<https://atproto.social/ontology/tools.ozone.moderation.defs#recordViewDetail/value>
        a            owl:ObjectProperty;
        rdfs:domain  <https://atproto.social/ontology/tools.ozone.moderation.defs#recordViewDetail> .

<https://atproto.social/ontology/tools.ozone.moderation.defs#recordViewDetail/blobs>
        a            owl:ObjectProperty;
        rdfs:domain  <https://atproto.social/ontology/tools.ozone.moderation.defs#recordViewDetail>;
        rdfs:range   <https://atproto.social/ontology/tools.ozone.moderation.defs#blobView> .

<https://atproto.social/ontology/tools.ozone.moderation.defs#recordViewDetail/labels>
        a            owl:ObjectProperty;
        rdfs:domain  <https://atproto.social/ontology/tools.ozone.moderation.defs#recordViewDetail>;
        rdfs:range   <https://atproto.social/ontology/com.atproto.label.defs#label> .

<https://atproto.social/ontology/tools.ozone.moderation.defs#recordViewDetail/indexedAt>
        a            owl:DatatypeProperty;
        rdfs:domain  <https://atproto.social/ontology/tools.ozone.moderation.defs#recordViewDetail>;
        rdfs:range   <xsd:string> .

<https://atproto.social/ontology/tools.ozone.moderation.defs#recordViewNotFound>
        a       owl:Class .

<https://atproto.social/ontology/tools.ozone.moderation.defs#recordViewNotFound/uri>
        a            owl:DatatypeProperty;
        rdfs:domain  <https://atproto.social/ontology/tools.ozone.moderation.defs#recordViewNotFound>;
        rdfs:range   <xsd:string> .

<https://atproto.social/ontology/tools.ozone.moderation.defs#moderation>
        a       owl:Class .

<https://atproto.social/ontology/tools.ozone.moderation.defs#moderation/subjectStatus>
        a            owl:ObjectProperty;
        rdfs:domain  <https://atproto.social/ontology/tools.ozone.moderation.defs#moderation>;
        rdfs:range   <https://atproto.social/ontology/tools.ozone.moderation.defs#subjectStatusView> .

<https://atproto.social/ontology/tools.ozone.moderation.defs#modEventView>
        a       owl:Class .

<https://atproto.social/ontology/tools.ozone.moderation.defs#modEventView/event>
        a            owl:ObjectProperty;
        rdfs:domain  <https://atproto.social/ontology/tools.ozone.moderation.defs#modEventView> .

<https://atproto.social/ontology/tools.ozone.moderation.defs#modEventView/subject>
        a            owl:ObjectProperty;
        rdfs:domain  <https://atproto.social/ontology/tools.ozone.moderation.defs#modEventView> .

<https://atproto.social/ontology/tools.ozone.moderation.defs#modEventView/subjectBlobCids>
        a            owl:DatatypeProperty;
        rdfs:domain  <https://atproto.social/ontology/tools.ozone.moderation.defs#modEventView>;
        rdfs:range   <xsd:string> .

<https://atproto.social/ontology/tools.ozone.moderation.defs#modEventView/createdBy>
        a            owl:DatatypeProperty;
        rdfs:domain  <https://atproto.social/ontology/tools.ozone.moderation.defs#modEventView>;
        rdfs:range   <xsd:string> .

<https://atproto.social/ontology/tools.ozone.moderation.defs#modEventView/createdAt>
        a            owl:DatatypeProperty;
        rdfs:domain  <https://atproto.social/ontology/tools.ozone.moderation.defs#modEventView>;
        rdfs:range   <xsd:string> .

<https://atproto.social/ontology/tools.ozone.moderation.defs#modEventView/creatorHandle>
        a            owl:DatatypeProperty;
        rdfs:domain  <https://atproto.social/ontology/tools.ozone.moderation.defs#modEventView>;
        rdfs:range   <xsd:string> .

<https://atproto.social/ontology/tools.ozone.moderation.defs#modEventView/subjectHandle>
        a            owl:DatatypeProperty;
        rdfs:domain  <https://atproto.social/ontology/tools.ozone.moderation.defs#modEventView>;
        rdfs:range   <xsd:string> .

<https://atproto.social/ontology/tools.ozone.moderation.defs#modEventView/id>
        a            owl:DatatypeProperty;
        rdfs:domain  <https://atproto.social/ontology/tools.ozone.moderation.defs#modEventView>;
        rdfs:range   <xsd:integer> .

<https://atproto.social/ontology/tools.ozone.moderation.defs#subjectStatusView>
        a       owl:Class .

<https://atproto.social/ontology/tools.ozone.moderation.defs#subjectStatusView/suspendUntil>
        a            owl:DatatypeProperty;
        rdfs:domain  <https://atproto.social/ontology/tools.ozone.moderation.defs#subjectStatusView>;
        rdfs:range   <xsd:string> .

<https://atproto.social/ontology/tools.ozone.moderation.defs#subjectStatusView/createdAt>
        a             owl:DatatypeProperty;
        rdfs:domain   <https://atproto.social/ontology/tools.ozone.moderation.defs#subjectStatusView>;
        rdfs:range    <xsd:string>;
        rdfs:comment  "Timestamp referencing the first moderation status impacting event was emitted on the subject" .

<https://atproto.social/ontology/tools.ozone.moderation.defs#subjectStatusView/priorityScore>
        a             owl:DatatypeProperty;
        rdfs:domain   <https://atproto.social/ontology/tools.ozone.moderation.defs#subjectStatusView>;
        rdfs:range    <xsd:integer>;
        rdfs:comment  "Numeric value representing the level of priority. Higher score means higher priority." .

<https://atproto.social/ontology/tools.ozone.moderation.defs#subjectStatusView/lastReviewedAt>
        a            owl:DatatypeProperty;
        rdfs:domain  <https://atproto.social/ontology/tools.ozone.moderation.defs#subjectStatusView>;
        rdfs:range   <xsd:string> .

<https://atproto.social/ontology/tools.ozone.moderation.defs#subjectStatusView/subject>
        a            owl:ObjectProperty;
        rdfs:domain  <https://atproto.social/ontology/tools.ozone.moderation.defs#subjectStatusView> .

<https://atproto.social/ontology/tools.ozone.moderation.defs#subjectStatusView/hosting>
        a            owl:ObjectProperty;
        rdfs:domain  <https://atproto.social/ontology/tools.ozone.moderation.defs#subjectStatusView> .

<https://atproto.social/ontology/tools.ozone.moderation.defs#subjectStatusView/comment>
        a             owl:DatatypeProperty;
        rdfs:domain   <https://atproto.social/ontology/tools.ozone.moderation.defs#subjectStatusView>;
        rdfs:range    <xsd:string>;
        rdfs:comment  "Sticky comment on the subject." .

<https://atproto.social/ontology/tools.ozone.moderation.defs#subjectStatusView/muteReportingUntil>
        a            owl:DatatypeProperty;
        rdfs:domain  <https://atproto.social/ontology/tools.ozone.moderation.defs#subjectStatusView>;
        rdfs:range   <xsd:string> .

<https://atproto.social/ontology/tools.ozone.moderation.defs#subjectStatusView/lastReviewedBy>
        a            owl:DatatypeProperty;
        rdfs:domain  <https://atproto.social/ontology/tools.ozone.moderation.defs#subjectStatusView>;
        rdfs:range   <xsd:string> .

<https://atproto.social/ontology/tools.ozone.moderation.defs#subjectStatusView/accountStats>
        a             owl:ObjectProperty;
        rdfs:domain   <https://atproto.social/ontology/tools.ozone.moderation.defs#subjectStatusView>;
        rdfs:range    <https://atproto.social/ontology/tools.ozone.moderation.defs#accountStats>;
        rdfs:comment  "Statistics related to the account subject" .

<https://atproto.social/ontology/tools.ozone.moderation.defs#subjectStatusView/recordsStats>
        a             owl:ObjectProperty;
        rdfs:domain   <https://atproto.social/ontology/tools.ozone.moderation.defs#subjectStatusView>;
        rdfs:range    <https://atproto.social/ontology/tools.ozone.moderation.defs#recordsStats>;
        rdfs:comment  "Statistics related to the record subjects authored by the subject's account" .

<https://atproto.social/ontology/tools.ozone.moderation.defs#subjectStatusView/id>
        a            owl:DatatypeProperty;
        rdfs:domain  <https://atproto.social/ontology/tools.ozone.moderation.defs#subjectStatusView>;
        rdfs:range   <xsd:integer> .

<https://atproto.social/ontology/tools.ozone.moderation.defs#subjectStatusView/subjectRepoHandle>
        a            owl:DatatypeProperty;
        rdfs:domain  <https://atproto.social/ontology/tools.ozone.moderation.defs#subjectStatusView>;
        rdfs:range   <xsd:string> .

<https://atproto.social/ontology/tools.ozone.moderation.defs#subjectStatusView/reviewState>
        a            owl:ObjectProperty;
        rdfs:domain  <https://atproto.social/ontology/tools.ozone.moderation.defs#subjectStatusView>;
        rdfs:range   <https://atproto.social/ontology/tools.ozone.moderation.defs#subjectReviewState> .

<https://atproto.social/ontology/tools.ozone.moderation.defs#subjectStatusView/lastAppealedAt>
        a             owl:DatatypeProperty;
        rdfs:domain   <https://atproto.social/ontology/tools.ozone.moderation.defs#subjectStatusView>;
        rdfs:range    <xsd:string>;
        rdfs:comment  "Timestamp referencing when the author of the subject appealed a moderation action" .

<https://atproto.social/ontology/tools.ozone.moderation.defs#subjectStatusView/takendown>
        a            owl:DatatypeProperty;
        rdfs:domain  <https://atproto.social/ontology/tools.ozone.moderation.defs#subjectStatusView>;
        rdfs:range   <xsd:boolean> .

<https://atproto.social/ontology/tools.ozone.moderation.defs#subjectStatusView/tags>
        a            owl:DatatypeProperty;
        rdfs:domain  <https://atproto.social/ontology/tools.ozone.moderation.defs#subjectStatusView>;
        rdfs:range   <xsd:string> .

<https://atproto.social/ontology/tools.ozone.moderation.defs#subjectStatusView/subjectBlobCids>
        a            owl:DatatypeProperty;
        rdfs:domain  <https://atproto.social/ontology/tools.ozone.moderation.defs#subjectStatusView>;
        rdfs:range   <xsd:string> .

<https://atproto.social/ontology/tools.ozone.moderation.defs#subjectStatusView/updatedAt>
        a             owl:DatatypeProperty;
        rdfs:domain   <https://atproto.social/ontology/tools.ozone.moderation.defs#subjectStatusView>;
        rdfs:range    <xsd:string>;
        rdfs:comment  "Timestamp referencing when the last update was made to the moderation status of the subject" .

<https://atproto.social/ontology/tools.ozone.moderation.defs#subjectStatusView/muteUntil>
        a            owl:DatatypeProperty;
        rdfs:domain  <https://atproto.social/ontology/tools.ozone.moderation.defs#subjectStatusView>;
        rdfs:range   <xsd:string> .

<https://atproto.social/ontology/tools.ozone.moderation.defs#subjectStatusView/lastReportedAt>
        a            owl:DatatypeProperty;
        rdfs:domain  <https://atproto.social/ontology/tools.ozone.moderation.defs#subjectStatusView>;
        rdfs:range   <xsd:string> .

<https://atproto.social/ontology/tools.ozone.moderation.defs#subjectStatusView/appealed>
        a             owl:DatatypeProperty;
        rdfs:domain   <https://atproto.social/ontology/tools.ozone.moderation.defs#subjectStatusView>;
        rdfs:range    <xsd:boolean>;
        rdfs:comment  "True indicates that the a previously taken moderator action was appealed against, by the author of the content. False indicates last appeal was resolved by moderators." .

<https://atproto.social/ontology/tools.ozone.moderation.defs#accountStats>
        a             owl:Class;
        rdfs:comment  "Statistics about a particular account subject" .

<https://atproto.social/ontology/tools.ozone.moderation.defs#accountStats/reportCount>
        a             owl:DatatypeProperty;
        rdfs:domain   <https://atproto.social/ontology/tools.ozone.moderation.defs#accountStats>;
        rdfs:range    <xsd:integer>;
        rdfs:comment  "Total number of reports on the account" .

<https://atproto.social/ontology/tools.ozone.moderation.defs#accountStats/appealCount>
        a             owl:DatatypeProperty;
        rdfs:domain   <https://atproto.social/ontology/tools.ozone.moderation.defs#accountStats>;
        rdfs:range    <xsd:integer>;
        rdfs:comment  "Total number of appeals against a moderation action on the account" .

<https://atproto.social/ontology/tools.ozone.moderation.defs#accountStats/suspendCount>
        a             owl:DatatypeProperty;
        rdfs:domain   <https://atproto.social/ontology/tools.ozone.moderation.defs#accountStats>;
        rdfs:range    <xsd:integer>;
        rdfs:comment  "Number of times the account was suspended" .

<https://atproto.social/ontology/tools.ozone.moderation.defs#accountStats/escalateCount>
        a             owl:DatatypeProperty;
        rdfs:domain   <https://atproto.social/ontology/tools.ozone.moderation.defs#accountStats>;
        rdfs:range    <xsd:integer>;
        rdfs:comment  "Number of times the account was escalated" .

<https://atproto.social/ontology/tools.ozone.moderation.defs#accountStats/takedownCount>
        a             owl:DatatypeProperty;
        rdfs:domain   <https://atproto.social/ontology/tools.ozone.moderation.defs#accountStats>;
        rdfs:range    <xsd:integer>;
        rdfs:comment  "Number of times the account was taken down" .

<https://atproto.social/ontology/tools.ozone.moderation.defs#reviewNone>
        a             owl:Class;
        rdfs:comment  "Moderator review status of a subject: Unnecessary. Indicates that the subject does not need a review at the moment but there is probably some moderation related metadata available for it" .

<https://atproto.social/ontology/tools.ozone.moderation.defs#modEventMuteReporter>
        a             owl:Class;
        rdfs:comment  "Mute incoming reports from an account" .

<https://atproto.social/ontology/tools.ozone.moderation.defs#modEventMuteReporter/comment>
        a            owl:DatatypeProperty;
        rdfs:domain  <https://atproto.social/ontology/tools.ozone.moderation.defs#modEventMuteReporter>;
        rdfs:range   <xsd:string> .

<https://atproto.social/ontology/tools.ozone.moderation.defs#modEventMuteReporter/durationInHours>
        a             owl:DatatypeProperty;
        rdfs:domain   <https://atproto.social/ontology/tools.ozone.moderation.defs#modEventMuteReporter>;
        rdfs:range    <xsd:integer>;
        rdfs:comment  "Indicates how long the account should remain muted. Falsy value here means a permanent mute." .

<https://atproto.social/ontology/tools.ozone.moderation.defs#modEventTag>
        a             owl:Class;
        rdfs:comment  "Add/Remove a tag on a subject" .

<https://atproto.social/ontology/tools.ozone.moderation.defs#modEventTag/add>
        a             owl:DatatypeProperty;
        rdfs:domain   <https://atproto.social/ontology/tools.ozone.moderation.defs#modEventTag>;
        rdfs:range    <xsd:string>;
        rdfs:comment  "Tags to be added to the subject. If already exists, won't be duplicated." .

<https://atproto.social/ontology/tools.ozone.moderation.defs#modEventTag/remove>
        a             owl:DatatypeProperty;
        rdfs:domain   <https://atproto.social/ontology/tools.ozone.moderation.defs#modEventTag>;
        rdfs:range    <xsd:string>;
        rdfs:comment  "Tags to be removed to the subject. Ignores a tag If it doesn't exist, won't be duplicated." .

<https://atproto.social/ontology/tools.ozone.moderation.defs#modEventTag/comment>
        a             owl:DatatypeProperty;
        rdfs:domain   <https://atproto.social/ontology/tools.ozone.moderation.defs#modEventTag>;
        rdfs:range    <xsd:string>;
        rdfs:comment  "Additional comment about added/removed tags." .

<https://atproto.social/ontology/tools.ozone.moderation.emitEvent#main>
        a             owl:Class;
        rdfs:comment  "Take a moderation action on an actor." .

<https://atproto.social/ontology/tools.ozone.moderation.getEvent#main>
        a             owl:Class;
        rdfs:comment  "Get details about a moderation event." .

<https://atproto.social/ontology/tools.ozone.moderation.getRecord#main>
        a             owl:Class;
        rdfs:comment  "Get details about a record." .

<https://atproto.social/ontology/tools.ozone.moderation.getRecords#main>
        a             owl:Class;
        rdfs:comment  "Get details about some records." .

<https://atproto.social/ontology/tools.ozone.moderation.getRepo#main>
        a             owl:Class;
        rdfs:comment  "Get details about a repository." .

<https://atproto.social/ontology/tools.ozone.moderation.getReporterStats#main>
        a             owl:Class;
        rdfs:comment  "Get reporter stats for a list of users." .

<https://atproto.social/ontology/tools.ozone.moderation.getRepos#main>
        a             owl:Class;
        rdfs:comment  "Get details about some repositories." .

<https://atproto.social/ontology/tools.ozone.moderation.getSubjects#main>
        a             owl:Class;
        rdfs:comment  "Get details about subjects." .

<https://atproto.social/ontology/tools.ozone.moderation.queryEvents#main>
        a             owl:Class;
        rdfs:comment  "List moderation events related to a subject." .

<https://atproto.social/ontology/tools.ozone.moderation.queryStatuses#main>
        a             owl:Class;
        rdfs:comment  "View moderation statuses of subjects (record or repo)." .

<https://atproto.social/ontology/tools.ozone.moderation.searchRepos#main>
        a             owl:Class;
        rdfs:comment  "Find repositories based on a search term." .

<https://atproto.social/ontology/tools.ozone.server.getConfig#viewerConfig>
        a       owl:Class .

<https://atproto.social/ontology/tools.ozone.server.getConfig#viewerConfig/role>
        a            owl:DatatypeProperty;
        rdfs:domain  <https://atproto.social/ontology/tools.ozone.server.getConfig#viewerConfig>;
        rdfs:range   <xsd:string> .

<https://atproto.social/ontology/tools.ozone.server.getConfig#main>
        a             owl:Class;
        rdfs:comment  "Get details about ozone's server configuration." .

<https://atproto.social/ontology/tools.ozone.server.getConfig#serviceConfig>
        a       owl:Class .

<https://atproto.social/ontology/tools.ozone.server.getConfig#serviceConfig/url>
        a            owl:DatatypeProperty;
        rdfs:domain  <https://atproto.social/ontology/tools.ozone.server.getConfig#serviceConfig>;
        rdfs:range   <xsd:string> .

<https://atproto.social/ontology/tools.ozone.set.addValues#main>
        a             owl:Class;
        rdfs:comment  "Add values to a specific set. Attempting to add values to a set that does not exist will result in an error." .

<https://atproto.social/ontology/tools.ozone.set.defs#set>
        a       owl:Class .

<https://atproto.social/ontology/tools.ozone.set.defs#set/name>
        a            owl:DatatypeProperty;
        rdfs:domain  <https://atproto.social/ontology/tools.ozone.set.defs#set>;
        rdfs:range   <xsd:string> .

<https://atproto.social/ontology/tools.ozone.set.defs#set/description>
        a            owl:DatatypeProperty;
        rdfs:domain  <https://atproto.social/ontology/tools.ozone.set.defs#set>;
        rdfs:range   <xsd:string> .

<https://atproto.social/ontology/tools.ozone.set.defs#setView>
        a       owl:Class .

<https://atproto.social/ontology/tools.ozone.set.defs#setView/name>
        a            owl:DatatypeProperty;
        rdfs:domain  <https://atproto.social/ontology/tools.ozone.set.defs#setView>;
        rdfs:range   <xsd:string> .

<https://atproto.social/ontology/tools.ozone.set.defs#setView/description>
        a            owl:DatatypeProperty;
        rdfs:domain  <https://atproto.social/ontology/tools.ozone.set.defs#setView>;
        rdfs:range   <xsd:string> .

<https://atproto.social/ontology/tools.ozone.set.defs#setView/setSize>
        a            owl:DatatypeProperty;
        rdfs:domain  <https://atproto.social/ontology/tools.ozone.set.defs#setView>;
        rdfs:range   <xsd:integer> .

<https://atproto.social/ontology/tools.ozone.set.defs#setView/createdAt>
        a            owl:DatatypeProperty;
        rdfs:domain  <https://atproto.social/ontology/tools.ozone.set.defs#setView>;
        rdfs:range   <xsd:string> .

<https://atproto.social/ontology/tools.ozone.set.defs#setView/updatedAt>
        a            owl:DatatypeProperty;
        rdfs:domain  <https://atproto.social/ontology/tools.ozone.set.defs#setView>;
        rdfs:range   <xsd:string> .

<https://atproto.social/ontology/tools.ozone.set.deleteSet#main>
        a             owl:Class;
        rdfs:comment  "Delete an entire set. Attempting to delete a set that does not exist will result in an error." .

<https://atproto.social/ontology/tools.ozone.set.deleteValues#main>
        a             owl:Class;
        rdfs:comment  "Delete values from a specific set. Attempting to delete values that are not in the set will not result in an error" .

<https://atproto.social/ontology/tools.ozone.set.getValues#main>
        a             owl:Class;
        rdfs:comment  "Get a specific set and its values" .

<https://atproto.social/ontology/tools.ozone.set.querySets#main>
        a             owl:Class;
        rdfs:comment  "Query available sets" .

<https://atproto.social/ontology/tools.ozone.set.upsertSet#main>
        a             owl:Class;
        rdfs:comment  "Create or update set metadata" .

<https://atproto.social/ontology/tools.ozone.setting.defs#option>
        a       owl:Class .

<https://atproto.social/ontology/tools.ozone.setting.defs#option/did>
        a            owl:DatatypeProperty;
        rdfs:domain  <https://atproto.social/ontology/tools.ozone.setting.defs#option>;
        rdfs:range   <xsd:string> .

<https://atproto.social/ontology/tools.ozone.setting.defs#option/createdAt>
        a            owl:DatatypeProperty;
        rdfs:domain  <https://atproto.social/ontology/tools.ozone.setting.defs#option>;
        rdfs:range   <xsd:string> .

<https://atproto.social/ontology/tools.ozone.setting.defs#option/updatedAt>
        a            owl:DatatypeProperty;
        rdfs:domain  <https://atproto.social/ontology/tools.ozone.setting.defs#option>;
        rdfs:range   <xsd:string> .

<https://atproto.social/ontology/tools.ozone.setting.defs#option/scope>
        a            owl:DatatypeProperty;
        rdfs:domain  <https://atproto.social/ontology/tools.ozone.setting.defs#option>;
        rdfs:range   <xsd:string> .

<https://atproto.social/ontology/tools.ozone.setting.defs#option/lastUpdatedBy>
        a            owl:DatatypeProperty;
        rdfs:domain  <https://atproto.social/ontology/tools.ozone.setting.defs#option>;
        rdfs:range   <xsd:string> .

<https://atproto.social/ontology/tools.ozone.setting.defs#option/key>
        a            owl:DatatypeProperty;
        rdfs:domain  <https://atproto.social/ontology/tools.ozone.setting.defs#option>;
        rdfs:range   <xsd:string> .

<https://atproto.social/ontology/tools.ozone.setting.defs#option/value>
        a            owl:ObjectProperty;
        rdfs:domain  <https://atproto.social/ontology/tools.ozone.setting.defs#option> .

<https://atproto.social/ontology/tools.ozone.setting.defs#option/description>
        a            owl:DatatypeProperty;
        rdfs:domain  <https://atproto.social/ontology/tools.ozone.setting.defs#option>;
        rdfs:range   <xsd:string> .

<https://atproto.social/ontology/tools.ozone.setting.defs#option/managerRole>
        a            owl:DatatypeProperty;
        rdfs:domain  <https://atproto.social/ontology/tools.ozone.setting.defs#option>;
        rdfs:range   <xsd:string> .

<https://atproto.social/ontology/tools.ozone.setting.defs#option/createdBy>
        a            owl:DatatypeProperty;
        rdfs:domain  <https://atproto.social/ontology/tools.ozone.setting.defs#option>;
        rdfs:range   <xsd:string> .

<https://atproto.social/ontology/tools.ozone.setting.listOptions#main>
        a             owl:Class;
        rdfs:comment  "List settings with optional filtering" .

<https://atproto.social/ontology/tools.ozone.setting.removeOptions#main>
        a             owl:Class;
        rdfs:comment  "Delete settings by key" .

<https://atproto.social/ontology/tools.ozone.setting.upsertOption#main>
        a             owl:Class;
        rdfs:comment  "Create or update setting option" .

<https://atproto.social/ontology/tools.ozone.signature.defs#sigDetail>
        a       owl:Class .

<https://atproto.social/ontology/tools.ozone.signature.defs#sigDetail/property>
        a            owl:DatatypeProperty;
        rdfs:domain  <https://atproto.social/ontology/tools.ozone.signature.defs#sigDetail>;
        rdfs:range   <xsd:string> .

<https://atproto.social/ontology/tools.ozone.signature.defs#sigDetail/value>
        a            owl:DatatypeProperty;
        rdfs:domain  <https://atproto.social/ontology/tools.ozone.signature.defs#sigDetail>;
        rdfs:range   <xsd:string> .

<https://atproto.social/ontology/tools.ozone.signature.findCorrelation#main>
        a             owl:Class;
        rdfs:comment  "Find all correlated threat signatures between 2 or more accounts." .

<https://atproto.social/ontology/tools.ozone.signature.findRelatedAccounts#main>
        a             owl:Class;
        rdfs:comment  "Get accounts that share some matching threat signatures with the root account." .

<https://atproto.social/ontology/tools.ozone.signature.findRelatedAccounts#relatedAccount>
        a       owl:Class .

<https://atproto.social/ontology/tools.ozone.signature.findRelatedAccounts#relatedAccount/account>
        a            owl:ObjectProperty;
        rdfs:domain  <https://atproto.social/ontology/tools.ozone.signature.findRelatedAccounts#relatedAccount>;
        rdfs:range   <https://atproto.social/ontology/com.atproto.admin.defs#accountView> .

<https://atproto.social/ontology/tools.ozone.signature.findRelatedAccounts#relatedAccount/similarities>
        a            owl:ObjectProperty;
        rdfs:domain  <https://atproto.social/ontology/tools.ozone.signature.findRelatedAccounts#relatedAccount>;
        rdfs:range   <https://atproto.social/ontology/tools.ozone.signature.defs#sigDetail> .

<https://atproto.social/ontology/tools.ozone.signature.searchAccounts#main>
        a             owl:Class;
        rdfs:comment  "Search for accounts that match one or more threat signature values." .

<https://atproto.social/ontology/tools.ozone.team.addMember#main>
        a             owl:Class;
        rdfs:comment  "Add a member to the ozone team. Requires admin role." .

<https://atproto.social/ontology/tools.ozone.team.defs#roleAdmin>
        a             owl:Class;
        rdfs:comment  "Admin role. Highest level of access, can perform all actions." .

<https://atproto.social/ontology/tools.ozone.team.defs#roleModerator>
        a             owl:Class;
        rdfs:comment  "Moderator role. Can perform most actions." .

<https://atproto.social/ontology/tools.ozone.team.defs#roleTriage>
        a             owl:Class;
        rdfs:comment  "Triage role. Mostly intended for monitoring and escalating issues." .

<https://atproto.social/ontology/tools.ozone.team.defs#roleVerifier>
        a             owl:Class;
        rdfs:comment  "Verifier role. Only allowed to issue verifications." .

<https://atproto.social/ontology/tools.ozone.team.defs#member>
        a       owl:Class .

<https://atproto.social/ontology/tools.ozone.team.defs#member/profile>
        a            owl:ObjectProperty;
        rdfs:domain  <https://atproto.social/ontology/tools.ozone.team.defs#member>;
        rdfs:range   <https://atproto.social/ontology/app.bsky.actor.defs#profileViewDetailed> .

<https://atproto.social/ontology/tools.ozone.team.defs#member/createdAt>
        a            owl:DatatypeProperty;
        rdfs:domain  <https://atproto.social/ontology/tools.ozone.team.defs#member>;
        rdfs:range   <xsd:string> .

<https://atproto.social/ontology/tools.ozone.team.defs#member/updatedAt>
        a            owl:DatatypeProperty;
        rdfs:domain  <https://atproto.social/ontology/tools.ozone.team.defs#member>;
        rdfs:range   <xsd:string> .

<https://atproto.social/ontology/tools.ozone.team.defs#member/lastUpdatedBy>
        a            owl:DatatypeProperty;
        rdfs:domain  <https://atproto.social/ontology/tools.ozone.team.defs#member>;
        rdfs:range   <xsd:string> .

<https://atproto.social/ontology/tools.ozone.team.defs#member/role>
        a            owl:DatatypeProperty;
        rdfs:domain  <https://atproto.social/ontology/tools.ozone.team.defs#member>;
        rdfs:range   <xsd:string> .

<https://atproto.social/ontology/tools.ozone.team.defs#member/did>
        a            owl:DatatypeProperty;
        rdfs:domain  <https://atproto.social/ontology/tools.ozone.team.defs#member>;
        rdfs:range   <xsd:string> .

<https://atproto.social/ontology/tools.ozone.team.defs#member/disabled>
        a            owl:DatatypeProperty;
        rdfs:domain  <https://atproto.social/ontology/tools.ozone.team.defs#member>;
        rdfs:range   <xsd:boolean> .

<https://atproto.social/ontology/tools.ozone.team.deleteMember#main>
        a             owl:Class;
        rdfs:comment  "Delete a member from ozone team. Requires admin role." .

<https://atproto.social/ontology/tools.ozone.team.listMembers#main>
        a             owl:Class;
        rdfs:comment  "List all members with access to the ozone service." .

<https://atproto.social/ontology/tools.ozone.team.updateMember#main>
        a             owl:Class;
        rdfs:comment  "Update a member in the ozone service. Requires admin role." .

<https://atproto.social/ontology/tools.ozone.verification.defs#verificationView>
        a             owl:Class;
        rdfs:comment  "Verification data for the associated subject." .

<https://atproto.social/ontology/tools.ozone.verification.defs#verificationView/uri>
        a             owl:DatatypeProperty;
        rdfs:domain   <https://atproto.social/ontology/tools.ozone.verification.defs#verificationView>;
        rdfs:range    <xsd:string>;
        rdfs:comment  "The AT-URI of the verification record." .

<https://atproto.social/ontology/tools.ozone.verification.defs#verificationView/subject>
        a             owl:DatatypeProperty;
        rdfs:domain   <https://atproto.social/ontology/tools.ozone.verification.defs#verificationView>;
        rdfs:range    <xsd:string>;
        rdfs:comment  "The subject of the verification." .

<https://atproto.social/ontology/tools.ozone.verification.defs#verificationView/handle>
        a             owl:DatatypeProperty;
        rdfs:domain   <https://atproto.social/ontology/tools.ozone.verification.defs#verificationView>;
        rdfs:range    <xsd:string>;
        rdfs:comment  "Handle of the subject the verification applies to at the moment of verifying, which might not be the same at the time of viewing. The verification is only valid if the current handle matches the one at the time of verifying." .

<https://atproto.social/ontology/tools.ozone.verification.defs#verificationView/displayName>
        a             owl:DatatypeProperty;
        rdfs:domain   <https://atproto.social/ontology/tools.ozone.verification.defs#verificationView>;
        rdfs:range    <xsd:string>;
        rdfs:comment  "Display name of the subject the verification applies to at the moment of verifying, which might not be the same at the time of viewing. The verification is only valid if the current displayName matches the one at the time of verifying." .

<https://atproto.social/ontology/tools.ozone.verification.defs#verificationView/createdAt>
        a             owl:DatatypeProperty;
        rdfs:domain   <https://atproto.social/ontology/tools.ozone.verification.defs#verificationView>;
        rdfs:range    <xsd:string>;
        rdfs:comment  "Timestamp when the verification was created." .

<https://atproto.social/ontology/tools.ozone.verification.defs#verificationView/revokedAt>
        a             owl:DatatypeProperty;
        rdfs:domain   <https://atproto.social/ontology/tools.ozone.verification.defs#verificationView>;
        rdfs:range    <xsd:string>;
        rdfs:comment  "Timestamp when the verification was revoked." .

<https://atproto.social/ontology/tools.ozone.verification.defs#verificationView/revokedBy>
        a             owl:DatatypeProperty;
        rdfs:domain   <https://atproto.social/ontology/tools.ozone.verification.defs#verificationView>;
        rdfs:range    <xsd:string>;
        rdfs:comment  "The user who revoked this verification." .

<https://atproto.social/ontology/tools.ozone.verification.defs#verificationView/revokeReason>
        a             owl:DatatypeProperty;
        rdfs:domain   <https://atproto.social/ontology/tools.ozone.verification.defs#verificationView>;
        rdfs:range    <xsd:string>;
        rdfs:comment  "Describes the reason for revocation, also indicating that the verification is no longer valid." .

<https://atproto.social/ontology/tools.ozone.verification.defs#verificationView/subjectProfile>
        a            owl:ObjectProperty;
        rdfs:domain  <https://atproto.social/ontology/tools.ozone.verification.defs#verificationView> .

<https://atproto.social/ontology/tools.ozone.verification.defs#verificationView/issuerProfile>
        a            owl:ObjectProperty;
        rdfs:domain  <https://atproto.social/ontology/tools.ozone.verification.defs#verificationView> .

<https://atproto.social/ontology/tools.ozone.verification.defs#verificationView/subjectRepo>
        a            owl:ObjectProperty;
        rdfs:domain  <https://atproto.social/ontology/tools.ozone.verification.defs#verificationView> .

<https://atproto.social/ontology/tools.ozone.verification.defs#verificationView/issuerRepo>
        a            owl:ObjectProperty;
        rdfs:domain  <https://atproto.social/ontology/tools.ozone.verification.defs#verificationView> .

<https://atproto.social/ontology/tools.ozone.verification.defs#verificationView/issuer>
        a             owl:DatatypeProperty;
        rdfs:domain   <https://atproto.social/ontology/tools.ozone.verification.defs#verificationView>;
        rdfs:range    <xsd:string>;
        rdfs:comment  "The user who issued this verification." .

<https://atproto.social/ontology/tools.ozone.verification.grantVerifications#grantError>
        a             owl:Class;
        rdfs:comment  "Error object for failed verifications." .

<https://atproto.social/ontology/tools.ozone.verification.grantVerifications#grantError/error>
        a             owl:DatatypeProperty;
        rdfs:domain   <https://atproto.social/ontology/tools.ozone.verification.grantVerifications#grantError>;
        rdfs:range    <xsd:string>;
        rdfs:comment  "Error message describing the reason for failure." .

<https://atproto.social/ontology/tools.ozone.verification.grantVerifications#grantError/subject>
        a             owl:DatatypeProperty;
        rdfs:domain   <https://atproto.social/ontology/tools.ozone.verification.grantVerifications#grantError>;
        rdfs:range    <xsd:string>;
        rdfs:comment  "The did of the subject being verified" .

<https://atproto.social/ontology/tools.ozone.verification.grantVerifications#main>
        a             owl:Class;
        rdfs:comment  "Grant verifications to multiple subjects. Allows batch processing of up to 100 verifications at once." .

<https://atproto.social/ontology/tools.ozone.verification.grantVerifications#verificationInput>
        a       owl:Class .

<https://atproto.social/ontology/tools.ozone.verification.grantVerifications#verificationInput/handle>
        a             owl:DatatypeProperty;
        rdfs:domain   <https://atproto.social/ontology/tools.ozone.verification.grantVerifications#verificationInput>;
        rdfs:range    <xsd:string>;
        rdfs:comment  "Handle of the subject the verification applies to at the moment of verifying." .

<https://atproto.social/ontology/tools.ozone.verification.grantVerifications#verificationInput/displayName>
        a             owl:DatatypeProperty;
        rdfs:domain   <https://atproto.social/ontology/tools.ozone.verification.grantVerifications#verificationInput>;
        rdfs:range    <xsd:string>;
        rdfs:comment  "Display name of the subject the verification applies to at the moment of verifying." .

<https://atproto.social/ontology/tools.ozone.verification.grantVerifications#verificationInput/createdAt>
        a             owl:DatatypeProperty;
        rdfs:domain   <https://atproto.social/ontology/tools.ozone.verification.grantVerifications#verificationInput>;
        rdfs:range    <xsd:string>;
        rdfs:comment  "Timestamp for verification record. Defaults to current time when not specified." .

<https://atproto.social/ontology/tools.ozone.verification.grantVerifications#verificationInput/subject>
        a             owl:DatatypeProperty;
        rdfs:domain   <https://atproto.social/ontology/tools.ozone.verification.grantVerifications#verificationInput>;
        rdfs:range    <xsd:string>;
        rdfs:comment  "The did of the subject being verified" .

<https://atproto.social/ontology/tools.ozone.verification.listVerifications#main>
        a             owl:Class;
        rdfs:comment  "List verifications" .

<https://atproto.social/ontology/tools.ozone.verification.revokeVerifications#main>
        a             owl:Class;
        rdfs:comment  "Revoke previously granted verifications in batches of up to 100." .

<https://atproto.social/ontology/tools.ozone.verification.revokeVerifications#revokeError>
        a             owl:Class;
        rdfs:comment  "Error object for failed revocations" .

<https://atproto.social/ontology/tools.ozone.verification.revokeVerifications#revokeError/uri>
        a             owl:DatatypeProperty;
        rdfs:domain   <https://atproto.social/ontology/tools.ozone.verification.revokeVerifications#revokeError>;
        rdfs:range    <xsd:string>;
        rdfs:comment  "The AT-URI of the verification record that failed to revoke." .

<https://atproto.social/ontology/tools.ozone.verification.revokeVerifications#revokeError/error>
        a             owl:DatatypeProperty;
        rdfs:domain   <https://atproto.social/ontology/tools.ozone.verification.revokeVerifications#revokeError>;
        rdfs:range    <xsd:string>;
        rdfs:comment  "Description of the error that occurred during revocation." .
